@prefix : <http://data.finance.gov.au/def/agrif#> .
@prefix dc: <http://purl.org/dc/elements/1.1/> .
@prefix owl: <http://www.w3.org/2002/07/owl#> .
@prefix rdf: <http://www.w3.org/1999/02/22-rdf-syntax-ns#> .
@prefix xml: <http://www.w3.org/XML/1998/namespace> .
@prefix xsd: <http://www.w3.org/2001/XMLSchema#> .
@prefix rdfs: <http://www.w3.org/2000/01/rdf-schema#> .
@prefix skos: <http://www.w3.org/2004/02/skos/core#> .
@prefix terms: <http://purl.org/dc/terms/> .
@base <http://data.finance.gov.au/def/agrif> .

<http://data.finance.gov.au/def/agrif> rdf:type owl:Ontology .


#################################################################
#
#    Annotation properties
#
#################################################################


###  http://purl.org/dc/elements/1.1/contributor

dc:contributor rdf:type owl:AnnotationProperty .



###  http://purl.org/dc/elements/1.1/coverage

dc:coverage rdf:type owl:AnnotationProperty .



###  http://purl.org/dc/elements/1.1/creator

dc:creator rdf:type owl:AnnotationProperty .



###  http://purl.org/dc/elements/1.1/date

dc:date rdf:type owl:AnnotationProperty .



###  http://purl.org/dc/elements/1.1/description

dc:description rdf:type owl:AnnotationProperty .



###  http://purl.org/dc/elements/1.1/format

dc:format rdf:type owl:AnnotationProperty .



###  http://purl.org/dc/elements/1.1/identifier

dc:identifier rdf:type owl:AnnotationProperty .



###  http://purl.org/dc/elements/1.1/language

dc:language rdf:type owl:AnnotationProperty .



###  http://purl.org/dc/elements/1.1/publisher

dc:publisher rdf:type owl:AnnotationProperty .



###  http://purl.org/dc/elements/1.1/relation

dc:relation rdf:type owl:AnnotationProperty .



###  http://purl.org/dc/elements/1.1/rights

dc:rights rdf:type owl:AnnotationProperty .



###  http://purl.org/dc/elements/1.1/source

dc:source rdf:type owl:AnnotationProperty .



###  http://purl.org/dc/elements/1.1/subject

dc:subject rdf:type owl:AnnotationProperty .



###  http://purl.org/dc/elements/1.1/title

dc:title rdf:type owl:AnnotationProperty .



###  http://purl.org/dc/elements/1.1/type

dc:type rdf:type owl:AnnotationProperty .



###  http://purl.org/dc/terms/abstract

terms:abstract rdf:type owl:AnnotationProperty ;
               
               rdfs:subPropertyOf dc:description ,
                                  terms:description .



###  http://purl.org/dc/terms/accessRights

terms:accessRights rdf:type owl:AnnotationProperty ;
                   
                   rdfs:subPropertyOf dc:rights .



###  http://purl.org/dc/terms/alternative

terms:alternative rdf:type owl:AnnotationProperty ;
                  
                  rdfs:subPropertyOf dc:title .



###  http://purl.org/dc/terms/available

terms:available rdf:type owl:AnnotationProperty ;
                
                rdfs:subPropertyOf dc:date .



###  http://purl.org/dc/terms/bibliographicCitation

terms:bibliographicCitation rdf:type owl:AnnotationProperty ;
                            
                            rdfs:subPropertyOf dc:identifier ;
                            
                            rdfs:domain terms:BibliographicResource .



###  http://purl.org/dc/terms/conformsTo

terms:conformsTo rdf:type owl:AnnotationProperty ;
                 
                 rdfs:subPropertyOf dc:relation ,
                                    terms:relation .



###  http://purl.org/dc/terms/contributor

terms:contributor rdf:type owl:AnnotationProperty ;
                  
                  rdfs:subPropertyOf dc:contributor .



###  http://purl.org/dc/terms/coverage

terms:coverage rdf:type owl:AnnotationProperty ;
               
               rdfs:subPropertyOf dc:coverage .



###  http://purl.org/dc/terms/created

terms:created rdf:type owl:AnnotationProperty ;
              
              rdfs:subPropertyOf dc:date .



###  http://purl.org/dc/terms/creator

terms:creator rdf:type owl:AnnotationProperty ;
              
              rdfs:subPropertyOf dc:creator .



###  http://purl.org/dc/terms/date

terms:date rdf:type owl:AnnotationProperty ;
           
           rdfs:subPropertyOf dc:date .



###  http://purl.org/dc/terms/dateAccepted

terms:dateAccepted rdf:type owl:AnnotationProperty ;
                   
                   rdfs:subPropertyOf dc:date .



###  http://purl.org/dc/terms/dateCopyrighted

terms:dateCopyrighted rdf:type owl:AnnotationProperty ;
                      
                      rdfs:subPropertyOf dc:date .



###  http://purl.org/dc/terms/dateSubmitted

terms:dateSubmitted rdf:type owl:AnnotationProperty ;
                    
                    rdfs:subPropertyOf dc:date .



###  http://purl.org/dc/terms/description

terms:description rdf:type owl:AnnotationProperty ;
                  
                  rdfs:subPropertyOf dc:description .



###  http://purl.org/dc/terms/extent

terms:extent rdf:type owl:AnnotationProperty ;
             
             rdfs:subPropertyOf dc:format .



###  http://purl.org/dc/terms/format

terms:format rdf:type owl:AnnotationProperty ;
             
             rdfs:subPropertyOf dc:format .



###  http://purl.org/dc/terms/hasFormat

terms:hasFormat rdf:type owl:AnnotationProperty ;
                
                rdfs:subPropertyOf dc:relation ,
                                   terms:relation .



###  http://purl.org/dc/terms/hasPart

terms:hasPart rdf:type owl:AnnotationProperty ;
              
              rdfs:subPropertyOf dc:relation ,
                                 terms:relation .



###  http://purl.org/dc/terms/hasVersion

terms:hasVersion rdf:type owl:AnnotationProperty ;
                 
                 rdfs:subPropertyOf dc:relation ,
                                    terms:relation .



###  http://purl.org/dc/terms/identifier

terms:identifier rdf:type owl:AnnotationProperty ;
                 
                 rdfs:subPropertyOf dc:identifier .



###  http://purl.org/dc/terms/isFormatOf

terms:isFormatOf rdf:type owl:AnnotationProperty ;
                 
                 rdfs:subPropertyOf dc:relation ,
                                    terms:relation .



###  http://purl.org/dc/terms/isPartOf

terms:isPartOf rdf:type owl:AnnotationProperty ;
               
               rdfs:subPropertyOf dc:relation ,
                                  terms:relation .



###  http://purl.org/dc/terms/isReferencedBy

terms:isReferencedBy rdf:type owl:AnnotationProperty ;
                     
                     rdfs:subPropertyOf dc:relation ,
                                        terms:relation .



###  http://purl.org/dc/terms/isReplacedBy

terms:isReplacedBy rdf:type owl:AnnotationProperty ;
                   
                   rdfs:subPropertyOf dc:relation ,
                                      terms:relation .



###  http://purl.org/dc/terms/isRequiredBy

terms:isRequiredBy rdf:type owl:AnnotationProperty ;
                   
                   rdfs:subPropertyOf dc:relation ,
                                      terms:relation .



###  http://purl.org/dc/terms/isVersionOf

terms:isVersionOf rdf:type owl:AnnotationProperty ;
                  
                  rdfs:subPropertyOf dc:relation ,
                                     terms:relation .



###  http://purl.org/dc/terms/issued

terms:issued rdf:type owl:AnnotationProperty ;
             
             rdfs:subPropertyOf dc:date .



###  http://purl.org/dc/terms/language

terms:language rdf:type owl:AnnotationProperty ;
               
               rdfs:subPropertyOf dc:language .



###  http://purl.org/dc/terms/license

terms:license rdf:type owl:AnnotationProperty ;
              
              rdfs:subPropertyOf dc:rights .



###  http://purl.org/dc/terms/medium

terms:medium rdf:type owl:AnnotationProperty ;
             
             rdfs:subPropertyOf dc:format .



###  http://purl.org/dc/terms/modified

terms:modified rdf:type owl:AnnotationProperty ;
               
               rdfs:subPropertyOf dc:date .



###  http://purl.org/dc/terms/publisher

terms:publisher rdf:type owl:AnnotationProperty ;
                
                rdfs:subPropertyOf dc:publisher .



###  http://purl.org/dc/terms/references

terms:references rdf:type owl:AnnotationProperty ;
                 
                 rdfs:subPropertyOf dc:relation ,
                                    terms:relation .



###  http://purl.org/dc/terms/relation

terms:relation rdf:type owl:AnnotationProperty ;
               
               rdfs:subPropertyOf dc:relation .



###  http://purl.org/dc/terms/replaces

terms:replaces rdf:type owl:AnnotationProperty ;
               
               rdfs:subPropertyOf dc:relation ,
                                  terms:relation .



###  http://purl.org/dc/terms/requires

terms:requires rdf:type owl:AnnotationProperty ;
               
               rdfs:subPropertyOf dc:relation ,
                                  terms:relation .



###  http://purl.org/dc/terms/rights

terms:rights rdf:type owl:AnnotationProperty ;
             
             rdfs:subPropertyOf dc:rights .



###  http://purl.org/dc/terms/source

terms:source rdf:type owl:AnnotationProperty ;
             
             rdfs:subPropertyOf dc:source ,
                                terms:relation .



###  http://purl.org/dc/terms/spatial

terms:spatial rdf:type owl:AnnotationProperty ;
              
              rdfs:subPropertyOf dc:coverage .



###  http://purl.org/dc/terms/subject

terms:subject rdf:type owl:AnnotationProperty ;
              
              rdfs:subPropertyOf dc:subject .



###  http://purl.org/dc/terms/tableOfContents

terms:tableOfContents rdf:type owl:AnnotationProperty ;
                      
                      rdfs:subPropertyOf dc:description ,
                                         terms:description .



###  http://purl.org/dc/terms/temporal

terms:temporal rdf:type owl:AnnotationProperty ;
               
               rdfs:subPropertyOf dc:coverage .



###  http://purl.org/dc/terms/title

terms:title rdf:type owl:AnnotationProperty ;
            
            rdfs:subPropertyOf dc:title .



###  http://purl.org/dc/terms/type

terms:type rdf:type owl:AnnotationProperty ;
           
           rdfs:subPropertyOf dc:type .



###  http://purl.org/dc/terms/valid

terms:valid rdf:type owl:AnnotationProperty ;
            
            rdfs:subPropertyOf dc:date .



###  http://www.w3.org/2004/02/skos/core#example

skos:example rdf:type owl:AnnotationProperty .



###  http://www.w3.org/2004/02/skos/core#note

skos:note rdf:type owl:AnnotationProperty .





#################################################################
#
#    Datatypes
#
#################################################################


###  http://purl.org/dc/terms/Box

terms:Box rdf:type rdfs:Datatype .



###  http://purl.org/dc/terms/ISO3166

terms:ISO3166 rdf:type rdfs:Datatype .



###  http://purl.org/dc/terms/ISO639-2

terms:ISO639-2 rdf:type rdfs:Datatype .



###  http://purl.org/dc/terms/ISO639-3

terms:ISO639-3 rdf:type rdfs:Datatype .



###  http://purl.org/dc/terms/Period

terms:Period rdf:type rdfs:Datatype .



###  http://purl.org/dc/terms/Point

terms:Point rdf:type rdfs:Datatype .



###  http://purl.org/dc/terms/RFC1766

terms:RFC1766 rdf:type rdfs:Datatype .



###  http://purl.org/dc/terms/RFC3066

terms:RFC3066 rdf:type rdfs:Datatype .



###  http://purl.org/dc/terms/RFC4646

terms:RFC4646 rdf:type rdfs:Datatype .



###  http://purl.org/dc/terms/RFC5646

terms:RFC5646 rdf:type rdfs:Datatype .



###  http://purl.org/dc/terms/URI

terms:URI rdf:type rdfs:Datatype .



###  http://purl.org/dc/terms/W3CDTF

terms:W3CDTF rdf:type rdfs:Datatype .



###  http://www.w3.org/2001/XMLSchema#date

xsd:date rdf:type rdfs:Datatype .





#################################################################
#
#    Object Properties
#
#################################################################


###  http://data.finance.gov.au/def/agrif#accessedBy

:accessedBy rdf:type owl:ObjectProperty ;
            
            rdfs:label "accessed By"@en ;
            
            rdfs:comment "A relation that indicates that an Agent has accessed a Record as defined in an Access Activity."@en ;
            
            rdfs:subPropertyOf :wasAssociatedWith .



###  http://data.finance.gov.au/def/agrif#actsAs

:actsAs rdf:type owl:ObjectProperty ;
        
        rdfs:label "acts As"@en ;
        
        rdfs:comment "A relation between an Agent and the Role that Agent acts in."@en .



###  http://data.finance.gov.au/def/agrif#associatedFunction

:associatedFunction rdf:type owl:ObjectProperty ;
                    
                    rdfs:label "associated Function"@en ;
                    
                    rdfs:comment "A relation that associates a Function to an Entity, Event or Activity."@en .



###  http://data.finance.gov.au/def/agrif#associatedRole

:associatedRole rdf:type owl:ObjectProperty ;
                
                rdfs:label "associated Role"@en ;
                
                dc:source "https://www.w3.org/TR/prov-o/#hadRole" ;
                
                rdfs:comment "An associated Role is a qualified association between a Role and an Activity or Event defined by an Association."@en .



###  http://data.finance.gov.au/def/agrif#guidingPolicy

:guidingPolicy rdf:type owl:ObjectProperty ;
               
               rdfs:label "guiding Policy"@en ;
               
               rdfs:comment "A relation that defines a Policy that is guiding an Activity or Change Event."@en .



###  http://data.finance.gov.au/def/agrif#hasActivity

:hasActivity rdf:type owl:ObjectProperty ;
             
             rdfs:label "has Activity"@en ;
             
             rdfs:comment "A relation between a Record and an Activity that acts upon the Record."@en ;
             
             dc:source "https://www.w3.org/TR/prov-o/#p_activity" .



###  http://data.finance.gov.au/def/agrif#hasAgent

:hasAgent rdf:type owl:ObjectProperty ;
          
          rdfs:label "has Agent"@en ;
          
          rdfs:comment "A qualified relation between an Agent and a Change Event defined through an Association."@en ;
          
          dc:source "https://www.w3.org/TR/prov-o/#p_agent" .



###  http://data.finance.gov.au/def/agrif#hasClassifier

:hasClassifier rdf:type owl:ObjectProperty ;
               
               rdfs:label "has Classifier"@en ;
               
               owl:deprecated ""@en ;
               
               rdfs:subPropertyOf owl:topObjectProperty .



###  http://data.finance.gov.au/def/agrif#hasControl

:hasControl rdf:type owl:ObjectProperty ;
            
            rdfs:label "requires Control"@en ;
            
            rdfs:comment "A relation between a Record, Artefact or Event and a Control that denotes the required level of Access or Security Control." .



###  http://data.finance.gov.au/def/agrif#hasCoverage

:hasCoverage rdf:type owl:ObjectProperty ;
             
             rdfs:label "has Coverage"@en ;
             
             rdfs:comment "A relation between a Record and its Jurisdictional Coverage, or its Temporal or Spatial Coverage."@en .



###  http://data.finance.gov.au/def/agrif#hasDecisionStatus

:hasDecisionStatus rdf:type owl:ObjectProperty ;
                   
                   rdfs:label "has Decision Status"@en ;
                   
                   rdfs:comment "A relation that indicates what the Decision on a Decision Event was."@en .



###  http://data.finance.gov.au/def/agrif#hasDisposalClass

:hasDisposalClass rdf:type owl:ObjectProperty ;
                  
                  rdfs:label "has Disposal Class"@en ;
                  
                  rdfs:comment "A relation that associates a Disposal Class with a Record."@en .



###  http://data.finance.gov.au/def/agrif#hasFormFactor

:hasFormFactor rdf:type owl:ObjectProperty ;
               
               rdfs:label "has Form Factor"@en ;
               
               rdfs:comment "A relation that defines the size, shape, and other physical specifications of a Physical Artefact."@en .



###  http://data.finance.gov.au/def/agrif#hasLocation

:hasLocation rdf:type owl:ObjectProperty ;
             
             rdfs:label "has Location"@en ;
             
             rdfs:comment "A relation that defines the Spatial Location of an Activity or Artefact."@en .



###  http://data.finance.gov.au/def/agrif#hasManifest

:hasManifest rdf:type owl:ObjectProperty ;
             
             rdfs:label "has Manifest"@en ;
             
             rdfs:comment "A relation between a Manifest and a Transfer Event that describes the files involved in the transfer of a Record."@en .



###  http://data.finance.gov.au/def/agrif#hasPart

:hasPart rdf:type owl:ObjectProperty ;
         
         rdfs:label "has Part"@en ;
         
         rdfs:comment "A relation that defines part-whole relations amongst Organisational Units."@en ;
         
         owl:inverseOf :partOf .



###  http://data.finance.gov.au/def/agrif#hasPermission

:hasPermission rdf:type owl:ObjectProperty ;
               
               rdfs:label "has Permission"@en ;
               
               rdfs:comment "A relation between an Agent and the Permission the Agent possesses."@en .



###  http://data.finance.gov.au/def/agrif#hasPrerequisiteDecisionEvent

:hasPrerequisiteDecisionEvent rdf:type owl:ObjectProperty ;
                              
                              rdfs:label "has Prerequisite Decision Event"@en ;
                              
                              rdfs:comment "A relation between a Decision Event and a prerequisite Decision Event, indicating a Decision chain in a Chain of Command."@en .



###  http://data.finance.gov.au/def/agrif#hasQuality

:hasQuality rdf:type owl:ObjectProperty ;
            
            rdfs:label "has Quality"@en ;
            
            rdfs:comment "A relation that indicates a specific Quality of an Artefact."@en .



###  http://data.finance.gov.au/def/agrif#hasSeries

:hasSeries rdf:type owl:ObjectProperty ;
           
           rdfs:label "has Series"@en ;
           
           rdfs:comment "A relation between a Record and its Series Number."@en ;
           
           rdfs:subPropertyOf owl:topObjectProperty .



###  http://data.finance.gov.au/def/agrif#hasStatus

:hasStatus rdf:type owl:ObjectProperty ;
           
           rdfs:label "has Status"@en ;
           
           rdfs:comment "A relation between an Activity and a Status that indicates its current state."@en .



###  http://data.finance.gov.au/def/agrif#hasVersionHistory

:hasVersionHistory rdf:type owl:ObjectProperty ;
                   
                   rdfs:label "has Version History"@en ;
                   
                   rdfs:comment "A relation between a Record and its previous Version qualified through a Replace Event."@en .



###  http://data.finance.gov.au/def/agrif#isChangedBy

:isChangedBy rdf:type owl:ObjectProperty ;
             
             rdfs:label "is Changed By"@en ;
             
             rdfs:comment "A relation between an Artefact or a Record and a Change Event."@en ;
             
             rdfs:subPropertyOf owl:topObjectProperty .



###  http://data.finance.gov.au/def/agrif#notifies

:notifies rdf:type owl:ObjectProperty ;
          
          rdfs:label "notifies"@en ;
          
          rdfs:comment "A relation between a Trigger and an Agent that is to be notified."@en .



###  http://data.finance.gov.au/def/agrif#partOf

:partOf rdf:type owl:ObjectProperty ,
                 owl:TransitiveProperty ;
        
        rdfs:label "part Of"@en ;
        
        rdfs:comment "A relation that defines part-whole relations amongst Organisational Units."@en .



###  http://data.finance.gov.au/def/agrif#positionIn

:positionIn rdf:type owl:ObjectProperty ;
            
            rdfs:label "position In"@en ;
            
            rdfs:comment "A relation that defines the position an Agent occupies in an Organisation or Organisational Unit."@en .



###  http://data.finance.gov.au/def/agrif#qualifiedAssociation

:qualifiedAssociation rdf:type owl:ObjectProperty ;
                      
                      rdfs:label "qualified Association"@en ;
                      
                      rdfs:comment "A relation that associates an assignment of responsibility to an Agent for an Activity or Event, indicating that the Agent had a Role in the Activity or Event."@en .



###  http://data.finance.gov.au/def/agrif#recordOf

:recordOf rdf:type owl:ObjectProperty ;
          
          rdfs:label "record Of"@en ;
          
          rdfs:comment "A relation that defines what Artefact the Record is about."@en .



###  http://data.finance.gov.au/def/agrif#relatedTo

:relatedTo rdf:type owl:ObjectProperty ;
           
           rdfs:label "related To"@en ;
           
           rdfs:comment "A relation that indicates that there is some form of relation between a Record and another Record or between an Artefact and another Artefact."@en .



###  http://data.finance.gov.au/def/agrif#replacedBy

:replacedBy rdf:type owl:ObjectProperty ;
            
            rdfs:label "replaced By"@en ;
            
            rdfs:comment "A relation that defines that a Record has been replaced by another Record, qualified through a Replace Event."@en .



###  http://data.finance.gov.au/def/agrif#replaces

:replaces rdf:type owl:ObjectProperty ;
          
          rdfs:label "replaces"@en ;
          
          rdfs:comment "A relation that defines that a Record replaces another Record, qualified through a Replace Event."@en ;
          
          owl:inverseOf :replacedBy .



###  http://data.finance.gov.au/def/agrif#requiresSecurityClassification

:requiresSecurityClassification rdf:type owl:ObjectProperty ;
                                
                                rdfs:label "requires Security Classification"@en ;
                                
                                rdfs:comment "A relation between a Record and a Security Classification that denotes the required level of Security Clearance an Agent needs to possess to access the Record."@en ;
                                
                                rdfs:subPropertyOf :hasControl .



###  http://data.finance.gov.au/def/agrif#sharedWith

:sharedWith rdf:type owl:ObjectProperty ;
            
            rdfs:label "shared With"@en ;
            
            rdfs:comment "A relation that indicates that a Record was shared with an Agent as defined in a Share Activity."@en ;
            
            rdfs:subPropertyOf :wasAssociatedWith .



###  http://data.finance.gov.au/def/agrif#storedIn

:storedIn rdf:type owl:ObjectProperty ;
          
          rdfs:label "stored In"@en ;
          
          rdfs:comment "A relation that indicates the Storage Location of an Artefact."@en ;
          
          rdfs:subPropertyOf owl:topObjectProperty .



###  http://data.finance.gov.au/def/agrif#transferredFrom

:transferredFrom rdf:type owl:ObjectProperty ;
                 
                 rdfs:label "transferred From"@en ;
                 
                 rdfs:comment "A relation that defines that the Control of a Record has been transferred from that Role."@en .



###  http://data.finance.gov.au/def/agrif#transferredTo

:transferredTo rdf:type owl:ObjectProperty ;
               
               rdfs:label "transferred To"@en ;
               
               rdfs:comment "A relation that defines that the Control of a Record has been transferred to that new Role."@en .



###  http://data.finance.gov.au/def/agrif#triggeredBy

:triggeredBy rdf:type owl:ObjectProperty ;
             
             rdfs:label "triggered By"@en ;
             
             rdfs:comment "A relation that indicates that a Change Event has been initiated by a Trigger."@en .



###  http://data.finance.gov.au/def/agrif#triggers

:triggers rdf:type owl:ObjectProperty ;
          
          rdfs:label "triggers"@en ;
          
          rdfs:comment "A relation that indicates that a Trigger has initiated a Change Event."@en .



###  http://data.finance.gov.au/def/agrif#usedRecord

:usedRecord rdf:type owl:ObjectProperty ;
            
            rdfs:label "used Record"@en ;
            
            rdfs:comment "A relation between an Activity and a Record the Activity uses."@en ;
            
            owl:inverseOf :hasActivity .



###  http://data.finance.gov.au/def/agrif#wasAssociatedWith

:wasAssociatedWith rdf:type owl:ObjectProperty ;
                   
                   rdfs:label "was Associated With"@en ;
                   
                   rdfs:comment "A relation that assigns responsibility of an Agent for an Activity or Change Event."@en ;
                   
                   dc:source "https://www.w3.org/TR/prov-o/#wasAssociatedWith" .



###  http://purl.org/dc/terms/accessRights

terms:accessRights rdf:type owl:ObjectProperty ;
                   
                   rdfs:range terms:RightsStatement ;
                   
                   rdfs:subPropertyOf terms:rights .



###  http://purl.org/dc/terms/accrualMethod

terms:accrualMethod rdf:type owl:ObjectProperty ;
                    
                    rdfs:domain <http://purl.org/dc/dcmitype/Collection> ;
                    
                    rdfs:range terms:MethodOfAccrual .



###  http://purl.org/dc/terms/accrualPeriodicity

terms:accrualPeriodicity rdf:type owl:ObjectProperty ;
                         
                         rdfs:domain <http://purl.org/dc/dcmitype/Collection> ;
                         
                         rdfs:range terms:Frequency .



###  http://purl.org/dc/terms/accrualPolicy

terms:accrualPolicy rdf:type owl:ObjectProperty ;
                    
                    rdfs:domain <http://purl.org/dc/dcmitype/Collection> ;
                    
                    rdfs:range terms:Policy .



###  http://purl.org/dc/terms/audience

terms:audience rdf:type owl:ObjectProperty ;
               
               rdfs:range terms:AgentClass .



###  http://purl.org/dc/terms/conformsTo

terms:conformsTo rdf:type owl:ObjectProperty ;
                 
                 rdfs:range terms:Standard .



###  http://purl.org/dc/terms/contributor

terms:contributor rdf:type owl:ObjectProperty ;
                  
                  rdfs:range terms:Agent .



###  http://purl.org/dc/terms/coverage

terms:coverage rdf:type owl:ObjectProperty ;
               
               rdfs:range terms:LocationPeriodOrJurisdiction .



###  http://purl.org/dc/terms/creator

terms:creator rdf:type owl:ObjectProperty ;
              
              rdfs:range terms:Agent ;
              
              rdfs:subPropertyOf terms:contributor .



###  http://purl.org/dc/terms/educationLevel

terms:educationLevel rdf:type owl:ObjectProperty ;
                     
                     rdfs:range terms:AgentClass ;
                     
                     rdfs:subPropertyOf terms:audience .



###  http://purl.org/dc/terms/extent

terms:extent rdf:type owl:ObjectProperty ;
             
             rdfs:range terms:SizeOrDuration ;
             
             rdfs:subPropertyOf terms:format .



###  http://purl.org/dc/terms/format

terms:format rdf:type owl:ObjectProperty ;
             
             rdfs:range terms:MediaTypeOrExtent .



###  http://purl.org/dc/terms/instructionalMethod

terms:instructionalMethod rdf:type owl:ObjectProperty ;
                          
                          rdfs:range terms:MethodOfInstruction .



###  http://purl.org/dc/terms/language

terms:language rdf:type owl:ObjectProperty ;
               
               rdfs:range terms:LinguisticSystem .



###  http://purl.org/dc/terms/license

terms:license rdf:type owl:ObjectProperty ;
              
              rdfs:range terms:LicenseDocument ;
              
              rdfs:subPropertyOf terms:rights .



###  http://purl.org/dc/terms/mediator

terms:mediator rdf:type owl:ObjectProperty ;
               
               rdfs:range terms:AgentClass ;
               
               rdfs:subPropertyOf terms:audience .



###  http://purl.org/dc/terms/medium

terms:medium rdf:type owl:ObjectProperty ;
             
             rdfs:range terms:PhysicalMedium ;
             
             rdfs:domain terms:PhysicalResource ;
             
             rdfs:subPropertyOf terms:format .



###  http://purl.org/dc/terms/provenance

terms:provenance rdf:type owl:ObjectProperty ;
                 
                 rdfs:range terms:ProvenanceStatement .



###  http://purl.org/dc/terms/publisher

terms:publisher rdf:type owl:ObjectProperty ;
                
                rdfs:range terms:Agent .



###  http://purl.org/dc/terms/rights

terms:rights rdf:type owl:ObjectProperty ;
             
             rdfs:range terms:RightsStatement .



###  http://purl.org/dc/terms/rightsHolder

terms:rightsHolder rdf:type owl:ObjectProperty ;
                   
                   rdfs:range terms:Agent .



###  http://purl.org/dc/terms/spatial

terms:spatial rdf:type owl:ObjectProperty ;
              
              rdfs:range terms:Location ;
              
              rdfs:subPropertyOf terms:coverage .



###  http://purl.org/dc/terms/temporal

terms:temporal rdf:type owl:ObjectProperty ;
               
               rdfs:range terms:PeriodOfTime ;
               
               rdfs:subPropertyOf terms:coverage .



###  http://purl.org/dc/terms/type

terms:type rdf:type owl:ObjectProperty ;
           
           rdfs:range rdfs:Class .





#################################################################
#
#    Data properties
#
#################################################################


###  http://data.finance.gov.au/def/agrif#atTime

:atTime rdf:type owl:DatatypeProperty ;
        
        dc:source "https://www.w3.org/TR/prov-o/#atTime" ;
        
        rdfs:comment "The time at which an Event occurred, in the form of xsd:dateTime."@en ;
        
        rdfs:range xsd:dateTime .



###  http://data.finance.gov.au/def/agrif#checksum

:checksum rdf:type owl:DatatypeProperty ;
          
          dc:source "A checksum is a small-sized datum derived from a block of digital data representing a Record for the purpose of detecting errors during the transfer or storage of a Record."@en ;
          
          rdfs:range xsd:float .



###  http://data.finance.gov.au/def/agrif#disposalClassNumber

:disposalClassNumber rdf:type owl:DatatypeProperty ;
                     
                     rdfs:comment "The number defining the sentencing requirements of a Record."@en ;
                     
                     rdfs:range xsd:integer .



###  http://data.finance.gov.au/def/agrif#endedAtTime

:endedAtTime rdf:type owl:DatatypeProperty ;
             
             rdfs:comment "The time at which an Activity ended."@en ;
             
             dc:source "https://www.w3.org/TR/prov-o/#endedAtTime" ;
             
             rdfs:range xsd:dateTime .



###  http://data.finance.gov.au/def/agrif#filename

:filename rdf:type owl:DatatypeProperty ;
          
          rdfs:comment "A filename is a name used to uniquely identify a computer file stored in a file system." .



###  http://data.finance.gov.au/def/agrif#filesize

:filesize rdf:type owl:DatatypeProperty ;
          
          rdfs:comment "File size is a measure of how much data a computer file contains or how much storage it consumes."@en .



###  http://data.finance.gov.au/def/agrif#format

:format rdf:type owl:DatatypeProperty ;
        
        rdfs:comment "The file format, physical medium, or dimensions of the resource."@en ;
        
        dc:source "http://purl.org/dc/elements/1.1/format" .



###  http://data.finance.gov.au/def/agrif#seriesNumber

:seriesNumber rdf:type owl:DatatypeProperty ;
              
              rdfs:comment "A seriesNumber is a numerical identifier for a Series."@en ;
              
              rdfs:range xsd:integer .



###  http://data.finance.gov.au/def/agrif#startedAtTime

:startedAtTime rdf:type owl:DatatypeProperty ;
               
               dc:source "https://www.w3.org/TR/prov-o/#startedAtTime" ;
               
               rdfs:comment "The time at which an Activity started."@en ;
               
               rdfs:range xsd:dateTime .



###  http://purl.org/dc/terms/alternative

terms:alternative rdf:type owl:DatatypeProperty ;
                  
                  rdfs:subPropertyOf terms:title ;
                  
                  rdfs:range rdfs:Literal .



###  http://purl.org/dc/terms/available

terms:available rdf:type owl:DatatypeProperty ;
                
                rdfs:subPropertyOf terms:date ;
                
                rdfs:range rdfs:Literal .



###  http://purl.org/dc/terms/bibliographicCitation

terms:bibliographicCitation rdf:type owl:DatatypeProperty ;
                            
                            rdfs:subPropertyOf terms:identifier ;
                            
                            rdfs:range rdfs:Literal .



###  http://purl.org/dc/terms/created

terms:created rdf:type owl:DatatypeProperty ;
              
              rdfs:subPropertyOf terms:date ;
              
              rdfs:range rdfs:Literal .



###  http://purl.org/dc/terms/date

terms:date rdf:type owl:DatatypeProperty ;
           
           rdfs:range rdfs:Literal .



###  http://purl.org/dc/terms/dateAccepted

terms:dateAccepted rdf:type owl:DatatypeProperty ;
                   
                   rdfs:subPropertyOf terms:date ;
                   
                   rdfs:range rdfs:Literal .



###  http://purl.org/dc/terms/dateCopyrighted

terms:dateCopyrighted rdf:type owl:DatatypeProperty ;
                      
                      rdfs:subPropertyOf terms:date ;
                      
                      rdfs:range rdfs:Literal .



###  http://purl.org/dc/terms/dateSubmitted

terms:dateSubmitted rdf:type owl:DatatypeProperty ;
                    
                    rdfs:subPropertyOf terms:date ;
                    
                    rdfs:range rdfs:Literal .



###  http://purl.org/dc/terms/identifier

terms:identifier rdf:type owl:DatatypeProperty ;
                 
                 rdfs:range rdfs:Literal .



###  http://purl.org/dc/terms/issued

terms:issued rdf:type owl:DatatypeProperty ;
             
             rdfs:subPropertyOf terms:date ;
             
             rdfs:range rdfs:Literal .



###  http://purl.org/dc/terms/modified

terms:modified rdf:type owl:DatatypeProperty ;
               
               rdfs:subPropertyOf terms:date ;
               
               rdfs:range rdfs:Literal .



###  http://purl.org/dc/terms/title

terms:title rdf:type owl:DatatypeProperty ;
            
            rdfs:range rdfs:Literal .



###  http://purl.org/dc/terms/valid

terms:valid rdf:type owl:DatatypeProperty ;
            
            rdfs:subPropertyOf terms:date ;
            
            rdfs:range rdfs:Literal .





#################################################################
#
#    Classes
#
#################################################################


###  http://data.finance.gov.au/def/agrif#AGIFTFunction

:AGIFTFunction rdf:type owl:Class ;
               
               rdfs:label "AGIFT Function"@en ;
               
               rdfs:subClassOf :Function ;
               
               rdfs:comment "An AGIFT Function is a Function that classifies a Record according to the Australian Governments' Interactive Functions Thesaurus."@en ;
               
               rdfs:isDefinedBy "https://data.naa.gov.au/def/agift/"@en .



###  http://data.finance.gov.au/def/agrif#AccessActivity

:AccessActivity rdf:type owl:Class ;
                
                rdfs:label "Access Activity"@en ;
                
                rdfs:subClassOf :Activity ,
                                [ rdf:type owl:Restriction ;
                                  owl:onProperty :triggers ;
                                  owl:someValuesFrom :AccessTrigger
                                ] ,
                                [ rdf:type owl:Restriction ;
                                  owl:onProperty :accessedBy ;
                                  owl:someValuesFrom :Agent
                                ] ;
                
                rdfs:comment "An Access Activity is an Activity where a Record is accessed by an Agent over a period of time."@en .



###  http://data.finance.gov.au/def/agrif#AccessControl

:AccessControl rdf:type owl:Class ;
               
               rdfs:label "Access Control"@en ;
               
               rdfs:subClassOf :Control ;
               
               rdfs:comment "Access Control is the selective restriction of access to a Record or Artefact."@en .



###  http://data.finance.gov.au/def/agrif#AccessTrigger

:AccessTrigger rdf:type owl:Class ;
               
               rdfs:label "Access Trigger"@en ;
               
               rdfs:subClassOf :Trigger ;
               
               rdfs:comment "An Access Trigger is a Trigger that can be initiated when a Record is accessed."@en .



###  http://data.finance.gov.au/def/agrif#Activity

:Activity rdf:type owl:Class ;
          
          rdfs:label "Activity"@en ;
          
          rdfs:subClassOf [ rdf:type owl:Restriction ;
                            owl:onProperty :startedAtTime ;
                            owl:qualifiedCardinality "1"^^xsd:nonNegativeInteger ;
                            owl:onDataRange xsd:dateTime
                          ] ,
                          [ rdf:type owl:Restriction ;
                            owl:onProperty :hasStatus ;
                            owl:allValuesFrom :Status
                          ] ,
                          [ rdf:type owl:Restriction ;
                            owl:onProperty :requiresSecurityClassification ;
                            owl:allValuesFrom :SecurityClassification
                          ] ,
                          [ rdf:type owl:Restriction ;
                            owl:onProperty :endedAtTime ;
                            owl:maxQualifiedCardinality "1"^^xsd:nonNegativeInteger ;
                            owl:onDataRange xsd:dateTime
                          ] ,
                          [ rdf:type owl:Restriction ;
                            owl:onProperty :wasAssociatedWith ;
                            owl:someValuesFrom :Agent
                          ] ,
                          [ rdf:type owl:Restriction ;
                            owl:onProperty :qualifiedAssociation ;
                            owl:someValuesFrom :Association
                          ] ,
                          [ rdf:type owl:Restriction ;
                            owl:onProperty :hasLocation ;
                            owl:allValuesFrom :SpatialLocation
                          ] ,
                          [ rdf:type owl:Restriction ;
                            owl:onProperty :usedRecord ;
                            owl:allValuesFrom :Record
                          ] ,
                          [ rdf:type owl:Restriction ;
                            owl:onProperty :associatedFunction ;
                            owl:allValuesFrom :Function
                          ] ,
                          [ rdf:type owl:Restriction ;
                            owl:onProperty :guidingPolicy ;
                            owl:allValuesFrom :Policy
                          ] ;
          
          rdfs:comment "An Activity is something that occurs over a period of time on a Record."@en ;
          
          dc:source "https://www.w3.org/TR/prov-o/#Activity" .



###  http://data.finance.gov.au/def/agrif#Administrator

:Administrator rdf:type owl:Class ;
               
               rdfs:label "Administrator"@en ;
               
               rdfs:subClassOf :Role ;
               
               rdfs:comment "An Administrator is a Role that has overall responsibility for the administration and functions of an Information System, but not necessarily for the information stored within."@en .



###  http://data.finance.gov.au/def/agrif#Agent

:Agent rdf:type owl:Class ;
       
       rdfs:label "Agent"@en ;
       
       rdfs:subClassOf [ rdf:type owl:Restriction ;
                         owl:onProperty :hasPermission ;
                         owl:someValuesFrom :Permission
                       ] ,
                       [ rdf:type owl:Restriction ;
                         owl:onProperty :positionIn ;
                         owl:someValuesFrom :Organisation
                       ] ,
                       [ rdf:type owl:Restriction ;
                         owl:onProperty :actsAs ;
                         owl:someValuesFrom :Role
                       ] ;
       
       rdfs:comment "An Agent is a corporate entity, organisational element or system, or individual responsible for the performance of some Activity or Event, including those on Records."@en ;
       
       dc:source "https://www.w3.org/TR/prov-o/#Agent" .



###  http://data.finance.gov.au/def/agrif#Artefact

:Artefact rdf:type owl:Class ;
          
          rdfs:label "Artefact"@en ;
          
          rdfs:subClassOf [ rdf:type owl:Restriction ;
                            owl:onProperty :isChangedBy ;
                            owl:someValuesFrom :Event
                          ] ,
                          [ rdf:type owl:Restriction ;
                            owl:onProperty :relatedTo ;
                            owl:someValuesFrom :Artefact
                          ] ,
                          [ rdf:type owl:Restriction ;
                            owl:onProperty :storedIn ;
                            owl:someValuesFrom :ControlledVocabulary
                          ] ,
                          [ rdf:type owl:Restriction ;
                            owl:onProperty :hasControl ;
                            owl:someValuesFrom :Control
                          ] ,
                          [ rdf:type owl:Restriction ;
                            owl:onProperty :hasLocation ;
                            owl:allValuesFrom :SpatialLocation
                          ] ,
                          [ rdf:type owl:Restriction ;
                            owl:onProperty :hasQuality ;
                            owl:someValuesFrom :PreservationQuality
                          ] ;
          
          rdfs:comment "An Artefact is an object that is made by a Person and that is to be preserved."@en .



###  http://data.finance.gov.au/def/agrif#Association

:Association rdf:type owl:Class ;
             
             rdfs:label "Association"@en ;
             
             rdfs:subClassOf [ rdf:type owl:Restriction ;
                               owl:onProperty :hasAgent ;
                               owl:allValuesFrom :Agent
                             ] ,
                             [ rdf:type owl:Restriction ;
                               owl:onProperty :associatedRole ;
                               owl:allValuesFrom :Role
                             ] ;
             
             rdfs:comment "An Association is a qualified assignment of responsibility to an Agent in an Activity or Event, indicating that the Agent had a Role in the Activity."@en ;
             
             dc:source "https://www.w3.org/TR/prov-o/#Association" .



###  http://data.finance.gov.au/def/agrif#AuditEvent

:AuditEvent rdf:type owl:Class ;
            
            rdfs:label "Audit Event"@en ;
            
            rdfs:subClassOf :ControlEvent ;
            
            rdfs:comment "An Audit Event is the systematic examination of a Record to ascertain how and where the Record is stored, who created it, or manages it, who uses it and how much longer the Record is required to be maintained."@en .



###  http://data.finance.gov.au/def/agrif#BusinessOwner

:BusinessOwner rdf:type owl:Class ;
               
               rdfs:label "Business Owner"@en ;
               
               rdfs:subClassOf :Role ;
               
               rdfs:comment "A Business Owner is the Role that has the managerial control of a Function."@en .



###  http://data.finance.gov.au/def/agrif#Classifier

:Classifier rdf:type owl:Class ;
            
            rdfs:label "Classifier"@en ;
            
            rdfs:subClassOf [ rdf:type owl:Restriction ;
                              owl:onProperty :associatedFunction ;
                              owl:allValuesFrom :Function
                            ] ;
            
            rdfs:comment "A Classifier is a machine-generated and applied category that a set of Records belong to."@en .



###  http://data.finance.gov.au/def/agrif#Control

:Control rdf:type owl:Class ;
         
         rdfs:label "Control"@en ;
         
         rdfs:comment "A Control is a security or access measure that safeguards or restricts access to an asset."@en .



###  http://data.finance.gov.au/def/agrif#ControlEvent

:ControlEvent rdf:type owl:Class ;
              
              rdfs:label "Control Event"@en ;
              
              rdfs:subClassOf :Event ,
                              [ rdf:type owl:Restriction ;
                                owl:onProperty :hasControl ;
                                owl:someValuesFrom :Control
                              ] ;
              
              rdfs:comment "A Control Event is an Event that requires a particular level of access to the Record."@en .



###  http://data.finance.gov.au/def/agrif#ControlledVocabulary

:ControlledVocabulary rdf:type owl:Class ;
                      
                      rdfs:label "Controlled Vocabulary"@en ;
                      
                      rdfs:subClassOf :IntellectualControlSystem ,
                                      [ rdf:type owl:Restriction ;
                                        owl:onProperty :associatedFunction ;
                                        owl:onClass :Function ;
                                        owl:minQualifiedCardinality "1"^^xsd:nonNegativeInteger
                                      ] ;
                      
                      rdfs:seeAlso "http://www.w3.org/2004/02/skos/core#ConceptScheme" ;
                      
                      rdfs:comment "A Controlled Vocabulary is an Intellectual Control System that provides a way to organize Records that facilitates a later discovery of a Record."@en .



###  http://data.finance.gov.au/def/agrif#Coverage

:Coverage rdf:type owl:Class ;
          
          rdfs:label "Coverage"@en ;
          
          rdfs:comment "A Coverage denotes the jurisdictional applicability, or the temporal and/or spatial extent to which a Record is observed."@en .



###  http://data.finance.gov.au/def/agrif#CreationEvent

:CreationEvent rdf:type owl:Class ;
               
               rdfs:label "Creation Event"@en ;
               
               rdfs:subClassOf :Event ;
               
               rdfs:comment "A Creation Event is a Change Event that results in the creation of a Record."@en .



###  http://data.finance.gov.au/def/agrif#Creator

:Creator rdf:type owl:Class ;
         
         rdfs:label "Creator"@en ;
         
         rdfs:subClassOf :Role ;
         
         rdfs:comment "A Creator is the Agent that has created a Record or Artefact."@en .



###  http://data.finance.gov.au/def/agrif#DecisionEvent

:DecisionEvent rdf:type owl:Class ;
               
               rdfs:label "Decision Event"@en ;
               
               rdfs:subClassOf :ControlEvent ,
                               [ rdf:type owl:Restriction ;
                                 owl:onProperty :hasDecisionStatus ;
                                 owl:someValuesFrom :DecisionStatus
                               ] ,
                               [ rdf:type owl:Restriction ;
                                 owl:onProperty :hasPrerequisiteDecisionEvent ;
                                 owl:someValuesFrom :DecisionEvent
                               ] ;
               
               rdfs:comment "A Decision Event changes the Decision Status on the Control of a Record."@en .



###  http://data.finance.gov.au/def/agrif#DecisionStatus

:DecisionStatus rdf:type owl:Class ;
                
                rdfs:label "Decision Status"@en ;
                
                rdfs:subClassOf :Status ;
                
                rdfs:comment "A Decision Status is a Status that indicates the approval or disapproval of a Decision Event."@en .



###  http://data.finance.gov.au/def/agrif#DestroyEvent

:DestroyEvent rdf:type owl:Class ;
              
              rdfs:label "Destroy Event"@en ;
              
              rdfs:subClassOf :DisposalEvent ;
              
              rdfs:comment "A Destroy Event is a Disposal Event that results in the regular authorised permanent desctruction of a Record that is no longer required for business purposes."@en .



###  http://data.finance.gov.au/def/agrif#DigitalArtefact

:DigitalArtefact rdf:type owl:Class ;
                 
                 rdfs:label "Digital Artefact"@en ;
                 
                 rdfs:subClassOf :Artefact ,
                                 [ rdf:type owl:Restriction ;
                                   owl:onProperty :format ;
                                   owl:someValuesFrom rdfs:Literal
                                 ] ,
                                 [ rdf:type owl:Restriction ;
                                   owl:onProperty :storedIn ;
                                   owl:someValuesFrom :InformationSystem
                                 ] ,
                                 [ rdf:type owl:Restriction ;
                                   owl:onProperty :filename ;
                                   owl:someValuesFrom rdfs:Literal
                                 ] ,
                                 [ rdf:type owl:Restriction ;
                                   owl:onProperty :filesize ;
                                   owl:someValuesFrom xsd:long
                                 ] ;
                 
                 rdfs:comment "A Digital Artefact is an Artefact that is of a digital nature and stored in an Information System."@en .



###  http://data.finance.gov.au/def/agrif#DigitalHoldingSpace

:DigitalHoldingSpace rdf:type owl:Class ;
                     
                     rdfs:label "Digital Holding Space"@en ;
                     
                     rdfs:subClassOf :HoldingSpace ;
                     
                     rdfs:comment "A Digital Holding Space is a space that is used or reserved for the storage of a Digital Artefact on a storage medium or virtual storage space."@en .



###  http://data.finance.gov.au/def/agrif#DigitalPreservationPolicy

:DigitalPreservationPolicy rdf:type owl:Class ;
                           
                           rdfs:label "Digital Preservation Policy"@en ;
                           
                           rdfs:subClassOf :Policy ;
                           
                           rdfs:comment "The Digital Preservation Policy defines the process of active management by which the National Archives ensures that a digital object will be accessible in the future."@en .



###  http://data.finance.gov.au/def/agrif#DisposalClass

:DisposalClass rdf:type owl:Class ;
               
               rdfs:label "Disposal Class"@en ;
               
               rdfs:subClassOf :RecordsAuthorityPolicy ,
                               [ rdf:type owl:Restriction ;
                                 owl:onProperty :disposalClassNumber ;
                                 owl:qualifiedCardinality "1"^^xsd:nonNegativeInteger ;
                                 owl:onDataRange xsd:integer
                               ] ;
               
               rdfs:comment "A Disposal Class is a Policy that defines the sentencing requirements of an item."@en .



###  http://data.finance.gov.au/def/agrif#DisposalEvent

:DisposalEvent rdf:type owl:Class ;
               
               rdfs:label "Disposal Event"@en ;
               
               rdfs:subClassOf :ControlEvent ;
               
               rdfs:comment "A Disposal Event is an Event that results in the regular authorised destruction or change of custody of a Record that is no longer required for business purposes."@en .



###  http://data.finance.gov.au/def/agrif#Event

:Event rdf:type owl:Class ;
       
       rdfs:label "Event"@en ;
       
       rdfs:subClassOf [ rdf:type owl:Restriction ;
                         owl:onProperty :wasAssociatedWith ;
                         owl:someValuesFrom :Agent
                       ] ,
                       [ rdf:type owl:Restriction ;
                         owl:onProperty :hasStatus ;
                         owl:allValuesFrom :Status
                       ] ,
                       [ rdf:type owl:Restriction ;
                         owl:onProperty :guidingPolicy ;
                         owl:allValuesFrom :Policy
                       ] ,
                       [ rdf:type owl:Restriction ;
                         owl:onProperty :associatedFunction ;
                         owl:allValuesFrom :Function
                       ] ,
                       [ rdf:type owl:Restriction ;
                         owl:onProperty :qualifiedAssociation ;
                         owl:someValuesFrom :Association
                       ] ,
                       [ rdf:type owl:Restriction ;
                         owl:onProperty :atTime ;
                         owl:qualifiedCardinality "1"^^xsd:nonNegativeInteger ;
                         owl:onDataRange xsd:dateTime
                       ] ,
                       [ rdf:type owl:Restriction ;
                         owl:onProperty :triggeredBy ;
                         owl:allValuesFrom :Trigger
                       ] ;
       
       dc:source "https://www.w3.org/TR/prov-o/#InstantaneousEvent" ;
       
       rdfs:comment "An Event denotes an instantaneous transition in the world."@en .



###  http://data.finance.gov.au/def/agrif#FormFactor

:FormFactor rdf:type owl:Class ;
            
            rdfs:label "Form Factor"@en ;
            
            rdfs:comment "A Form Factor defines and prescribes the size, shape, and other physical specifications of a Physical Artefact that is stored."@en .



###  http://data.finance.gov.au/def/agrif#FreezeEvent

:FreezeEvent rdf:type owl:Class ;
             
             rdfs:label "Freeze Event"@en ;
             
             rdfs:subClassOf :DisposalEvent ;
             
             rdfs:comment "A Freeze Event is a Disposal Event that leads to a records disposal freeze or retention notice in support of compliance requirements or an identified need to suspend the Archives' records destruction permissions."@en .



###  http://data.finance.gov.au/def/agrif#Function

:Function rdf:type owl:Class ;
          
          rdfs:label "Function"@en ;
          
          rdfs:subClassOf [ rdf:type owl:Restriction ;
                            owl:onProperty :guidingPolicy ;
                            owl:allValuesFrom :Policy
                          ] ;
          
          rdfs:comment "A Function is a process that is performed routinely to carry out a part of the mandate of an Australian Government Agency."@en ,
                       "A Function reflects the responsibilities of an Organisation that can be delegated through official channels. [Commonwealth Records Series Manual]"@en .



###  http://data.finance.gov.au/def/agrif#HoldingSpace

:HoldingSpace rdf:type owl:Class ;
              
              rdfs:label "Holding Space"@en ;
              
              rdfs:subClassOf :SpatialLocation ;
              
              rdfs:comment "A Holding Space is a space that is used or reserved for the storage of an Artefact."@en .



###  http://data.finance.gov.au/def/agrif#InformationManagementPolicy

:InformationManagementPolicy rdf:type owl:Class ;
                             
                             rdfs:label "Information Management Policy"@en ;
                             
                             rdfs:subClassOf :Policy ,
                                             [ rdf:type owl:Restriction ;
                                               owl:onProperty :hasDisposalClass ;
                                               owl:allValuesFrom :DisposalClass
                                             ] ;
                             
                             rdfs:comment "An Information Management Policy is a Policy that helps to align information management practices to fulfill the requirements of an information governance framework. An Information Management Policy provides direction and guidance to staff for creating, capturing and managing information to satisfy business, legal and stakeholder requirements, and assigns responsibilities across the agency."@en .



###  http://data.finance.gov.au/def/agrif#InformationSystem

:InformationSystem rdf:type owl:Class ;
                   
                   rdfs:label "Information System"@en ;
                   
                   rdfs:comment "An Information System is an organized system for the collection, organization, storage and communication of information, typically Digital Artefacts or Records."@en .



###  http://data.finance.gov.au/def/agrif#IntellectualControlSystem

:IntellectualControlSystem rdf:type owl:Class ;
                           
                           rdfs:label "Intellectual Control System"@en ;
                           
                           rdfs:subClassOf :InformationSystem ,
                                           [ rdf:type owl:Restriction ;
                                             owl:onProperty :guidingPolicy ;
                                             owl:allValuesFrom :Policy
                                           ] ;
                           
                           rdfs:comment "An Intellectual Control System is a System that enables Agents to locate and manage information."@en .



###  http://data.finance.gov.au/def/agrif#JurisdictionalCoverage

:JurisdictionalCoverage rdf:type owl:Class ;
                        
                        rdfs:label "Jurisdictional Coverage"@en ;
                        
                        rdfs:subClassOf :Coverage ;
                        
                        rdfs:seeAlso "http://purl.org/dc/terms/Jurisdiction" ;
                        
                        rdfs:comment "A Jurisdictional Coverage denotes the jurisdictional applicability of the Record."@en .



###  http://data.finance.gov.au/def/agrif#MaintainActivity

:MaintainActivity rdf:type owl:Class ;
                  
                  rdfs:label "Maintain Activity"@en ;
                  
                  rdfs:subClassOf :Activity ,
                                  [ rdf:type owl:Restriction ;
                                    owl:onProperty :hasQuality ;
                                    owl:someValuesFrom :PreservationQuality
                                  ] ;
                  
                  rdfs:comment "A Maintain Activity is an Activity to maintain a Record over a period of time due to a BusinessFunction or Policy."@en .



###  http://data.finance.gov.au/def/agrif#Manifest

:Manifest rdf:type owl:Class ;
          
          rdfs:label "Manifest"@en ;
          
          rdfs:subClassOf [ rdf:type owl:Restriction ;
                            owl:onProperty :checksum ;
                            owl:qualifiedCardinality "1"^^xsd:nonNegativeInteger ;
                            owl:onDataRange xsd:float
                          ] ;
          
          rdfs:comment "A Manifest describes the files involved in the transfer of a Record from an Agency to the National Archives, including details such as the filesize, the destination hierarchy and the file's metadata."@en .



###  http://data.finance.gov.au/def/agrif#MinimumMetadataSetPolicy

:MinimumMetadataSetPolicy rdf:type owl:Class ;
                          
                          rdfs:label "Minimum Metadata Set Policy"@en ;
                          
                          rdfs:subClassOf :Policy ;
                          
                          rdfs:comment "The Minimum Metadata Set Policy is a Policy that has been developed by the National Archives of Australia to identify metadata properties essential for agency management of information as well as those needed for records which will be transferred to the Archives. It supports the Digital Continuity 2020 principles of interoperable systems and processes and is a practical application of the Australian Government Recordkeeping Metadata Standard 2.2 (AGRkMS) to support metadata implementation and information use in agencies."@en .



###  http://data.finance.gov.au/def/agrif#Organisation

:Organisation rdf:type owl:Class ;
              
              rdfs:label "Organisation"@en ;
              
              rdfs:subClassOf :Agent ,
                              [ rdf:type owl:Restriction ;
                                owl:onProperty :associatedFunction ;
                                owl:someValuesFrom :Function
                              ] ;
              
              rdfs:comment "An Organisation is a type of Agent that denotes a social or legal institution such as a government agency, a corporation, society, etc."@en ;
              
              dc:source "https://www.w3.org/TR/prov-o/#Organization" .



###  http://data.finance.gov.au/def/agrif#OrganisationalUnit

:OrganisationalUnit rdf:type owl:Class ;
                    
                    rdfs:label "Organisational Unit"@en ;
                    
                    rdfs:subClassOf :Organisation ,
                                    [ rdf:type owl:Restriction ;
                                      owl:onProperty :partOf ;
                                      owl:someValuesFrom :Organisation
                                    ] ;
                    
                    rdfs:comment "An Organisational Unit is a division of labour typically organised around a business function that form part of the Organisation."@en .



###  http://data.finance.gov.au/def/agrif#Permission

:Permission rdf:type owl:Class ;
            
            rdfs:label "Permission"@en ;
            
            rdfs:comment "A Permission denotes the Security Clearance of an Agent that determines its access and use rights to Records."@en ;
            
            dc:source "Australian Government Recordkeeping Metadata Standard"@en .



###  http://data.finance.gov.au/def/agrif#Person

:Person rdf:type owl:Class ;
        
        rdfs:label "Person"@en ;
        
        rdfs:subClassOf :Agent ;
        
        dc:source "https://www.w3.org/TR/prov-o/#Person" ;
        
        rdfs:comment "A Person is an Agent that denotes a human."@en .



###  http://data.finance.gov.au/def/agrif#PhysicalArtefact

:PhysicalArtefact rdf:type owl:Class ;
                  
                  rdfs:label "Physical Artefact"@en ;
                  
                  rdfs:subClassOf :Artefact ,
                                  [ rdf:type owl:Restriction ;
                                    owl:onProperty :hasFormFactor ;
                                    owl:someValuesFrom :FormFactor
                                  ] ;
                  
                  rdfs:comment "A Physical Artefact is an Artefact that is of physical nature."@en ;
                  
                  skos:example "An example of a Phyiscal Artefact in the context of record keeping is information printed or written on paper."@en .



###  http://data.finance.gov.au/def/agrif#PhysicalHoldingSpace

:PhysicalHoldingSpace rdf:type owl:Class ;
                      
                      rdfs:label "Physical Holding Space"@en ;
                      
                      rdfs:subClassOf :HoldingSpace ;
                      
                      rdfs:comment "A Physical Holding Space is a Spatial Location that is used or reserved for the storage of a Physical Artefact."@en .



###  http://data.finance.gov.au/def/agrif#Policy

:Policy rdf:type owl:Class ;
        
        rdfs:label "Policy"@en ;
        
        dc:source "http://purl.org/dc/terms/Policy" ;
        
        rdfs:comment "A Policy is a deliberate system of principles to guide decisions and achieve rational outcomes."@en .



###  http://data.finance.gov.au/def/agrif#PreservationQuality

:PreservationQuality rdf:type owl:Class ;
                     
                     rdfs:label "Preservation Quality"@en ;
                     
                     rdfs:subClassOf :Quality ;
                     
                     rdfs:comment "A Preservation Quality describes a Quality of an Artefact that supports or threatens the long term preservation of the information that is to be preserved."@en .



###  http://data.finance.gov.au/def/agrif#Quality

:Quality rdf:type owl:Class ;
         
         rdfs:label "Quality"@en ;
         
         rdfs:comment "A Quality is an attribute that is intrinsically associated with an entity."@en .



###  http://data.finance.gov.au/def/agrif#Record

:Record rdf:type owl:Class ;
        
        rdfs:label "Record"@en ;
        
        rdfs:subClassOf [ rdf:type owl:Restriction ;
                          owl:onProperty :hasStatus ;
                          owl:allValuesFrom :Status
                        ] ,
                        [ rdf:type owl:Restriction ;
                          owl:onProperty :replaces ;
                          owl:allValuesFrom :Record
                        ] ,
                        [ rdf:type owl:Restriction ;
                          owl:onProperty :hasControl ;
                          owl:someValuesFrom :Control
                        ] ,
                        [ rdf:type owl:Restriction ;
                          owl:onProperty :qualifiedAssociation ;
                          owl:someValuesFrom :Association
                        ] ,
                        [ rdf:type owl:Restriction ;
                          owl:onProperty :hasCoverage ;
                          owl:allValuesFrom :Coverage
                        ] ,
                        [ rdf:type owl:Restriction ;
                          owl:onProperty :checksum ;
                          owl:maxQualifiedCardinality "1"^^xsd:nonNegativeInteger ;
                          owl:onDataRange xsd:float
                        ] ,
                        [ rdf:type owl:Restriction ;
                          owl:onProperty :relatedTo ;
                          owl:someValuesFrom :Record
                        ] ,
                        [ rdf:type owl:Restriction ;
                          owl:onProperty :recordOf ;
                          owl:onClass :Artefact ;
                          owl:minQualifiedCardinality "1"^^xsd:nonNegativeInteger
                        ] ,
                        [ rdf:type owl:Restriction ;
                          owl:onProperty :requiresSecurityClassification ;
                          owl:allValuesFrom :SecurityClassification
                        ] ,
                        [ rdf:type owl:Restriction ;
                          owl:onProperty :hasDisposalClass ;
                          owl:onClass :DisposalClass ;
                          owl:qualifiedCardinality "1"^^xsd:nonNegativeInteger
                        ] ,
                        [ rdf:type owl:Restriction ;
                          owl:onProperty :isChangedBy ;
                          owl:onClass :CreationEvent ;
                          owl:qualifiedCardinality "1"^^xsd:nonNegativeInteger
                        ] ,
                        [ rdf:type owl:Restriction ;
                          owl:onProperty :associatedFunction ;
                          owl:onClass :Function ;
                          owl:minQualifiedCardinality "1"^^xsd:nonNegativeInteger
                        ] ,
                        [ rdf:type owl:Restriction ;
                          owl:onProperty :isChangedBy ;
                          owl:allValuesFrom :Event
                        ] ,
                        [ rdf:type owl:Restriction ;
                          owl:onProperty :hasSeries ;
                          owl:allValuesFrom :Series
                        ] ,
                        [ rdf:type owl:Restriction ;
                          owl:onProperty :hasActivity ;
                          owl:allValuesFrom :Activity
                        ] ,
                        [ rdf:type owl:Restriction ;
                          owl:onProperty :hasClassifier ;
                          owl:someValuesFrom :Classifier
                        ] ;
        
        rdfs:comment "A Record is information in any format created, received and maintained as evidence by an Organisation or Person, in pursuance of legal obligations or in the transaction of business. A Record may comprise a Digital or Physical Artefact."@en .



###  http://data.finance.gov.au/def/agrif#RecordStorageStandard

:RecordStorageStandard rdf:type owl:Class ;
                       
                       rdfs:label "Record Storage Standard"@en ;
                       
                       rdfs:subClassOf :Policy ;
                       
                       rdfs:comment "The Standard for the storage of non-digital archival Records is designed to set out the requirements for the safe storage and preservation of non-digital records in the Archives’ custody; to ensure all non-digital records are protected, secure and accessible for as long as they are required to meet business and accountability needs and community expectations; and to ensure all non-digital records are stored in the most cost-effective manner possible."@en .



###  http://data.finance.gov.au/def/agrif#RecordsAuthorityFunction

:RecordsAuthorityFunction rdf:type owl:Class ;
                          
                          rdfs:label "Records Authority Function"@en ;
                          
                          rdfs:subClassOf :Function ;
                          
                          rdfs:comment "A Records Authority Function is a Function that is assigned by the National Archives to classify Agency business."@en .



###  http://data.finance.gov.au/def/agrif#RecordsAuthorityPolicy

:RecordsAuthorityPolicy rdf:type owl:Class ;
                        
                        rdfs:label "Records Authority Disposal Class Policy"@en ;
                        
                        rdfs:subClassOf :Policy ,
                                        [ rdf:type owl:Restriction ;
                                          owl:onProperty :hasDisposalClass ;
                                          owl:allValuesFrom :DisposalClass
                                        ] ;
                        
                        rdfs:comment "A Records Authority Disposal Class Policy is a Policy that identifies the specific disposal class that authorises the retention or destruction of a Record."@en ;
                        
                        dc:source "Australian Government Recordkeeping Metadata Standard"@en .



###  http://data.finance.gov.au/def/agrif#ReplaceEvent

:ReplaceEvent rdf:type owl:Class ;
              
              rdfs:label "Replace Event"@en ;
              
              rdfs:subClassOf :ControlEvent ,
                              [ rdf:type owl:Restriction ;
                                owl:onProperty :hasVersionHistory ;
                                owl:someValuesFrom :VersionHistory
                              ] ,
                              [ rdf:type owl:Restriction ;
                                owl:onProperty :replacedBy ;
                                owl:onClass :Record ;
                                owl:qualifiedCardinality "1"^^xsd:nonNegativeInteger
                              ] ;
              
              rdfs:comment "A Replace Event is an Event that results in the replacement of a Record with a new version. Edits to a Record constitute a Replace Event."@en .



###  http://data.finance.gov.au/def/agrif#Role

:Role rdf:type owl:Class ;
      
      rdfs:label "Role"@en ;
      
      rdfs:subClassOf [ rdf:type owl:Restriction ;
                        owl:onProperty :hasPermission ;
                        owl:someValuesFrom :Permission
                      ] ;
      
      dc:source "https://www.w3.org/TR/prov-o/#Role" ;
      
      rdfs:comment "A Role is the function of an entity or agent with respect to an Activity or Event, in the context of a usage, generation, invalidation, association, start, and end."@en .



###  http://data.finance.gov.au/def/agrif#SecurityClassification

:SecurityClassification rdf:type owl:Class ;
                        
                        rdfs:label "Security Classification"@en ;
                        
                        rdfs:subClassOf :AccessControl ;
                        
                        rdfs:comment "A Security Classification denotes the security status of a Record that an Agent needs to possess to access the Record."@en ;
                        
                        dc:source "Australian Government Recordkeeping Metadata Standard"@en .



###  http://data.finance.gov.au/def/agrif#SecurityControl

:SecurityControl rdf:type owl:Class ;
                 
                 rdfs:label "Security Control"@en ;
                 
                 rdfs:subClassOf :Control ;
                 
                 rdfs:comment "A Security Control is a safeguard or countermeasures to avoid, detect, counteract, or minimize security risks to a Record or Artefact."@en .



###  http://data.finance.gov.au/def/agrif#SentencingEvent

:SentencingEvent rdf:type owl:Class ;
                 
                 rdfs:label "Sentencing Event"@en ;
                 
                 rdfs:subClassOf :ControlEvent ;
                 
                 rdfs:comment "A Sentencing Event is an Event that classifies an Agencies Record to a specific class of a Records Authority Policy. This helps determine the Records value and how it should be managed throughout its lifecycle."@en .



###  http://data.finance.gov.au/def/agrif#Series

:Series rdf:type owl:Class ;
        
        rdfs:label "Series"@en ;
        
        rdfs:subClassOf :IntellectualControlSystem ,
                        [ rdf:type owl:Restriction ;
                          owl:onProperty :associatedFunction ;
                          owl:allValuesFrom :Function
                        ] ;
        
        rdfs:comment "A Series is an identifier for an item, and when combined with a control symbol gives an item its intellectual context."@en .



###  http://data.finance.gov.au/def/agrif#ShareActivity

:ShareActivity rdf:type owl:Class ;
               
               rdfs:label "Share Activity"@en ;
               
               rdfs:subClassOf :Activity ,
                               [ rdf:type owl:Restriction ;
                                 owl:onProperty :sharedWith ;
                                 owl:someValuesFrom :Agent
                               ] ;
               
               rdfs:comment "A Share Activity is an Activity where the custodianship of a Record is transferred to or shared with Agents over a period of time."@en .



###  http://data.finance.gov.au/def/agrif#SpatialCoverage

:SpatialCoverage rdf:type owl:Class ;
                 
                 rdfs:label "Spatial Coverage"@en ;
                 
                 rdfs:subClassOf :Coverage ;
                 
                 rdfs:comment "A Spatial Coverage denotes the spatial extent to which a Record is observed."@en ;
                 
                 rdfs:seeAlso "http://purl.org/dc/terms/spatial" .



###  http://data.finance.gov.au/def/agrif#SpatialLocation

:SpatialLocation rdf:type owl:Class ;
                 
                 rdfs:label "Spatial Location"@en ;
                 
                 rdfs:comment "A Spatial Location describes where a something (e.g. a Record, Collection or Artefact) is physically located, using geospatial coordinates such as latitude and longitude."@en .



###  http://data.finance.gov.au/def/agrif#Status

:Status rdf:type owl:Class ;
        
        rdfs:label "Status"@en ;
        
        rdfs:comment "A Status indicates an Activities current state."@en .



###  http://data.finance.gov.au/def/agrif#TemporalCoverage

:TemporalCoverage rdf:type owl:Class ;
                  
                  rdfs:label "Temporal Coverage"@en ;
                  
                  rdfs:subClassOf :Coverage ;
                  
                  rdfs:comment "A Temporal Coverage denotes the temporal extent to which a Record is observed."@en ;
                  
                  rdfs:seeAlso "http://purl.org/dc/terms/temporal" .



###  http://data.finance.gov.au/def/agrif#TransferEvent

:TransferEvent rdf:type owl:Class ;
               
               rdfs:label "Transfer Event"@en ;
               
               rdfs:subClassOf :DisposalEvent ,
                               [ rdf:type owl:Restriction ;
                                 owl:onProperty :transferredTo ;
                                 owl:someValuesFrom :Role
                               ] ,
                               [ rdf:type owl:Restriction ;
                                 owl:onProperty :transferredTo ;
                                 owl:someValuesFrom :BusinessOwner
                               ] ,
                               [ rdf:type owl:Restriction ;
                                 owl:onProperty :hasManifest ;
                                 owl:someValuesFrom :Manifest
                               ] ,
                               [ rdf:type owl:Restriction ;
                                 owl:onProperty :transferredFrom ;
                                 owl:someValuesFrom :BusinessOwner
                               ] ,
                               [ rdf:type owl:Restriction ;
                                 owl:onProperty :transferredFrom ;
                                 owl:someValuesFrom :Role
                               ] ;
               
               rdfs:comment "A Transfer Event is a Disposal Event that results in a change of custody."@en ;
               
               skos:example "An example of a Transfer Event is the transfer of a Record from an Agency to the National Archives. Section 27 of the Archives Act 1983 requires Australian government agencies to transfer Records to the Archives within 15 years of their creation."@en .



###  http://data.finance.gov.au/def/agrif#Trigger

:Trigger rdf:type owl:Class ;
         
         rdfs:label "Trigger"@en ;
         
         rdfs:subClassOf [ rdf:type owl:Restriction ;
                           owl:onProperty :notifies ;
                           owl:someValuesFrom :Agent
                         ] ;
         
         rdfs:comment "A Trigger is an entity that initiated an Activity or Event."@en .



###  http://data.finance.gov.au/def/agrif#User

:User rdf:type owl:Class ;
      
      rdfs:label "User"@en ;
      
      rdfs:subClassOf :Role ;
      
      rdfs:comment "A User is an Agent that uses a Record."@en .



###  http://data.finance.gov.au/def/agrif#VersionHistory

:VersionHistory rdf:type owl:Class ;
                
                rdfs:label "Version History"@en ;
                
                rdfs:comment "A Version History is the cumulative change to a previous version of a file."@en .



###  http://purl.org/dc/dcam/VocabularyEncodingScheme

<http://purl.org/dc/dcam/VocabularyEncodingScheme> rdf:type owl:Class .



###  http://purl.org/dc/dcmitype/Collection

<http://purl.org/dc/dcmitype/Collection> rdf:type owl:Class .



###  http://purl.org/dc/terms/Agent

terms:Agent rdf:type owl:Class .



###  http://purl.org/dc/terms/AgentClass

terms:AgentClass rdf:type owl:Class ;
                 
                 rdfs:subClassOf rdfs:Class .



###  http://purl.org/dc/terms/BibliographicResource

terms:BibliographicResource rdf:type owl:Class .



###  http://purl.org/dc/terms/FileFormat

terms:FileFormat rdf:type owl:Class ;
                 
                 rdfs:subClassOf terms:MediaType .



###  http://purl.org/dc/terms/Frequency

terms:Frequency rdf:type owl:Class .



###  http://purl.org/dc/terms/Jurisdiction

terms:Jurisdiction rdf:type owl:Class ;
                   
                   rdfs:subClassOf terms:LocationPeriodOrJurisdiction .



###  http://purl.org/dc/terms/LicenseDocument

terms:LicenseDocument rdf:type owl:Class ;
                      
                      rdfs:subClassOf terms:RightsStatement .



###  http://purl.org/dc/terms/LinguisticSystem

terms:LinguisticSystem rdf:type owl:Class .



###  http://purl.org/dc/terms/Location

terms:Location rdf:type owl:Class ;
               
               rdfs:subClassOf terms:LocationPeriodOrJurisdiction .



###  http://purl.org/dc/terms/LocationPeriodOrJurisdiction

terms:LocationPeriodOrJurisdiction rdf:type owl:Class .



###  http://purl.org/dc/terms/MediaType

terms:MediaType rdf:type owl:Class ;
                
                rdfs:subClassOf terms:MediaTypeOrExtent .



###  http://purl.org/dc/terms/MediaTypeOrExtent

terms:MediaTypeOrExtent rdf:type owl:Class .



###  http://purl.org/dc/terms/MethodOfAccrual

terms:MethodOfAccrual rdf:type owl:Class .



###  http://purl.org/dc/terms/MethodOfInstruction

terms:MethodOfInstruction rdf:type owl:Class .



###  http://purl.org/dc/terms/PeriodOfTime

terms:PeriodOfTime rdf:type owl:Class ;
                   
                   rdfs:subClassOf terms:LocationPeriodOrJurisdiction .



###  http://purl.org/dc/terms/PhysicalMedium

terms:PhysicalMedium rdf:type owl:Class ;
                     
                     rdfs:subClassOf terms:MediaType .



###  http://purl.org/dc/terms/PhysicalResource

terms:PhysicalResource rdf:type owl:Class .



###  http://purl.org/dc/terms/Policy

terms:Policy rdf:type owl:Class .



###  http://purl.org/dc/terms/ProvenanceStatement

terms:ProvenanceStatement rdf:type owl:Class .



###  http://purl.org/dc/terms/RightsStatement

terms:RightsStatement rdf:type owl:Class .



###  http://purl.org/dc/terms/SizeOrDuration

terms:SizeOrDuration rdf:type owl:Class ;
                     
                     rdfs:subClassOf terms:MediaTypeOrExtent .



###  http://purl.org/dc/terms/Standard

terms:Standard rdf:type owl:Class .



###  http://www.w3.org/2000/01/rdf-schema#Class

rdfs:Class rdf:type owl:Class .





#################################################################
#
#    Individuals
#
#################################################################


###  http://data.finance.gov.au/def/agrif#Active

:Active rdf:type :Status ,
                 owl:NamedIndividual .



###  http://data.finance.gov.au/def/agrif#Approved

:Approved rdf:type :DecisionStatus ,
                   owl:NamedIndividual .



###  http://data.finance.gov.au/def/agrif#AwaitingDisposal

:AwaitingDisposal rdf:type :Status ,
                           owl:NamedIndividual .



###  http://data.finance.gov.au/def/agrif#Completed

:Completed rdf:type :Status ,
                    owl:NamedIndividual .



###  http://data.finance.gov.au/def/agrif#Confidential

:Confidential rdf:type :SecurityClassification ,
                       owl:NamedIndividual ;
              
              rdfs:label "Confidential"@en .



###  http://data.finance.gov.au/def/agrif#Disapproved

:Disapproved rdf:type :DecisionStatus ,
                      owl:NamedIndividual .



###  http://data.finance.gov.au/def/agrif#Disposed

:Disposed rdf:type :Status ,
                   owl:NamedIndividual .



###  http://data.finance.gov.au/def/agrif#HighlyProtected

:HighlyProtected rdf:type :SecurityClassification ,
                          owl:NamedIndividual ;
                 
                 rdfs:label "Highly Protected"@en .



###  http://data.finance.gov.au/def/agrif#Protected

:Protected rdf:type :SecurityClassification ,
                    owl:NamedIndividual ;
           
           rdfs:label "Protected"@en .



###  http://data.finance.gov.au/def/agrif#Redundant

:Redundant rdf:type :Status ,
                    owl:NamedIndividual .



###  http://data.finance.gov.au/def/agrif#RetainAsNationalArchives

:RetainAsNationalArchives rdf:type :DisposalClass ,
                                   owl:NamedIndividual .



###  http://data.finance.gov.au/def/agrif#Secret

:Secret rdf:type :SecurityClassification ,
                 owl:NamedIndividual ;
        
        rdfs:label "Secret"@en .



###  http://data.finance.gov.au/def/agrif#TopSecretNV

:TopSecretNV rdf:type :SecurityClassification ,
                      owl:NamedIndividual ;
             
             rdfs:label "Top Secret (NV)"@en .



###  http://data.finance.gov.au/def/agrif#TopSecretPV

:TopSecretPV rdf:type :SecurityClassification ,
                      owl:NamedIndividual ;
             
             rdfs:label "Top Secret (PV)"@en .



###  http://data.finance.gov.au/def/agrif#Unclassified

:Unclassified rdf:type :SecurityClassification ,
                       owl:NamedIndividual ;
              
              rdfs:label "Unclassified"@en .



###  http://purl.org/dc/aboutdcmi#DCMI

<http://purl.org/dc/aboutdcmi#DCMI> rdf:type owl:NamedIndividual .



###  http://purl.org/dc/terms/

terms: rdf:type owl:NamedIndividual ;
       
       terms:modified "2012-06-14"^^xsd:date ;
       
       terms:title "DCMI Metadata Terms - other"@en ;
       
       terms:publisher <http://purl.org/dc/aboutdcmi#DCMI> .



###  http://purl.org/dc/terms/Agent

terms:Agent rdf:type terms:AgentClass ,
                     owl:NamedIndividual .



###  http://purl.org/dc/terms/AgentClass

terms:AgentClass rdf:type owl:NamedIndividual .



###  http://purl.org/dc/terms/BibliographicResource

terms:BibliographicResource rdf:type owl:NamedIndividual .



###  http://purl.org/dc/terms/Box

terms:Box rdf:type owl:NamedIndividual .



###  http://purl.org/dc/terms/DCMIType

terms:DCMIType rdf:type <http://purl.org/dc/dcam/VocabularyEncodingScheme> ,
                        owl:NamedIndividual ;
               
               rdfs:label "DCMI Type Vocabulary"@en ;
               
               terms:issued "2000-07-11"^^xsd:date ;
               
               terms:modified "2012-06-14"^^xsd:date ;
               
               rdfs:comment "The set of classes specified by the DCMI Type Vocabulary, used to categorize the nature or genre of the resource."@en ;
               
               terms:hasVersion <http://dublincore.org/usage/terms/history/#DCMIType-005> ;
               
               rdfs:seeAlso <http://purl.org/dc/dcmitype/> ;
               
               rdfs:isDefinedBy terms: .



###  http://purl.org/dc/terms/DDC

terms:DDC rdf:type <http://purl.org/dc/dcam/VocabularyEncodingScheme> ,
                   owl:NamedIndividual ;
          
          rdfs:label "DDC"@en ;
          
          terms:issued "2000-07-11"^^xsd:date ;
          
          terms:modified "2008-01-14"^^xsd:date ;
          
          rdfs:comment "The set of conceptual resources specified by the Dewey Decimal Classification."@en ;
          
          terms:hasVersion <http://dublincore.org/usage/terms/history/#DDC-003> ;
          
          rdfs:isDefinedBy terms: ;
          
          rdfs:seeAlso <http://www.oclc.org/dewey/> .



###  http://purl.org/dc/terms/FileFormat

terms:FileFormat rdf:type owl:NamedIndividual .



###  http://purl.org/dc/terms/Frequency

terms:Frequency rdf:type owl:NamedIndividual .



###  http://purl.org/dc/terms/IMT

terms:IMT rdf:type <http://purl.org/dc/dcam/VocabularyEncodingScheme> ,
                   owl:NamedIndividual ;
          
          rdfs:label "IMT"@en ;
          
          terms:issued "2000-07-11"^^xsd:date ;
          
          terms:modified "2008-01-14"^^xsd:date ;
          
          rdfs:comment "The set of media types specified by the Internet Assigned Numbers Authority."@en ;
          
          terms:hasVersion <http://dublincore.org/usage/terms/history/#IMT-004> ;
          
          rdfs:isDefinedBy terms: ;
          
          rdfs:seeAlso <http://www.iana.org/assignments/media-types/> .



###  http://purl.org/dc/terms/ISO3166

terms:ISO3166 rdf:type owl:NamedIndividual .



###  http://purl.org/dc/terms/ISO639-2

terms:ISO639-2 rdf:type owl:NamedIndividual .



###  http://purl.org/dc/terms/ISO639-3

terms:ISO639-3 rdf:type owl:NamedIndividual .



###  http://purl.org/dc/terms/Jurisdiction

terms:Jurisdiction rdf:type owl:NamedIndividual .



###  http://purl.org/dc/terms/LCC

terms:LCC rdf:type <http://purl.org/dc/dcam/VocabularyEncodingScheme> ,
                   owl:NamedIndividual ;
          
          rdfs:label "LCC"@en ;
          
          terms:issued "2000-07-11"^^xsd:date ;
          
          terms:modified "2008-01-14"^^xsd:date ;
          
          rdfs:comment "The set of conceptual resources specified by the Library of Congress Classification."@en ;
          
          terms:hasVersion <http://dublincore.org/usage/terms/history/#LCC-003> ;
          
          rdfs:seeAlso <http://lcweb.loc.gov/catdir/cpso/lcco/lcco.html> ;
          
          rdfs:isDefinedBy terms: .



###  http://purl.org/dc/terms/LCSH

terms:LCSH rdf:type <http://purl.org/dc/dcam/VocabularyEncodingScheme> ,
                    owl:NamedIndividual ;
           
           rdfs:label "LCSH"@en ;
           
           terms:issued "2000-07-11"^^xsd:date ;
           
           terms:modified "2008-01-14"^^xsd:date ;
           
           rdfs:comment "The set of labeled concepts specified by the Library of Congress Subject Headings."@en ;
           
           terms:hasVersion <http://dublincore.org/usage/terms/history/#LCSH-003> ;
           
           rdfs:isDefinedBy terms: .



###  http://purl.org/dc/terms/LicenseDocument

terms:LicenseDocument rdf:type owl:NamedIndividual .



###  http://purl.org/dc/terms/LinguisticSystem

terms:LinguisticSystem rdf:type owl:NamedIndividual .



###  http://purl.org/dc/terms/Location

terms:Location rdf:type owl:NamedIndividual .



###  http://purl.org/dc/terms/LocationPeriodOrJurisdiction

terms:LocationPeriodOrJurisdiction rdf:type owl:NamedIndividual .



###  http://purl.org/dc/terms/MESH

terms:MESH rdf:type <http://purl.org/dc/dcam/VocabularyEncodingScheme> ,
                    owl:NamedIndividual ;
           
           rdfs:label "MeSH"@en ;
           
           terms:issued "2000-07-11"^^xsd:date ;
           
           terms:modified "2008-01-14"^^xsd:date ;
           
           rdfs:comment "The set of labeled concepts specified by the Medical Subject Headings."@en ;
           
           terms:hasVersion <http://dublincore.org/usage/terms/history/#MESH-003> ;
           
           rdfs:isDefinedBy terms: ;
           
           rdfs:seeAlso <http://www.nlm.nih.gov/mesh/meshhome.html> .



###  http://purl.org/dc/terms/MediaType

terms:MediaType rdf:type owl:NamedIndividual .



###  http://purl.org/dc/terms/MediaTypeOrExtent

terms:MediaTypeOrExtent rdf:type owl:NamedIndividual .



###  http://purl.org/dc/terms/MethodOfAccrual

terms:MethodOfAccrual rdf:type owl:NamedIndividual .



###  http://purl.org/dc/terms/MethodOfInstruction

terms:MethodOfInstruction rdf:type owl:NamedIndividual .



###  http://purl.org/dc/terms/NLM

terms:NLM rdf:type <http://purl.org/dc/dcam/VocabularyEncodingScheme> ,
                   owl:NamedIndividual ;
          
          rdfs:label "NLM"@en ;
          
          terms:issued "2005-06-13"^^xsd:date ;
          
          terms:modified "2008-01-14"^^xsd:date ;
          
          rdfs:comment "The set of conceptual resources specified by the National Library of Medicine Classification."@en ;
          
          terms:hasVersion <http://dublincore.org/usage/terms/history/#NLM-002> ;
          
          rdfs:isDefinedBy terms: ;
          
          rdfs:seeAlso <http://wwwcf.nlm.nih.gov/class/> .



###  http://purl.org/dc/terms/Period

terms:Period rdf:type owl:NamedIndividual .



###  http://purl.org/dc/terms/PeriodOfTime

terms:PeriodOfTime rdf:type owl:NamedIndividual .



###  http://purl.org/dc/terms/PhysicalMedium

terms:PhysicalMedium rdf:type owl:NamedIndividual .



###  http://purl.org/dc/terms/PhysicalResource

terms:PhysicalResource rdf:type owl:NamedIndividual .



###  http://purl.org/dc/terms/Point

terms:Point rdf:type owl:NamedIndividual .



###  http://purl.org/dc/terms/Policy

terms:Policy rdf:type owl:NamedIndividual .



###  http://purl.org/dc/terms/ProvenanceStatement

terms:ProvenanceStatement rdf:type owl:NamedIndividual .



###  http://purl.org/dc/terms/RFC1766

terms:RFC1766 rdf:type owl:NamedIndividual .



###  http://purl.org/dc/terms/RFC3066

terms:RFC3066 rdf:type owl:NamedIndividual .



###  http://purl.org/dc/terms/RFC4646

terms:RFC4646 rdf:type owl:NamedIndividual .



###  http://purl.org/dc/terms/RFC5646

terms:RFC5646 rdf:type owl:NamedIndividual .



###  http://purl.org/dc/terms/RightsStatement

terms:RightsStatement rdf:type owl:NamedIndividual .



###  http://purl.org/dc/terms/SizeOrDuration

terms:SizeOrDuration rdf:type owl:NamedIndividual .



###  http://purl.org/dc/terms/Standard

terms:Standard rdf:type owl:NamedIndividual .



###  http://purl.org/dc/terms/TGN

terms:TGN rdf:type <http://purl.org/dc/dcam/VocabularyEncodingScheme> ,
                   owl:NamedIndividual ;
          
          rdfs:label "TGN"@en ;
          
          terms:issued "2000-07-11"^^xsd:date ;
          
          terms:modified "2008-01-14"^^xsd:date ;
          
          rdfs:comment "The set of places specified by the Getty Thesaurus of Geographic Names."@en ;
          
          terms:hasVersion <http://dublincore.org/usage/terms/history/#TGN-003> ;
          
          rdfs:isDefinedBy terms: ;
          
          rdfs:seeAlso <http://www.getty.edu/research/tools/vocabulary/tgn/index.html> .



###  http://purl.org/dc/terms/UDC

terms:UDC rdf:type <http://purl.org/dc/dcam/VocabularyEncodingScheme> ,
                   owl:NamedIndividual ;
          
          rdfs:label "UDC"@en ;
          
          terms:issued "2000-07-11"^^xsd:date ;
          
          terms:modified "2008-01-14"^^xsd:date ;
          
          rdfs:comment "The set of conceptual resources specified by the Universal Decimal Classification."@en ;
          
          terms:hasVersion <http://dublincore.org/usage/terms/history/#UDC-003> ;
          
          rdfs:isDefinedBy terms: ;
          
          rdfs:seeAlso <http://www.udcc.org/> .



###  http://purl.org/dc/terms/URI

terms:URI rdf:type owl:NamedIndividual .



###  http://purl.org/dc/terms/W3CDTF

terms:W3CDTF rdf:type owl:NamedIndividual .



###  http://purl.org/dc/terms/abstract

terms:abstract rdf:type owl:NamedIndividual .



###  http://purl.org/dc/terms/accessRights

terms:accessRights rdf:type owl:NamedIndividual .



###  http://purl.org/dc/terms/accrualMethod

terms:accrualMethod rdf:type owl:NamedIndividual .



###  http://purl.org/dc/terms/accrualPeriodicity

terms:accrualPeriodicity rdf:type owl:NamedIndividual .



###  http://purl.org/dc/terms/accrualPolicy

terms:accrualPolicy rdf:type owl:NamedIndividual .



###  http://purl.org/dc/terms/alternative

terms:alternative rdf:type owl:NamedIndividual .



###  http://purl.org/dc/terms/audience

terms:audience rdf:type owl:NamedIndividual .



###  http://purl.org/dc/terms/available

terms:available rdf:type owl:NamedIndividual .



###  http://purl.org/dc/terms/bibliographicCitation

terms:bibliographicCitation rdf:type owl:NamedIndividual .



###  http://purl.org/dc/terms/conformsTo

terms:conformsTo rdf:type owl:NamedIndividual .



###  http://purl.org/dc/terms/contributor

terms:contributor rdf:type owl:NamedIndividual .



###  http://purl.org/dc/terms/coverage

terms:coverage rdf:type owl:NamedIndividual .



###  http://purl.org/dc/terms/created

terms:created rdf:type owl:NamedIndividual .



###  http://purl.org/dc/terms/creator

terms:creator rdf:type owl:NamedIndividual .



###  http://purl.org/dc/terms/date

terms:date rdf:type owl:NamedIndividual .



###  http://purl.org/dc/terms/dateAccepted

terms:dateAccepted rdf:type owl:NamedIndividual .



###  http://purl.org/dc/terms/dateCopyrighted

terms:dateCopyrighted rdf:type owl:NamedIndividual .



###  http://purl.org/dc/terms/dateSubmitted

terms:dateSubmitted rdf:type owl:NamedIndividual .



###  http://purl.org/dc/terms/description

terms:description rdf:type owl:NamedIndividual .



###  http://purl.org/dc/terms/educationLevel

terms:educationLevel rdf:type owl:NamedIndividual .



###  http://purl.org/dc/terms/extent

terms:extent rdf:type owl:NamedIndividual .



###  http://purl.org/dc/terms/format

terms:format rdf:type owl:NamedIndividual .



###  http://purl.org/dc/terms/hasFormat

terms:hasFormat rdf:type owl:NamedIndividual .



###  http://purl.org/dc/terms/hasPart

terms:hasPart rdf:type owl:NamedIndividual .



###  http://purl.org/dc/terms/hasVersion

terms:hasVersion rdf:type owl:NamedIndividual .



###  http://purl.org/dc/terms/identifier

terms:identifier rdf:type owl:NamedIndividual .



###  http://purl.org/dc/terms/instructionalMethod

terms:instructionalMethod rdf:type owl:NamedIndividual .



###  http://purl.org/dc/terms/isFormatOf

terms:isFormatOf rdf:type owl:NamedIndividual .



###  http://purl.org/dc/terms/isPartOf

terms:isPartOf rdf:type owl:NamedIndividual .



###  http://purl.org/dc/terms/isReferencedBy

terms:isReferencedBy rdf:type owl:NamedIndividual .



###  http://purl.org/dc/terms/isReplacedBy

terms:isReplacedBy rdf:type owl:NamedIndividual .



###  http://purl.org/dc/terms/isRequiredBy

terms:isRequiredBy rdf:type owl:NamedIndividual .



###  http://purl.org/dc/terms/isVersionOf

terms:isVersionOf rdf:type owl:NamedIndividual .



###  http://purl.org/dc/terms/issued

terms:issued rdf:type owl:NamedIndividual .



###  http://purl.org/dc/terms/language

terms:language rdf:type owl:NamedIndividual .



###  http://purl.org/dc/terms/license

terms:license rdf:type owl:NamedIndividual .



###  http://purl.org/dc/terms/mediator

terms:mediator rdf:type owl:NamedIndividual .



###  http://purl.org/dc/terms/medium

terms:medium rdf:type owl:NamedIndividual .



###  http://purl.org/dc/terms/modified

terms:modified rdf:type owl:NamedIndividual .



###  http://purl.org/dc/terms/provenance

terms:provenance rdf:type owl:NamedIndividual .



###  http://purl.org/dc/terms/publisher

terms:publisher rdf:type owl:NamedIndividual .



###  http://purl.org/dc/terms/references

terms:references rdf:type owl:NamedIndividual .



###  http://purl.org/dc/terms/relation

terms:relation rdf:type owl:NamedIndividual .



###  http://purl.org/dc/terms/replaces

terms:replaces rdf:type owl:NamedIndividual .



###  http://purl.org/dc/terms/requires

terms:requires rdf:type owl:NamedIndividual .



###  http://purl.org/dc/terms/rights

terms:rights rdf:type owl:NamedIndividual .



###  http://purl.org/dc/terms/rightsHolder

terms:rightsHolder rdf:type owl:NamedIndividual .



###  http://purl.org/dc/terms/source

terms:source rdf:type owl:NamedIndividual .



###  http://purl.org/dc/terms/spatial

terms:spatial rdf:type owl:NamedIndividual .



###  http://purl.org/dc/terms/subject

terms:subject rdf:type owl:NamedIndividual .



###  http://purl.org/dc/terms/tableOfContents

terms:tableOfContents rdf:type owl:NamedIndividual .



###  http://purl.org/dc/terms/temporal

terms:temporal rdf:type owl:NamedIndividual .



###  http://purl.org/dc/terms/title

terms:title rdf:type owl:NamedIndividual .



###  http://purl.org/dc/terms/type

terms:type rdf:type owl:NamedIndividual .



###  http://purl.org/dc/terms/valid

terms:valid rdf:type owl:NamedIndividual .





#################################################################
#
#    Annotations
#
#################################################################


terms:BibliographicResource rdfs:label "Bibliographic Resource"@en ;
                            
                            terms:issued "2008-01-14"^^xsd:date ;
                            
                            rdfs:comment "A book, article, or other documentary resource."@en ;
                            
                            terms:hasVersion <http://dublincore.org/usage/terms/history/#BibliographicResource-001> ;
                            
                            rdfs:isDefinedBy terms: .



terms:issued rdfs:label "Date Issued"@en ;
             
             terms:issued "2000-07-11"^^xsd:date ;
             
             terms:modified "2008-01-14"^^xsd:date ;
             
             rdfs:comment "Date of formal issuance (e.g., publication) of the resource."@en ;
             
             terms:hasVersion <http://dublincore.org/usage/terms/history/#issued-003> ;
             
             rdfs:isDefinedBy terms: .



terms:FileFormat rdfs:label "File Format"@en ;
                 
                 terms:issued "2008-01-14"^^xsd:date ;
                 
                 rdfs:comment "A digital resource format."@en ;
                 
                 terms:description "Examples include the formats defined by the list of Internet Media Types."@en ;
                 
                 terms:hasVersion <http://dublincore.org/usage/terms/history/#FileFormat-001> ;
                 
                 rdfs:isDefinedBy terms: .



terms:RFC3066 rdfs:label "RFC 3066"@en ;
              
              terms:issued "2002-07-13"^^xsd:date ;
              
              terms:modified "2008-01-14"^^xsd:date ;
              
              terms:description "RFC 3066 has been obsoleted by RFC 4646."@en ;
              
              rdfs:comment "The set of tags constructed according to RFC 3066 for the identification of languages."@en ;
              
              terms:hasVersion <http://dublincore.org/usage/terms/history/#RFC3066-002> ;
              
              rdfs:isDefinedBy terms: ;
              
              rdfs:seeAlso <http://www.ietf.org/rfc/rfc3066.txt> .



terms:modified rdfs:label "Date Modified"@en ;
               
               terms:issued "2000-07-11"^^xsd:date ;
               
               terms:modified "2008-01-14"^^xsd:date ;
               
               rdfs:comment "Date on which the resource was changed."@en ;
               
               terms:hasVersion <http://dublincore.org/usage/terms/history/#modified-003> ;
               
               rdfs:isDefinedBy terms: .



terms:isVersionOf rdfs:label "Is Version Of"@en ;
                  
                  terms:issued "2000-07-11"^^xsd:date ;
                  
                  terms:modified "2008-01-14"^^xsd:date ;
                  
                  rdfs:comment "A related resource of which the described resource is a version, edition, or adaptation."@en ;
                  
                  terms:description "Changes in version imply substantive changes in content rather than differences in format."@en ;
                  
                  skos:note "This term is intended to be used with non-literal values as defined in the DCMI Abstract Model (http://dublincore.org/documents/abstract-model/).  As of December 2007, the DCMI Usage Board is seeking a way to express this intention with a formal range declaration."@en ;
                  
                  terms:hasVersion <http://dublincore.org/usage/terms/history/#isVersionOf-003> ;
                  
                  rdfs:isDefinedBy terms: .



terms:Frequency rdfs:label "Frequency"@en ;
                
                terms:issued "2008-01-14"^^xsd:date ;
                
                rdfs:comment "A rate at which something recurs."@en ;
                
                terms:hasVersion <http://dublincore.org/usage/terms/history/#Frequency-001> ;
                
                rdfs:isDefinedBy terms: .



terms:bibliographicCitation rdfs:label "Bibliographic Citation"@en ;
                            
                            terms:issued "2003-02-15"^^xsd:date ;
                            
                            terms:modified "2008-01-14"^^xsd:date ;
                            
                            rdfs:comment "A bibliographic reference for the resource."@en ;
                            
                            terms:description "Recommended practice is to include sufficient bibliographic detail to identify the resource as unambiguously as possible."@en ;
                            
                            terms:hasVersion <http://dublincore.org/usage/terms/history/#bibliographicCitation-002> ;
                            
                            rdfs:isDefinedBy terms: .



terms:spatial rdfs:label "Spatial Coverage"@en ;
              
              terms:issued "2000-07-11"^^xsd:date ;
              
              terms:modified "2008-01-14"^^xsd:date ;
              
              rdfs:comment "Spatial characteristics of the resource."@en ;
              
              terms:hasVersion <http://dublincore.org/usage/terms/history/#spatial-003> ;
              
              rdfs:isDefinedBy terms: .



terms:temporal rdfs:label "Temporal Coverage"@en ;
               
               terms:issued "2000-07-11"^^xsd:date ;
               
               terms:modified "2008-01-14"^^xsd:date ;
               
               rdfs:comment "Temporal characteristics of the resource."@en ;
               
               terms:hasVersion <http://dublincore.org/usage/terms/history/#temporal-003> ;
               
               rdfs:isDefinedBy terms: .



terms:hasFormat rdfs:label "Has Format"@en ;
                
                terms:issued "2000-07-11"^^xsd:date ;
                
                terms:modified "2008-01-14"^^xsd:date ;
                
                rdfs:comment "A related resource that is substantially the same as the pre-existing described resource, but in another format."@en ;
                
                skos:note "This term is intended to be used with non-literal values as defined in the DCMI Abstract Model (http://dublincore.org/documents/abstract-model/).  As of December 2007, the DCMI Usage Board is seeking a way to express this intention with a formal range declaration."@en ;
                
                terms:hasVersion <http://dublincore.org/usage/terms/history/#hasFormat-003> ;
                
                rdfs:isDefinedBy terms: .



terms:date rdfs:label "Date"@en ;
           
           terms:issued "2008-01-14"^^xsd:date ;
           
           terms:modified "2008-01-14"^^xsd:date ;
           
           rdfs:comment "A point or period of time associated with an event in the lifecycle of the resource."@en ;
           
           terms:description "Date may be used to express temporal information at any level of granularity.  Recommended best practice is to use an encoding scheme, such as the W3CDTF profile of ISO 8601 [W3CDTF]."@en ;
           
           terms:hasVersion <http://dublincore.org/usage/terms/history/#dateT-001> ;
           
           rdfs:isDefinedBy terms: .



terms:extent rdfs:label "Extent"@en ;
             
             terms:issued "2000-07-11"^^xsd:date ;
             
             terms:modified "2008-01-14"^^xsd:date ;
             
             rdfs:comment "The size or duration of the resource."@en ;
             
             terms:hasVersion <http://dublincore.org/usage/terms/history/#extent-003> ;
             
             rdfs:isDefinedBy terms: .



terms:replaces rdfs:label "Replaces"@en ;
               
               terms:issued "2000-07-11"^^xsd:date ;
               
               terms:modified "2008-01-14"^^xsd:date ;
               
               rdfs:comment "A related resource that is supplanted, displaced, or superseded by the described resource."@en ;
               
               skos:note "This term is intended to be used with non-literal values as defined in the DCMI Abstract Model (http://dublincore.org/documents/abstract-model/).  As of December 2007, the DCMI Usage Board is seeking a way to express this intention with a formal range declaration."@en ;
               
               terms:hasVersion <http://dublincore.org/usage/terms/history/#replaces-003> ;
               
               rdfs:isDefinedBy terms: .



terms:references rdfs:label "References"@en ;
                 
                 terms:issued "2000-07-11"^^xsd:date ;
                 
                 terms:modified "2008-01-14"^^xsd:date ;
                 
                 rdfs:comment "A related resource that is referenced, cited, or otherwise pointed to by the described resource."@en ;
                 
                 skos:note "This term is intended to be used with non-literal values as defined in the DCMI Abstract Model (http://dublincore.org/documents/abstract-model/).  As of December 2007, the DCMI Usage Board is seeking a way to express this intention with a formal range declaration."@en ;
                 
                 terms:hasVersion <http://dublincore.org/usage/terms/history/#references-003> ;
                 
                 rdfs:isDefinedBy terms: .



terms:subject rdfs:label "Subject"@en ;
              
              terms:issued "2008-01-14"^^xsd:date ;
              
              terms:modified "2012-06-14"^^xsd:date ;
              
              rdfs:comment "The topic of the resource."@en ;
              
              skos:note "This term is intended to be used with non-literal values as defined in the DCMI Abstract Model (http://dublincore.org/documents/abstract-model/).  As of December 2007, the DCMI Usage Board is seeking a way to express this intention with a formal range declaration."@en ;
              
              terms:description "Typically, the subject will be represented using keywords, key phrases, or classification codes. Recommended best practice is to use a controlled vocabulary."@en ;
              
              terms:hasVersion <http://dublincore.org/usage/terms/history/#subjectT-002> ;
              
              rdfs:isDefinedBy terms: .



terms:rightsHolder rdfs:label "Rights Holder"@en ;
                   
                   terms:issued "2004-06-14"^^xsd:date ;
                   
                   terms:modified "2008-01-14"^^xsd:date ;
                   
                   rdfs:comment "A person or organization owning or managing rights over the resource."@en ;
                   
                   terms:hasVersion <http://dublincore.org/usage/terms/history/#rightsHolder-002> ;
                   
                   rdfs:isDefinedBy terms: .



terms:available rdfs:label "Date Available"@en ;
                
                terms:issued "2000-07-11"^^xsd:date ;
                
                terms:modified "2008-01-14"^^xsd:date ;
                
                rdfs:comment "Date (often a range) that the resource became or will become available."@en ;
                
                terms:hasVersion <http://dublincore.org/usage/terms/history/#available-003> ;
                
                rdfs:isDefinedBy terms: .



terms:Point rdfs:label "DCMI Point"@en ;
            
            terms:issued "2000-07-11"^^xsd:date ;
            
            terms:modified "2008-01-14"^^xsd:date ;
            
            rdfs:comment "The set of points in space defined by their geographic coordinates according to the DCMI Point Encoding Scheme."@en ;
            
            rdfs:seeAlso <http://dublincore.org/documents/dcmi-point/> ;
            
            terms:hasVersion <http://dublincore.org/usage/terms/history/#Point-003> ;
            
            rdfs:isDefinedBy terms: .



terms:MethodOfAccrual rdfs:label "Method of Accrual"@en ;
                      
                      terms:issued "2008-01-14"^^xsd:date ;
                      
                      rdfs:comment "A method by which resources are added to a collection."@en ;
                      
                      terms:hasVersion <http://dublincore.org/usage/terms/history/#MethodOfAccrual-001> ;
                      
                      rdfs:isDefinedBy terms: .



terms:license rdfs:label "License"@en ;
              
              terms:issued "2004-06-14"^^xsd:date ;
              
              terms:modified "2008-01-14"^^xsd:date ;
              
              rdfs:comment "A legal document giving official permission to do something with the resource."@en ;
              
              terms:hasVersion <http://dublincore.org/usage/terms/history/#license-002> ;
              
              rdfs:isDefinedBy terms: .



terms:isReferencedBy rdfs:label "Is Referenced By"@en ;
                     
                     terms:issued "2000-07-11"^^xsd:date ;
                     
                     terms:modified "2008-01-14"^^xsd:date ;
                     
                     rdfs:comment "A related resource that references, cites, or otherwise points to the described resource."@en ;
                     
                     skos:note "This term is intended to be used with non-literal values as defined in the DCMI Abstract Model (http://dublincore.org/documents/abstract-model/).  As of December 2007, the DCMI Usage Board is seeking a way to express this intention with a formal range declaration."@en ;
                     
                     terms:hasVersion <http://dublincore.org/usage/terms/history/#isReferencedBy-003> ;
                     
                     rdfs:isDefinedBy terms: .



terms:valid rdfs:label "Date Valid"@en ;
            
            terms:issued "2000-07-11"^^xsd:date ;
            
            terms:modified "2008-01-14"^^xsd:date ;
            
            rdfs:comment "Date (often a range) of validity of a resource."@en ;
            
            terms:hasVersion <http://dublincore.org/usage/terms/history/#valid-003> ;
            
            rdfs:isDefinedBy terms: .



terms:Jurisdiction rdfs:label "Jurisdiction"@en ;
                   
                   terms:issued "2008-01-14"^^xsd:date ;
                   
                   rdfs:comment "The extent or range of judicial, law enforcement, or other authority."@en ;
                   
                   terms:hasVersion <http://dublincore.org/usage/terms/history/#Jurisdiction-001> ;
                   
                   rdfs:isDefinedBy terms: .



terms:RightsStatement rdfs:label "Rights Statement"@en ;
                      
                      terms:issued "2008-01-14"^^xsd:date ;
                      
                      rdfs:comment "A statement about the intellectual property rights (IPR) held in or over a Resource, a legal document giving official permission to do something with a resource, or a statement about access rights."@en ;
                      
                      terms:hasVersion <http://dublincore.org/usage/terms/history/#RightsStatement-001> ;
                      
                      rdfs:isDefinedBy terms: .



terms:LocationPeriodOrJurisdiction rdfs:label "Location, Period, or Jurisdiction"@en ;
                                   
                                   terms:issued "2008-01-14"^^xsd:date ;
                                   
                                   rdfs:comment "A location, period of time, or jurisdiction."@en ;
                                   
                                   terms:hasVersion <http://dublincore.org/usage/terms/history/#LocationPeriodOrJurisdiction-001> ;
                                   
                                   rdfs:isDefinedBy terms: .



terms:educationLevel rdfs:label "Audience Education Level"@en ;
                     
                     terms:issued "2002-07-13"^^xsd:date ;
                     
                     terms:modified "2008-01-14"^^xsd:date ;
                     
                     rdfs:comment "A class of entity, defined in terms of progression through an educational or training context, for which the described resource is intended."@en ;
                     
                     terms:hasVersion <http://dublincore.org/usage/terms/history/#educationLevel-002> ;
                     
                     rdfs:isDefinedBy terms: .



terms:ISO3166 rdfs:label "ISO 3166"@en ;
              
              terms:issued "2000-07-11"^^xsd:date ;
              
              terms:modified "2008-01-14"^^xsd:date ;
              
              rdfs:comment "The set of codes listed in ISO 3166-1 for the representation of names of countries."@en ;
              
              terms:hasVersion <http://dublincore.org/usage/terms/history/#ISO3166-004> ;
              
              rdfs:isDefinedBy terms: ;
              
              rdfs:seeAlso <http://www.iso.org/iso/en/prods-services/iso3166ma/02iso-3166-code-lists/list-en1.html> .



terms:MediaType rdfs:label "Media Type"@en ;
                
                terms:issued "2008-01-14"^^xsd:date ;
                
                rdfs:comment "A file format or physical medium."@en ;
                
                terms:hasVersion <http://dublincore.org/usage/terms/history/#MediaType-001> ;
                
                rdfs:isDefinedBy terms: .



terms:dateSubmitted rdfs:label "Date Submitted"@en ;
                    
                    terms:issued "2002-07-13"^^xsd:date ;
                    
                    terms:modified "2008-01-14"^^xsd:date ;
                    
                    rdfs:comment "Date of submission of the resource."@en ;
                    
                    terms:description "Examples of resources to which a Date Submitted may be relevant are a thesis (submitted to a university department) or an article (submitted to a journal)."@en ;
                    
                    terms:hasVersion <http://dublincore.org/usage/terms/history/#dateSubmitted-002> ;
                    
                    rdfs:isDefinedBy terms: .



terms:accrualPeriodicity rdfs:label "Accrual Periodicity"@en ;
                         
                         terms:issued "2005-06-13"^^xsd:date ;
                         
                         terms:modified "2010-10-11"^^xsd:date ;
                         
                         rdfs:comment "The frequency with which items are added to a collection."@en ;
                         
                         terms:hasVersion <http://dublincore.org/usage/terms/history/#accrualPeriodicity-003> ;
                         
                         rdfs:isDefinedBy terms: .



terms:requires rdfs:label "Requires"@en ;
               
               terms:issued "2000-07-11"^^xsd:date ;
               
               terms:modified "2008-01-14"^^xsd:date ;
               
               rdfs:comment "A related resource that is required by the described resource to support its function, delivery, or coherence."@en ;
               
               skos:note "This term is intended to be used with non-literal values as defined in the DCMI Abstract Model (http://dublincore.org/documents/abstract-model/).  As of December 2007, the DCMI Usage Board is seeking a way to express this intention with a formal range declaration."@en ;
               
               terms:hasVersion <http://dublincore.org/usage/terms/history/#requires-003> ;
               
               rdfs:isDefinedBy terms: .



terms:conformsTo rdfs:label "Conforms To"@en ;
                 
                 terms:issued "2001-05-21"^^xsd:date ;
                 
                 terms:modified "2008-01-14"^^xsd:date ;
                 
                 rdfs:comment "An established standard to which the described resource conforms."@en ;
                 
                 terms:hasVersion <http://dublincore.org/usage/terms/history/#conformsTo-003> ;
                 
                 rdfs:isDefinedBy terms: .



terms:MethodOfInstruction rdfs:label "Method of Instruction"@en ;
                          
                          terms:issued "2008-01-14"^^xsd:date ;
                          
                          rdfs:comment "A process that is used to engender knowledge, attitudes, and skills."@en ;
                          
                          terms:hasVersion <http://dublincore.org/usage/terms/history/#MethodOfInstruction-001> ;
                          
                          rdfs:isDefinedBy terms: .



terms:Agent rdfs:label "Agent"@en ;
            
            terms:issued "2008-01-14"^^xsd:date ;
            
            rdfs:comment "A resource that acts or has the power to act."@en ;
            
            terms:description "Examples of Agent include person, organization, and software agent."@en ;
            
            terms:hasVersion <http://dublincore.org/usage/terms/history/#Agent-001> ;
            
            rdfs:isDefinedBy terms: .



terms:identifier rdfs:label "Identifier"@en ;
                 
                 terms:issued "2008-01-14"^^xsd:date ;
                 
                 terms:modified "2008-01-14"^^xsd:date ;
                 
                 rdfs:comment "An unambiguous reference to the resource within a given context."@en ;
                 
                 terms:description "Recommended best practice is to identify the resource by means of a string conforming to a formal identification system. "@en ;
                 
                 terms:hasVersion <http://dublincore.org/usage/terms/history/#identifierT-001> ;
                 
                 rdfs:isDefinedBy terms: .



terms:LinguisticSystem rdfs:label "Linguistic System"@en ;
                       
                       terms:issued "2008-01-14"^^xsd:date ;
                       
                       rdfs:comment "A system of signs, symbols, sounds, gestures, or rules used in communication."@en ;
                       
                       terms:description "Examples include written, spoken, sign, and computer languages."@en ;
                       
                       terms:hasVersion <http://dublincore.org/usage/terms/history/#LinguisticSystem-001> ;
                       
                       rdfs:isDefinedBy terms: .



terms:Policy rdfs:label "Policy"@en ;
             
             terms:issued "2008-01-14"^^xsd:date ;
             
             rdfs:comment "A plan or course of action by an authority, intended to influence and determine decisions, actions, and other matters."@en ;
             
             terms:hasVersion <http://dublincore.org/usage/terms/history/#Policy-001> ;
             
             rdfs:isDefinedBy terms: .



terms:audience rdfs:label "Audience"@en ;
               
               terms:issued "2001-05-21"^^xsd:date ;
               
               terms:modified "2008-01-14"^^xsd:date ;
               
               rdfs:comment "A class of entity for whom the resource is intended or useful."@en ;
               
               terms:hasVersion <http://dublincore.org/usage/terms/history/#audience-003> ;
               
               rdfs:isDefinedBy terms: .



terms:hasPart rdfs:label "Has Part"@en ;
              
              terms:issued "2000-07-11"^^xsd:date ;
              
              terms:modified "2008-01-14"^^xsd:date ;
              
              rdfs:comment "A related resource that is included either physically or logically in the described resource."@en ;
              
              skos:note "This term is intended to be used with non-literal values as defined in the DCMI Abstract Model (http://dublincore.org/documents/abstract-model/).  As of December 2007, the DCMI Usage Board is seeking a way to express this intention with a formal range declaration."@en ;
              
              terms:hasVersion <http://dublincore.org/usage/terms/history/#hasPart-003> ;
              
              rdfs:isDefinedBy terms: .



terms:MediaTypeOrExtent rdfs:label "Media Type or Extent"@en ;
                        
                        terms:issued "2008-01-14"^^xsd:date ;
                        
                        rdfs:comment "A media type or extent."@en ;
                        
                        terms:hasVersion <http://dublincore.org/usage/terms/history/#MediaTypeOrExtent-001> ;
                        
                        rdfs:isDefinedBy terms: .



terms:ISO639-3 rdfs:label "ISO 639-3"@en ;
               
               terms:issued "2008-01-14"^^xsd:date ;
               
               rdfs:comment "The set of three-letter codes listed in ISO 639-3 for the representation of names of languages."@en ;
               
               terms:hasVersion <http://dublincore.org/usage/terms/history/#ISO639-3-001> ;
               
               rdfs:isDefinedBy terms: ;
               
               rdfs:seeAlso <http://www.sil.org/iso639-3/> .



terms:PhysicalMedium rdfs:label "Physical Medium"@en ;
                     
                     terms:issued "2008-01-14"^^xsd:date ;
                     
                     rdfs:comment "A physical material or carrier."@en ;
                     
                     terms:description "Examples include paper, canvas, or DVD."@en ;
                     
                     terms:hasVersion <http://dublincore.org/usage/terms/history/#PhysicalMedium-001> ;
                     
                     rdfs:isDefinedBy terms: .



terms:created rdfs:label "Date Created"@en ;
              
              terms:issued "2000-07-11"^^xsd:date ;
              
              terms:modified "2008-01-14"^^xsd:date ;
              
              rdfs:comment "Date of creation of the resource."@en ;
              
              terms:hasVersion <http://dublincore.org/usage/terms/history/#created-003> ;
              
              rdfs:isDefinedBy terms: .



terms:ISO639-2 rdfs:label "ISO 639-2"@en ;
               
               terms:issued "2000-07-11"^^xsd:date ;
               
               terms:modified "2008-01-14"^^xsd:date ;
               
               rdfs:comment "The three-letter alphabetic codes listed in ISO639-2 for the representation of names of languages."@en ;
               
               terms:hasVersion <http://dublincore.org/usage/terms/history/#ISO639-2-003> ;
               
               rdfs:seeAlso <http://lcweb.loc.gov/standards/iso639-2/langhome.html> ;
               
               rdfs:isDefinedBy terms: .



terms:dateAccepted rdfs:label "Date Accepted"@en ;
                   
                   terms:issued "2002-07-13"^^xsd:date ;
                   
                   terms:modified "2008-01-14"^^xsd:date ;
                   
                   rdfs:comment "Date of acceptance of the resource."@en ;
                   
                   terms:description "Examples of resources to which a Date Accepted may be relevant are a thesis (accepted by a university department) or an article (accepted by a journal)."@en ;
                   
                   terms:hasVersion <http://dublincore.org/usage/terms/history/#dateAccepted-002> ;
                   
                   rdfs:isDefinedBy terms: .



terms:Period rdfs:label "DCMI Period"@en ;
             
             terms:issued "2000-07-11"^^xsd:date ;
             
             terms:modified "2008-01-14"^^xsd:date ;
             
             rdfs:comment "The set of time intervals defined by their limits according to the DCMI Period Encoding Scheme."@en ;
             
             rdfs:seeAlso <http://dublincore.org/documents/dcmi-period/> ;
             
             terms:hasVersion <http://dublincore.org/usage/terms/history/#Period-003> ;
             
             rdfs:isDefinedBy terms: .



terms:description rdfs:label "Description"@en ;
                  
                  terms:issued "2008-01-14"^^xsd:date ;
                  
                  terms:modified "2008-01-14"^^xsd:date ;
                  
                  rdfs:comment "An account of the resource."@en ;
                  
                  terms:description "Description may include but is not limited to: an abstract, a table of contents, a graphical representation, or a free-text account of the resource."@en ;
                  
                  terms:hasVersion <http://dublincore.org/usage/terms/history/#descriptionT-001> ;
                  
                  rdfs:isDefinedBy terms: .



terms:Box rdfs:label "DCMI Box"@en ;
          
          terms:issued "2000-07-11"^^xsd:date ;
          
          terms:modified "2008-01-14"^^xsd:date ;
          
          rdfs:comment "The set of regions in space defined by their geographic coordinates according to the DCMI Box Encoding Scheme."@en ;
          
          rdfs:seeAlso <http://dublincore.org/documents/dcmi-box/> ;
          
          terms:hasVersion <http://dublincore.org/usage/terms/history/#Box-003> ;
          
          rdfs:isDefinedBy terms: .



terms:source rdfs:label "Source"@en ;
             
             terms:modified "2008-01-14"^^xsd:date ;
             
             terms:issued "2008-01-14"^^xsd:date ;
             
             rdfs:comment "A related resource from which the described resource is derived."@en ;
             
             terms:description "The described resource may be derived from the related resource in whole or in part. Recommended best practice is to identify the related resource by means of a string conforming to a formal identification system."@en ;
             
             skos:note "This term is intended to be used with non-literal values as defined in the DCMI Abstract Model (http://dublincore.org/documents/abstract-model/).  As of December 2007, the DCMI Usage Board is seeking a way to express this intention with a formal range declaration."@en ;
             
             terms:hasVersion <http://dublincore.org/usage/terms/history/#sourceT-001> ;
             
             rdfs:isDefinedBy terms: .



terms:medium rdfs:label "Medium"@en ;
             
             terms:issued "2000-07-11"^^xsd:date ;
             
             terms:modified "2008-01-14"^^xsd:date ;
             
             rdfs:comment "The material or physical carrier of the resource."@en ;
             
             terms:hasVersion <http://dublincore.org/usage/terms/history/#medium-003> ;
             
             rdfs:isDefinedBy terms: .



terms:ProvenanceStatement rdfs:label "Provenance Statement"@en ;
                          
                          terms:issued "2008-01-14"^^xsd:date ;
                          
                          rdfs:comment "A statement of any changes in ownership and custody of a resource since its creation that are significant for its authenticity, integrity, and interpretation."@en ;
                          
                          terms:hasVersion <http://dublincore.org/usage/terms/history/#ProvenanceStatement-001> ;
                          
                          rdfs:isDefinedBy terms: .



terms:language rdfs:label "Language"@en ;
               
               terms:issued "2008-01-14"^^xsd:date ;
               
               terms:modified "2008-01-14"^^xsd:date ;
               
               rdfs:comment "A language of the resource."@en ;
               
               terms:description "Recommended best practice is to use a controlled vocabulary such as RFC 4646 [RFC4646]."@en ;
               
               terms:hasVersion <http://dublincore.org/usage/terms/history/#languageT-001> ;
               
               rdfs:isDefinedBy terms: .



terms:W3CDTF rdfs:label "W3C-DTF"@en ;
             
             terms:issued "2000-07-11"^^xsd:date ;
             
             terms:modified "2008-01-14"^^xsd:date ;
             
             rdfs:comment "The set of dates and times constructed according to the W3C Date and Time Formats Specification."@en ;
             
             terms:hasVersion <http://dublincore.org/usage/terms/history/#W3CDTF-003> ;
             
             rdfs:isDefinedBy terms: ;
             
             rdfs:seeAlso <http://www.w3.org/TR/NOTE-datetime> .



terms:LicenseDocument rdfs:label "License Document"@en ;
                      
                      terms:issued "2008-01-14"^^xsd:date ;
                      
                      rdfs:comment "A legal document giving official permission to do something with a Resource."@en ;
                      
                      terms:hasVersion <http://dublincore.org/usage/terms/history/#LicenseDocument-001> ;
                      
                      rdfs:isDefinedBy terms: .



terms:PeriodOfTime rdfs:label "Period of Time"@en ;
                   
                   terms:issued "2008-01-14"^^xsd:date ;
                   
                   rdfs:comment "An interval of time that is named or defined by its start and end dates."@en ;
                   
                   terms:hasVersion <http://dublincore.org/usage/terms/history/#PeriodOfTime-001> ;
                   
                   rdfs:isDefinedBy terms: .



terms:provenance rdfs:label "Provenance"@en ;
                 
                 terms:issued "2004-09-20"^^xsd:date ;
                 
                 terms:modified "2008-01-14"^^xsd:date ;
                 
                 rdfs:comment "A statement of any changes in ownership and custody of the resource since its creation that are significant for its authenticity, integrity, and interpretation."@en ;
                 
                 terms:description "The statement may include a description of any changes successive custodians made to the resource."@en ;
                 
                 terms:hasVersion <http://dublincore.org/usage/terms/history/#provenance-002> ;
                 
                 rdfs:isDefinedBy terms: .



terms:PhysicalResource rdfs:label "Physical Resource"@en ;
                       
                       terms:issued "2008-01-14"^^xsd:date ;
                       
                       rdfs:comment "A material thing."@en ;
                       
                       terms:hasVersion <http://dublincore.org/usage/terms/history/#PhysicalResource-001> ;
                       
                       rdfs:isDefinedBy terms: .



terms:accessRights rdfs:label "Access Rights"@en ;
                   
                   terms:issued "2003-02-15"^^xsd:date ;
                   
                   terms:modified "2008-01-14"^^xsd:date ;
                   
                   terms:description "Access Rights may include information regarding access or restrictions based on privacy, security, or other policies."@en ;
                   
                   rdfs:comment "Information about who can access the resource or an indication of its security status."@en ;
                   
                   terms:hasVersion <http://dublincore.org/usage/terms/history/#accessRights-002> ;
                   
                   rdfs:isDefinedBy terms: .



terms:publisher rdfs:label "Publisher"@en ;
                
                terms:issued "2008-01-14"^^xsd:date ;
                
                terms:modified "2010-10-11"^^xsd:date ;
                
                rdfs:comment "An entity responsible for making the resource available."@en ;
                
                terms:description "Examples of a Publisher include a person, an organization, or a service."@en ;
                
                terms:hasVersion <http://dublincore.org/usage/terms/history/#publisherT-001> ;
                
                rdfs:isDefinedBy terms: .



terms:tableOfContents rdfs:label "Table Of Contents"@en ;
                      
                      terms:issued "2000-07-11"^^xsd:date ;
                      
                      terms:modified "2008-01-14"^^xsd:date ;
                      
                      rdfs:comment "A list of subunits of the resource."@en ;
                      
                      terms:hasVersion <http://dublincore.org/usage/terms/history/#tableOfContents-003> ;
                      
                      rdfs:isDefinedBy terms: .



terms:Location rdfs:label "Location"@en ;
               
               terms:issued "2008-01-14"^^xsd:date ;
               
               rdfs:comment "A spatial region or named place."@en ;
               
               terms:hasVersion <http://dublincore.org/usage/terms/history/#Location-001> ;
               
               rdfs:isDefinedBy terms: .



terms:isRequiredBy rdfs:label "Is Required By"@en ;
                   
                   terms:issued "2000-07-11"^^xsd:date ;
                   
                   terms:modified "2008-01-14"^^xsd:date ;
                   
                   rdfs:comment "A related resource that requires the described resource to support its function, delivery, or coherence."@en ;
                   
                   skos:note "This term is intended to be used with non-literal values as defined in the DCMI Abstract Model (http://dublincore.org/documents/abstract-model/).  As of December 2007, the DCMI Usage Board is seeking a way to express this intention with a formal range declaration."@en ;
                   
                   terms:hasVersion <http://dublincore.org/usage/terms/history/#isRequiredBy-003> ;
                   
                   rdfs:isDefinedBy terms: .



terms:mediator rdfs:label "Mediator"@en ;
               
               terms:issued "2001-05-21"^^xsd:date ;
               
               terms:modified "2008-01-14"^^xsd:date ;
               
               rdfs:comment "An entity that mediates access to the resource and for whom the resource is intended or useful."@en ;
               
               terms:description "In an educational context, a mediator might be a parent, teacher, teaching assistant, or care-giver."@en ;
               
               terms:hasVersion <http://dublincore.org/usage/terms/history/#mediator-003> ;
               
               rdfs:isDefinedBy terms: .



terms:RFC4646 rdfs:label "RFC 4646"@en ;
              
              terms:issued "2008-01-14"^^xsd:date ;
              
              terms:description "RFC 4646 obsoletes RFC 3066."@en ;
              
              rdfs:comment "The set of tags constructed according to RFC 4646 for the identification of languages."@en ;
              
              terms:hasVersion <http://dublincore.org/usage/terms/history/#RFC4646-001> ;
              
              rdfs:isDefinedBy terms: ;
              
              rdfs:seeAlso <http://www.ietf.org/rfc/rfc4646.txt> .



terms:accrualPolicy rdfs:label "Accrual Policy"@en ;
                    
                    terms:issued "2005-06-13"^^xsd:date ;
                    
                    terms:modified "2010-10-11"^^xsd:date ;
                    
                    rdfs:comment "The policy governing the addition of items to a collection."@en ;
                    
                    terms:hasVersion <http://dublincore.org/usage/terms/history/#accrualPolicy-003> ;
                    
                    rdfs:isDefinedBy terms: .



terms:isPartOf rdfs:label "Is Part Of"@en ;
               
               terms:issued "2000-07-11"^^xsd:date ;
               
               terms:modified "2008-01-14"^^xsd:date ;
               
               rdfs:comment "A related resource in which the described resource is physically or logically included."@en ;
               
               skos:note "This term is intended to be used with non-literal values as defined in the DCMI Abstract Model (http://dublincore.org/documents/abstract-model/).  As of December 2007, the DCMI Usage Board is seeking a way to express this intention with a formal range declaration."@en ;
               
               terms:hasVersion <http://dublincore.org/usage/terms/history/#isPartOf-003> ;
               
               rdfs:isDefinedBy terms: .



terms:URI rdfs:label "URI"@en ;
          
          terms:issued "2000-07-11"^^xsd:date ;
          
          terms:modified "2008-01-14"^^xsd:date ;
          
          rdfs:comment "The set of identifiers constructed according to the generic syntax for Uniform Resource Identifiers as specified by the Internet Engineering Task Force."@en ;
          
          terms:hasVersion <http://dublincore.org/usage/terms/history/#URI-003> ;
          
          rdfs:isDefinedBy terms: ;
          
          rdfs:seeAlso <http://www.ietf.org/rfc/rfc3986.txt> .



terms:contributor rdfs:label "Contributor"@en ;
                  
                  terms:issued "2008-01-14"^^xsd:date ;
                  
                  terms:modified "2010-10-11"^^xsd:date ;
                  
                  rdfs:comment "An entity responsible for making contributions to the resource."@en ;
                  
                  terms:description "Examples of a Contributor include a person, an organization, or a service."@en ;
                  
                  terms:hasVersion <http://dublincore.org/usage/terms/history/#contributorT-001> ;
                  
                  rdfs:isDefinedBy terms: .



terms:accrualMethod rdfs:label "Accrual Method"@en ;
                    
                    terms:issued "2005-06-13"^^xsd:date ;
                    
                    terms:modified "2010-10-11"^^xsd:date ;
                    
                    rdfs:comment "The method by which items are added to a collection."@en ;
                    
                    terms:hasVersion <http://dublincore.org/usage/terms/history/#accrualMethod-003> ;
                    
                    rdfs:isDefinedBy terms: .



terms:SizeOrDuration rdfs:label "Size or Duration"@en ;
                     
                     terms:issued "2008-01-14"^^xsd:date ;
                     
                     rdfs:comment "A dimension or extent, or a time taken to play or execute."@en ;
                     
                     terms:description "Examples include a number of pages, a specification of length, width, and breadth, or a period in hours, minutes, and seconds."@en ;
                     
                     terms:hasVersion <http://dublincore.org/usage/terms/history/#SizeOrDuration-001> ;
                     
                     rdfs:isDefinedBy terms: .



terms:rights rdfs:label "Rights"@en ;
             
             terms:issued "2008-01-14"^^xsd:date ;
             
             terms:modified "2008-01-14"^^xsd:date ;
             
             rdfs:comment "Information about rights held in and over the resource."@en ;
             
             terms:description "Typically, rights information includes a statement about various property rights associated with the resource, including intellectual property rights."@en ;
             
             terms:hasVersion <http://dublincore.org/usage/terms/history/#rightsT-001> ;
             
             rdfs:isDefinedBy terms: .



terms:format rdfs:label "Format"@en ;
             
             terms:issued "2008-01-14"^^xsd:date ;
             
             terms:modified "2008-01-14"^^xsd:date ;
             
             terms:description "Examples of dimensions include size and duration. Recommended best practice is to use a controlled vocabulary such as the list of Internet Media Types [MIME]."@en ;
             
             rdfs:comment "The file format, physical medium, or dimensions of the resource."@en ;
             
             terms:hasVersion <http://dublincore.org/usage/terms/history/#formatT-001> ;
             
             rdfs:isDefinedBy terms: .



terms:instructionalMethod rdfs:label "Instructional Method"@en ;
                          
                          terms:issued "2005-06-13"^^xsd:date ;
                          
                          terms:modified "2008-01-14"^^xsd:date ;
                          
                          rdfs:comment "A process, used to engender knowledge, attitudes and skills, that the described resource is designed to support."@en ;
                          
                          terms:description "Instructional Method will typically include ways of presenting instructional materials or conducting instructional activities, patterns of learner-to-learner and learner-to-instructor interactions, and mechanisms by which group and individual levels of learning are measured.  Instructional methods include all aspects of the instruction and learning processes from planning and implementation through evaluation and feedback."@en ;
                          
                          terms:hasVersion <http://dublincore.org/usage/terms/history/#instructionalMethod-002> ;
                          
                          rdfs:isDefinedBy terms: .



terms:AgentClass rdfs:label "Agent Class"@en ;
                 
                 terms:issued "2008-01-14"^^xsd:date ;
                 
                 terms:modified "2012-06-14"^^xsd:date ;
                 
                 rdfs:comment "A group of agents."@en ;
                 
                 terms:description "Examples of Agent Class include groups seen as classes, such as students, women, charities, lecturers."@en ;
                 
                 terms:hasVersion <http://dublincore.org/usage/terms/history/#AgentClass-003> ;
                 
                 rdfs:isDefinedBy terms: .



terms:isReplacedBy rdfs:label "Is Replaced By"@en ;
                   
                   terms:issued "2000-07-11"^^xsd:date ;
                   
                   terms:modified "2008-01-14"^^xsd:date ;
                   
                   rdfs:comment "A related resource that supplants, displaces, or supersedes the described resource."@en ;
                   
                   skos:note "This term is intended to be used with non-literal values as defined in the DCMI Abstract Model (http://dublincore.org/documents/abstract-model/).  As of December 2007, the DCMI Usage Board is seeking a way to express this intention with a formal range declaration."@en ;
                   
                   terms:hasVersion <http://dublincore.org/usage/terms/history/#isReplacedBy-003> ;
                   
                   rdfs:isDefinedBy terms: .



terms:coverage rdfs:label "Coverage"@en ;
               
               terms:modified "2008-01-14"^^xsd:date ;
               
               terms:issued "2008-01-14"^^xsd:date ;
               
               terms:description "Spatial topic and spatial applicability may be a named place or a location specified by its geographic coordinates. Temporal topic may be a named period, date, or date range. A jurisdiction may be a named administrative entity or a geographic place to which the resource applies. Recommended best practice is to use a controlled vocabulary such as the Thesaurus of Geographic Names [TGN]. Where appropriate, named places or time periods can be used in preference to numeric identifiers such as sets of coordinates or date ranges."@en ;
               
               rdfs:comment "The spatial or temporal topic of the resource, the spatial applicability of the resource, or the jurisdiction under which the resource is relevant."@en ;
               
               terms:hasVersion <http://dublincore.org/usage/terms/history/#coverageT-001> ;
               
               rdfs:isDefinedBy terms: .



terms:isFormatOf rdfs:label "Is Format Of"@en ;
                 
                 terms:issued "2000-07-11"^^xsd:date ;
                 
                 terms:modified "2008-01-14"^^xsd:date ;
                 
                 rdfs:comment "A related resource that is substantially the same as the described resource, but in another format."@en ;
                 
                 skos:note "This term is intended to be used with non-literal values as defined in the DCMI Abstract Model (http://dublincore.org/documents/abstract-model/).  As of December 2007, the DCMI Usage Board is seeking a way to express this intention with a formal range declaration."@en ;
                 
                 terms:hasVersion <http://dublincore.org/usage/terms/history/#isFormatOf-003> ;
                 
                 rdfs:isDefinedBy terms: .



terms:creator rdfs:label "Creator"@en ;
              
              terms:issued "2008-01-14"^^xsd:date ;
              
              terms:modified "2010-10-11"^^xsd:date ;
              
              rdfs:comment "An entity primarily responsible for making the resource."@en ;
              
              terms:description "Examples of a Creator include a person, an organization, or a service."@en ;
              
              terms:hasVersion <http://dublincore.org/usage/terms/history/#creatorT-002> ;
              
              rdfs:isDefinedBy terms: .



terms:Standard rdfs:label "Standard"@en ;
               
               terms:issued "2008-01-14"^^xsd:date ;
               
               rdfs:comment "A basis for comparison; a reference point against which other things can be evaluated."@en ;
               
               terms:hasVersion <http://dublincore.org/usage/terms/history/#Standard-001> ;
               
               rdfs:isDefinedBy terms: .



terms:hasVersion rdfs:label "Has Version"@en ;
                 
                 terms:issued "2000-07-11"^^xsd:date ;
                 
                 terms:modified "2008-01-14"^^xsd:date ;
                 
                 rdfs:comment "A related resource that is a version, edition, or adaptation of the described resource."@en ;
                 
                 skos:note "This term is intended to be used with non-literal values as defined in the DCMI Abstract Model (http://dublincore.org/documents/abstract-model/).  As of December 2007, the DCMI Usage Board is seeking a way to express this intention with a formal range declaration."@en ;
                 
                 terms:hasVersion <http://dublincore.org/usage/terms/history/#hasVersion-003> ;
                 
                 rdfs:isDefinedBy terms: .



terms:relation rdfs:label "Relation"@en ;
               
               terms:modified "2008-01-14"^^xsd:date ;
               
               terms:issued "2008-01-14"^^xsd:date ;
               
               rdfs:comment "A related resource."@en ;
               
               terms:description "Recommended best practice is to identify the related resource by means of a string conforming to a formal identification system. "@en ;
               
               skos:note "This term is intended to be used with non-literal values as defined in the DCMI Abstract Model (http://dublincore.org/documents/abstract-model/).  As of December 2007, the DCMI Usage Board is seeking a way to express this intention with a formal range declaration."@en ;
               
               terms:hasVersion <http://dublincore.org/usage/terms/history/#relationT-001> ;
               
               rdfs:isDefinedBy terms: .



terms:abstract rdfs:label "Abstract"@en ;
               
               terms:issued "2000-07-11"^^xsd:date ;
               
               terms:modified "2008-01-14"^^xsd:date ;
               
               rdfs:comment "A summary of the resource."@en ;
               
               terms:hasVersion <http://dublincore.org/usage/terms/history/#abstract-003> ;
               
               rdfs:isDefinedBy terms: .



terms:alternative rdfs:label "Alternative Title"@en ;
                  
                  terms:issued "2000-07-11"^^xsd:date ;
                  
                  terms:modified "2010-10-11"^^xsd:date ;
                  
                  rdfs:comment "An alternative name for the resource."@en ;
                  
                  terms:description "The distinction between titles and alternative titles is application-specific."@en ;
                  
                  terms:hasVersion <http://dublincore.org/usage/terms/history/#alternative-003> ;
                  
                  rdfs:isDefinedBy terms: .



terms:title rdfs:label "Title"@en ;
            
            terms:issued "2008-01-14"^^xsd:date ;
            
            terms:modified "2010-10-11"^^xsd:date ;
            
            rdfs:comment "A name given to the resource."@en ;
            
            terms:hasVersion <http://dublincore.org/usage/terms/history/#titleT-002> ;
            
            rdfs:isDefinedBy terms: .



terms:type rdfs:label "Type"@en ;
           
           terms:modified "2008-01-14"^^xsd:date ;
           
           terms:issued "2008-01-14"^^xsd:date ;
           
           terms:description "Recommended best practice is to use a controlled vocabulary such as the DCMI Type Vocabulary [DCMITYPE]. To describe the file format, physical medium, or dimensions of the resource, use the Format element."@en ;
           
           rdfs:comment "The nature or genre of the resource."@en ;
           
           terms:hasVersion <http://dublincore.org/usage/terms/history/#typeT-001> ;
           
           rdfs:isDefinedBy terms: .



terms:RFC5646 rdfs:label "RFC 5646"@en ;
              
              terms:issued "2010-10-11"^^xsd:date ;
              
              terms:description "RFC 5646 obsoletes RFC 4646."@en ;
              
              rdfs:comment "The set of tags constructed according to RFC 5646 for the identification of languages."@en ;
              
              terms:hasVersion <http://dublincore.org/usage/terms/history/#RFC5646-001> ;
              
              rdfs:isDefinedBy terms: ;
              
              rdfs:seeAlso <http://www.ietf.org/rfc/rfc5646.txt> .



terms:dateCopyrighted rdfs:label "Date Copyrighted"@en ;
                      
                      terms:issued "2002-07-13"^^xsd:date ;
                      
                      terms:modified "2008-01-14"^^xsd:date ;
                      
                      rdfs:comment "Date of copyright."@en ;
                      
                      terms:hasVersion <http://dublincore.org/usage/terms/history/#dateCopyrighted-002> ;
                      
                      rdfs:isDefinedBy terms: .



terms:RFC1766 rdfs:label "RFC 1766"@en ;
              
              terms:issued "2000-07-11"^^xsd:date ;
              
              terms:modified "2008-01-14"^^xsd:date ;
              
              rdfs:comment "The set of tags, constructed according to RFC 1766, for the identification of languages."@en ;
              
              terms:hasVersion <http://dublincore.org/usage/terms/history/#RFC1766-003> ;
              
              rdfs:isDefinedBy terms: ;
              
              rdfs:seeAlso <http://www.ietf.org/rfc/rfc1766.txt> .




###  Generated by the OWL API (version 3.5.1) http://owlapi.sourceforge.net

