@prefix : <http://reference.data.gov.au/def/ont/agrif#> .
@prefix dc: <http://purl.org/dc/elements/1.1/> .
@prefix owl: <http://www.w3.org/2002/07/owl#> .
@prefix rdf: <http://www.w3.org/1999/02/22-rdf-syntax-ns#> .
@prefix xml: <http://www.w3.org/XML/1998/namespace> .
@prefix xsd: <http://www.w3.org/2001/XMLSchema#> .
@prefix rdfs: <http://www.w3.org/2000/01/rdf-schema#> .
@prefix skos: <http://www.w3.org/2004/02/skos/core#> .
@prefix dcterms: <http://purl.org/dc/terms/> .
@prefix vann: <http://purl.org/vocab/vann/> .
@base <http://reference.data.gov.au/def/ont/agrif> .

<http://reference.data.gov.au/def/ont/agrif> rdf:type owl:Ontology ;
                                              owl:versionIRI <http://reference.data.gov.au/def/ont/agrif/0.6> ;
                                              dc:contributor "Nicholas Car"@en ;
                                              dcterms:contributor <http://orcid.org/0000-0002-8742-7730> ;
                                              dc:creator "Armin Haller"@en ;
                                              rdfs:label "The Australian Government Records Interoperability Framework (AGRIF) ontology"@en ;
                                              dc:creator "John Machin"@en ;
                                              rdfs:comment "The Australian Government Records Interoperability Framework (AGRIF, ‘the Framework’) is a system of related semantic ontologies that describe the structure, functions, and activities of the Australian Government, providing sufficient context for the effective use – including but not limited to management – of Australian Government information assets. It complies with the World Wide Web Consortium’s Web Ontology Language (OWL2) Recommendation and makes reference to other Recommendations and existing domain ontologies for archival and preservation processes."@en ;
                                              dc:creator "Katherine Stuart"@en ;
                                              dcterms:license <https://creativecommons.org/licenses/by/4.0/> ;
                                              dc:publisher "Australian Government Linked Data Working Group"@en ;
                                              dcterms:publisher <http://linked.data.gov.au> ;
                                              owl:versionInfo "0.6"@en ;
											  dcterms:created "2016-12-06"^^xsd:date ;
											  vann:preferredNamespaceUri "http://reference.data.gov.au/def/ont/agrif#"^^xsd:string ;
											  vann:preferredNamespacePrefix "agrif"@en ;
											  dcterms:modified "2017-08-21"@en ;
											  dcterms:rights "(c) Commonwealth of Australia (Department of Finance) 2017"@en ;
											  rdfs:seeAlso <https://github.com/nicholascar/agrif-ont> .
											  

#################################################################
#    Annotation properties
#################################################################

###  http://purl.org/dc/elements/1.1/contributor
dc:contributor rdf:type owl:AnnotationProperty .


###  http://purl.org/dc/elements/1.1/coverage
dc:coverage rdf:type owl:AnnotationProperty .


###  http://purl.org/dc/elements/1.1/creator
dc:creator rdf:type owl:AnnotationProperty .


###  http://purl.org/dc/elements/1.1/date
dc:date rdf:type owl:AnnotationProperty .


###  http://purl.org/dc/elements/1.1/description
dc:description rdf:type owl:AnnotationProperty .


###  http://purl.org/dc/elements/1.1/format
dc:format rdf:type owl:AnnotationProperty .


###  http://purl.org/dc/elements/1.1/identifier
dc:identifier rdf:type owl:AnnotationProperty .


###  http://purl.org/dc/elements/1.1/language
dc:language rdf:type owl:AnnotationProperty .


###  http://purl.org/dc/elements/1.1/publisher
dc:publisher rdf:type owl:AnnotationProperty .


###  http://purl.org/dc/elements/1.1/relation
dc:relation rdf:type owl:AnnotationProperty .


###  http://purl.org/dc/elements/1.1/rights
dc:rights rdf:type owl:AnnotationProperty .


###  http://purl.org/dc/elements/1.1/source
dc:source rdf:type owl:AnnotationProperty .


###  http://purl.org/dc/elements/1.1/subject
dc:subject rdf:type owl:AnnotationProperty .


###  http://purl.org/dc/elements/1.1/title
dc:title rdf:type owl:AnnotationProperty .


###  http://purl.org/dc/elements/1.1/type
dc:type rdf:type owl:AnnotationProperty .


###  http://purl.org/dc/terms/abstract
dcterms:abstract rdf:type owl:AnnotationProperty ;
               rdfs:subPropertyOf dc:description ,
                                  dcterms:description .


###  http://purl.org/dc/terms/accessRights
dcterms:accessRights rdf:type owl:AnnotationProperty ;
                   rdfs:subPropertyOf dc:rights ;
                   rdfs:range dcterms:RightsStatement .


###  http://purl.org/dc/terms/alternative
dcterms:alternative rdf:type owl:AnnotationProperty ;
                  rdfs:subPropertyOf dc:title ;
                  rdfs:range rdfs:Literal .


###  http://purl.org/dc/terms/available
dcterms:available rdf:type owl:AnnotationProperty ;
                rdfs:subPropertyOf dc:date ;
                rdfs:range rdfs:Literal .


###  http://purl.org/dc/terms/bibliographicCitation
dcterms:bibliographicCitation rdf:type owl:AnnotationProperty ;
                            rdfs:subPropertyOf dc:identifier ;
                            rdfs:range rdfs:Literal ;
                            rdfs:domain dcterms:BibliographicResource .


###  http://purl.org/dc/terms/conformsTo
dcterms:conformsTo rdf:type owl:AnnotationProperty ;
                 rdfs:subPropertyOf dc:relation ,
                                    dcterms:relation ;
                 rdfs:range dcterms:Standard .


###  http://purl.org/dc/terms/contributor
dcterms:contributor rdf:type owl:AnnotationProperty ;
                  rdfs:subPropertyOf dc:contributor ;
                  rdfs:range dcterms:Agent .


###  http://purl.org/dc/terms/coverage
dcterms:coverage rdf:type owl:AnnotationProperty ;
               rdfs:subPropertyOf dc:coverage ;
               rdfs:range dcterms:LocationPeriodOrJurisdiction .


###  http://purl.org/dc/terms/created
dcterms:created rdf:type owl:AnnotationProperty ;
              rdfs:subPropertyOf dc:date ;
              rdfs:range rdfs:Literal .


###  http://purl.org/dc/terms/creator
dcterms:creator rdf:type owl:AnnotationProperty ;
              rdfs:subPropertyOf dc:creator ;
              rdfs:range dcterms:Agent .


###  http://purl.org/dc/terms/date
dcterms:date rdf:type owl:AnnotationProperty ;
           rdfs:subPropertyOf dc:date ;
           rdfs:range rdfs:Literal .


###  http://purl.org/dc/terms/dateAccepted
dcterms:dateAccepted rdf:type owl:AnnotationProperty ;
                   rdfs:subPropertyOf dc:date ;
                   rdfs:range rdfs:Literal .


###  http://purl.org/dc/terms/dateCopyrighted
dcterms:dateCopyrighted rdf:type owl:AnnotationProperty ;
                      rdfs:subPropertyOf dc:date ;
                      rdfs:range rdfs:Literal .


###  http://purl.org/dc/terms/dateSubmitted
dcterms:dateSubmitted rdf:type owl:AnnotationProperty ;
                    rdfs:subPropertyOf dc:date ;
                    rdfs:range rdfs:Literal .


###  http://purl.org/dc/terms/description
dcterms:description rdf:type owl:AnnotationProperty ;
                  rdfs:subPropertyOf dc:description .


###  http://purl.org/dc/terms/extent
dcterms:extent rdf:type owl:AnnotationProperty ;
             rdfs:subPropertyOf dc:format ;
             rdfs:range dcterms:SizeOrDuration .


###  http://purl.org/dc/terms/format
dcterms:format rdf:type owl:AnnotationProperty ;
             rdfs:subPropertyOf dc:format ;
             rdfs:range dcterms:MediaTypeOrExtent .


###  http://purl.org/dc/terms/hasFormat
dcterms:hasFormat rdf:type owl:AnnotationProperty ;
                rdfs:subPropertyOf dc:relation ,
                                   dcterms:relation .


###  http://purl.org/dc/terms/hasPart
dcterms:hasPart rdf:type owl:AnnotationProperty ;
              rdfs:subPropertyOf dc:relation ,
                                 dcterms:relation .


###  http://purl.org/dc/terms/hasVersion
dcterms:hasVersion rdf:type owl:AnnotationProperty ;
                 rdfs:subPropertyOf dc:relation ,
                                    dcterms:relation .


###  http://purl.org/dc/terms/identifier
dcterms:identifier rdf:type owl:AnnotationProperty ;
                 rdfs:subPropertyOf dc:identifier ;
                 rdfs:range rdfs:Literal .


###  http://purl.org/dc/terms/isFormatOf
dcterms:isFormatOf rdf:type owl:AnnotationProperty ;
                 rdfs:subPropertyOf dc:relation ,
                                    dcterms:relation .


###  http://purl.org/dc/terms/isPartOf
dcterms:isPartOf rdf:type owl:AnnotationProperty ;
               rdfs:subPropertyOf dc:relation ,
                                  dcterms:relation .


###  http://purl.org/dc/terms/isReferencedBy
dcterms:isReferencedBy rdf:type owl:AnnotationProperty ;
                     rdfs:subPropertyOf dc:relation ,
                                        dcterms:relation .


###  http://purl.org/dc/terms/isReplacedBy
dcterms:isReplacedBy rdf:type owl:AnnotationProperty ;
                   rdfs:subPropertyOf dc:relation ,
                                      dcterms:relation .


###  http://purl.org/dc/terms/isRequiredBy
dcterms:isRequiredBy rdf:type owl:AnnotationProperty ;
                   rdfs:subPropertyOf dc:relation ,
                                      dcterms:relation .


###  http://purl.org/dc/terms/isVersionOf
dcterms:isVersionOf rdf:type owl:AnnotationProperty ;
                  rdfs:subPropertyOf dc:relation ,
                                     dcterms:relation .


###  http://purl.org/dc/terms/issued
dcterms:issued rdf:type owl:AnnotationProperty ;
             rdfs:subPropertyOf dc:date ;
             rdfs:range rdfs:Literal .


###  http://purl.org/dc/terms/language
dcterms:language rdf:type owl:AnnotationProperty ;
               rdfs:subPropertyOf dc:language ;
               rdfs:range dcterms:LinguisticSystem .


###  http://purl.org/dc/terms/license
dcterms:license rdf:type owl:AnnotationProperty ;
              rdfs:subPropertyOf dc:rights ;
              rdfs:range dcterms:LicenseDocument .


###  http://purl.org/dc/terms/medium
dcterms:medium rdf:type owl:AnnotationProperty ;
             rdfs:subPropertyOf dc:format ;
             rdfs:range dcterms:PhysicalMedium .


###  http://purl.org/dc/terms/modified
dcterms:modified rdf:type owl:AnnotationProperty ;
               rdfs:subPropertyOf dc:date ;
               rdfs:range rdfs:Literal .


###  http://purl.org/dc/terms/publisher
dcterms:publisher rdf:type owl:AnnotationProperty ;
                rdfs:subPropertyOf dc:publisher ;
                rdfs:range dcterms:Agent .


###  http://purl.org/dc/terms/references
dcterms:references rdf:type owl:AnnotationProperty ;
                 rdfs:subPropertyOf dc:relation ,
                                    dcterms:relation .


###  http://purl.org/dc/terms/relation
dcterms:relation rdf:type owl:AnnotationProperty ;
               rdfs:subPropertyOf dc:relation .


###  http://purl.org/dc/terms/replaces
dcterms:replaces rdf:type owl:AnnotationProperty ;
               rdfs:subPropertyOf dc:relation ,
                                  dcterms:relation .


###  http://purl.org/dc/terms/requires
dcterms:requires rdf:type owl:AnnotationProperty ;
               rdfs:subPropertyOf dc:relation ,
                                  dcterms:relation .


###  http://purl.org/dc/terms/rights
dcterms:rights rdf:type owl:AnnotationProperty ;
             rdfs:subPropertyOf dc:rights ;
             rdfs:range dcterms:RightsStatement .


###  http://purl.org/dc/terms/source
dcterms:source rdf:type owl:AnnotationProperty ;
             rdfs:subPropertyOf dc:source ,
                                dcterms:relation .


###  http://purl.org/dc/terms/spatial
dcterms:spatial rdf:type owl:AnnotationProperty ;
              rdfs:subPropertyOf dc:coverage ;
              rdfs:range dcterms:Location .


###  http://purl.org/dc/terms/subject
dcterms:subject rdf:type owl:AnnotationProperty ;
              rdfs:subPropertyOf dc:subject .


###  http://purl.org/dc/terms/tableOfContents
dcterms:tableOfContents rdf:type owl:AnnotationProperty ;
                      rdfs:subPropertyOf dc:description ,
                                         dcterms:description .


###  http://purl.org/dc/terms/temporal
dcterms:temporal rdf:type owl:AnnotationProperty ;
               rdfs:subPropertyOf dc:coverage ;
               rdfs:range dcterms:PeriodOfTime .


###  http://purl.org/dc/terms/title
dcterms:title rdf:type owl:AnnotationProperty ;
            rdfs:subPropertyOf dc:title ;
            rdfs:range rdfs:Literal .


###  http://purl.org/dc/terms/type
dcterms:type rdf:type owl:AnnotationProperty ;
           rdfs:subPropertyOf dc:type ;
           rdfs:range rdfs:Class .


###  http://purl.org/dc/terms/valid
dcterms:valid rdf:type owl:AnnotationProperty ;
            rdfs:subPropertyOf dc:date ;
            rdfs:range rdfs:Literal .


###  http://www.w3.org/2004/02/skos/core#example
skos:example rdf:type owl:AnnotationProperty .


###  http://www.w3.org/2004/02/skos/core#note
skos:note rdf:type owl:AnnotationProperty .


#################################################################
#    Datatypes
#################################################################

###  http://purl.org/dc/terms/Box
dcterms:Box rdf:type rdfs:Datatype .


###  http://purl.org/dc/terms/ISO3166
dcterms:ISO3166 rdf:type rdfs:Datatype .


###  http://purl.org/dc/terms/ISO639-2
dcterms:ISO639-2 rdf:type rdfs:Datatype .


###  http://purl.org/dc/terms/ISO639-3
dcterms:ISO639-3 rdf:type rdfs:Datatype .


###  http://purl.org/dc/terms/Period
dcterms:Period rdf:type rdfs:Datatype .


###  http://purl.org/dc/terms/Point
dcterms:Point rdf:type rdfs:Datatype .


###  http://purl.org/dc/terms/RFC1766
dcterms:RFC1766 rdf:type rdfs:Datatype .


###  http://purl.org/dc/terms/RFC3066
dcterms:RFC3066 rdf:type rdfs:Datatype .


###  http://purl.org/dc/terms/RFC4646
dcterms:RFC4646 rdf:type rdfs:Datatype .


###  http://purl.org/dc/terms/RFC5646
dcterms:RFC5646 rdf:type rdfs:Datatype .


###  http://purl.org/dc/terms/URI
dcterms:URI rdf:type rdfs:Datatype .


###  http://purl.org/dc/terms/W3CDTF
dcterms:W3CDTF rdf:type rdfs:Datatype .


###  http://www.w3.org/2001/XMLSchema#date
xsd:date rdf:type rdfs:Datatype .


#################################################################
#    Object Properties
#################################################################

###  http://purl.org/dc/terms/accessRights
dcterms:accessRights rdf:type owl:ObjectProperty ;
                   rdfs:subPropertyOf dcterms:rights .


###  http://purl.org/dc/terms/accrualMethod
dcterms:accrualMethod rdf:type owl:ObjectProperty ;
                    rdfs:domain <http://purl.org/dc/dcmitype/Collection> ;
                    rdfs:range dcterms:MethodOfAccrual .


###  http://purl.org/dc/terms/accrualPeriodicity
dcterms:accrualPeriodicity rdf:type owl:ObjectProperty ;
                         rdfs:domain <http://purl.org/dc/dcmitype/Collection> ;
                         rdfs:range dcterms:Frequency .


###  http://purl.org/dc/terms/accrualPolicy
dcterms:accrualPolicy rdf:type owl:ObjectProperty ;
                    rdfs:domain <http://purl.org/dc/dcmitype/Collection> ;
                    rdfs:range dcterms:Policy .


###  http://purl.org/dc/terms/audience
dcterms:audience rdf:type owl:ObjectProperty ;
               rdfs:range dcterms:AgentClass .


###  http://purl.org/dc/terms/conformsTo
dcterms:conformsTo rdf:type owl:ObjectProperty .


###  http://purl.org/dc/terms/contributor
dcterms:contributor rdf:type owl:ObjectProperty .


###  http://purl.org/dc/terms/coverage
dcterms:coverage rdf:type owl:ObjectProperty .


###  http://purl.org/dc/terms/creator
dcterms:creator rdf:type owl:ObjectProperty ;
              rdfs:subPropertyOf dcterms:contributor .


###  http://purl.org/dc/terms/educationLevel
dcterms:educationLevel rdf:type owl:ObjectProperty ;
                     rdfs:subPropertyOf dcterms:audience ;
                     rdfs:range dcterms:AgentClass .


###  http://purl.org/dc/terms/extent
dcterms:extent rdf:type owl:ObjectProperty ;
             rdfs:subPropertyOf dcterms:format .


###  http://purl.org/dc/terms/format
dcterms:format rdf:type owl:ObjectProperty .


###  http://purl.org/dc/terms/instructionalMethod
dcterms:instructionalMethod rdf:type owl:ObjectProperty ;
                          rdfs:range dcterms:MethodOfInstruction .


###  http://purl.org/dc/terms/language
dcterms:language rdf:type owl:ObjectProperty .


###  http://purl.org/dc/terms/license
dcterms:license rdf:type owl:ObjectProperty ;
              rdfs:subPropertyOf dcterms:rights .


###  http://purl.org/dc/terms/mediator
dcterms:mediator rdf:type owl:ObjectProperty ;
               rdfs:subPropertyOf dcterms:audience ;
               rdfs:range dcterms:AgentClass .


###  http://purl.org/dc/terms/medium
dcterms:medium rdf:type owl:ObjectProperty ;
             rdfs:subPropertyOf dcterms:format ;
             rdfs:domain dcterms:PhysicalResource .


###  http://purl.org/dc/terms/provenance
dcterms:provenance rdf:type owl:ObjectProperty ;
                 rdfs:range dcterms:ProvenanceStatement .


###  http://purl.org/dc/terms/publisher
dcterms:publisher rdf:type owl:ObjectProperty .


###  http://purl.org/dc/terms/rights
dcterms:rights rdf:type owl:ObjectProperty .


###  http://purl.org/dc/terms/rightsHolder
dcterms:rightsHolder rdf:type owl:ObjectProperty ;
                   rdfs:range dcterms:Agent .


###  http://purl.org/dc/terms/spatial
dcterms:spatial rdf:type owl:ObjectProperty ;
              rdfs:subPropertyOf dcterms:coverage .


###  http://purl.org/dc/terms/temporal
dcterms:temporal rdf:type owl:ObjectProperty ;
               rdfs:subPropertyOf dcterms:coverage .


###  http://purl.org/dc/terms/type
dcterms:type rdf:type owl:ObjectProperty .


###  http://reference.data.gov.au/def/ont/agrif#accessedBy
:accessedBy rdf:type owl:ObjectProperty ;
            rdfs:subPropertyOf :wasAssociatedWith ;
            rdfs:comment "A relation that indicates that an Agent has accessed a Record as defined in an Access Activity."@en ;
            rdfs:label "accessed By"@en .


###  http://reference.data.gov.au/def/ont/agrif#actsAs
:actsAs rdf:type owl:ObjectProperty ;
        rdfs:comment "A relation between an Agent and the Role that Agent acts in."@en ;
        rdfs:label "acts As"@en .


###  http://reference.data.gov.au/def/ont/agrif#associatedFunction
:associatedFunction rdf:type owl:ObjectProperty ;
                    rdfs:comment "A relation that associates a Function to an Entity, Event or Activity."@en ;
                    rdfs:label "associated Function"@en .


###  http://reference.data.gov.au/def/ont/agrif#associatedRole
:associatedRole rdf:type owl:ObjectProperty ;
                dc:source "https://www.w3.org/TR/prov-o/#hadRole" ;
                rdfs:comment "An associated Role is a qualified association between a Role and an Activity or Event defined by an Association."@en ;
                rdfs:label "associated Role"@en .


###  http://reference.data.gov.au/def/ont/agrif#guidingPolicy
:guidingPolicy rdf:type owl:ObjectProperty ;
               rdfs:comment "A relation that defines a Policy that is guiding an Activity or Change Event."@en ;
               rdfs:label "guiding Policy"@en .


###  http://reference.data.gov.au/def/ont/agrif#hasActivity
:hasActivity rdf:type owl:ObjectProperty ;
             owl:inverseOf :usedRecord ;
             dc:source "https://www.w3.org/TR/prov-o/#p_activity" ;
             rdfs:comment "A relation between a Record and an Activity that acts upon the Record."@en ;
             rdfs:label "has Activity"@en .


###  http://reference.data.gov.au/def/ont/agrif#hasAgent
:hasAgent rdf:type owl:ObjectProperty ;
          dc:source "https://www.w3.org/TR/prov-o/#p_agent" ;
          rdfs:comment "A qualified relation between an Agent and a Change Event defined through an Association."@en ;
          rdfs:label "has Agent"@en .


###  http://reference.data.gov.au/def/ont/agrif#hasClassifier
:hasClassifier rdf:type owl:ObjectProperty ;
               rdfs:subPropertyOf owl:topObjectProperty ;
               rdfs:label "has Classifier"@en ;
               owl:deprecated ""@en .


###  http://reference.data.gov.au/def/ont/agrif#hasControl
:hasControl rdf:type owl:ObjectProperty ;
            rdfs:comment "A relation between a Record, Artefact or Event and a Control that denotes the required level of Access or Security Control." ;
            rdfs:label "requires Control"@en .


###  http://reference.data.gov.au/def/ont/agrif#hasCoverage
:hasCoverage rdf:type owl:ObjectProperty ;
             rdfs:comment "A relation between a Record and its Jurisdictional Coverage, or its Temporal or Spatial Coverage."@en ;
             rdfs:label "has Coverage"@en .


###  http://reference.data.gov.au/def/ont/agrif#hasDecisionStatus
:hasDecisionStatus rdf:type owl:ObjectProperty ;
                   rdfs:comment "A relation that indicates what the Decision on a Decision Event was."@en ;
                   rdfs:label "has Decision Status"@en .


###  http://reference.data.gov.au/def/ont/agrif#hasDisposalClass
:hasDisposalClass rdf:type owl:ObjectProperty ;
                  rdfs:comment "A relation that associates a Disposal Class with a Record."@en ;
                  rdfs:label "has Disposal Class"@en .


###  http://reference.data.gov.au/def/ont/agrif#hasFormFactor
:hasFormFactor rdf:type owl:ObjectProperty ;
               rdfs:comment "A relation that defines the size, shape, and other physical specifications of a Physical Artefact."@en ;
               rdfs:label "has Form Factor"@en .


###  http://reference.data.gov.au/def/ont/agrif#hasLocation
:hasLocation rdf:type owl:ObjectProperty ;
             rdfs:comment "A relation that defines the Spatial Location of an Activity or Artefact."@en ;
             rdfs:label "has Location"@en .


###  http://reference.data.gov.au/def/ont/agrif#hasManifest
:hasManifest rdf:type owl:ObjectProperty ;
             rdfs:comment "A relation between a Manifest and a Transfer Event that describes the files involved in the transfer of a Record."@en ;
             rdfs:label "has Manifest"@en .


###  http://reference.data.gov.au/def/ont/agrif#hasPart
:hasPart rdf:type owl:ObjectProperty ;
         owl:inverseOf :partOf ;
         rdfs:comment "A relation that defines part-whole relations amongst Organisational Units."@en ;
         rdfs:label "has Part"@en .


###  http://reference.data.gov.au/def/ont/agrif#hasPermission
:hasPermission rdf:type owl:ObjectProperty ;
               rdfs:comment "A relation between an Agent and the Permission the Agent possesses."@en ;
               rdfs:label "has Permission"@en .


###  http://reference.data.gov.au/def/ont/agrif#hasPrerequisiteDecisionEvent
:hasPrerequisiteDecisionEvent rdf:type owl:ObjectProperty ;
                              rdfs:comment "A relation between a Decision Event and a prerequisite Decision Event, indicating a Decision chain in a Chain of Command."@en ;
                              rdfs:label "has Prerequisite Decision Event"@en .


###  http://reference.data.gov.au/def/ont/agrif#hasQuality
:hasQuality rdf:type owl:ObjectProperty ;
            rdfs:comment "A relation that indicates a specific Quality of an Artefact."@en ;
            rdfs:label "has Quality"@en .


###  http://reference.data.gov.au/def/ont/agrif#hasSeries
:hasSeries rdf:type owl:ObjectProperty ;
           rdfs:subPropertyOf owl:topObjectProperty ;
           rdfs:comment "A relation between a Record and its Series Number."@en ;
           rdfs:label "has Series"@en .


###  http://reference.data.gov.au/def/ont/agrif#hasStatus
:hasStatus rdf:type owl:ObjectProperty ;
           rdfs:comment "A relation between an Activity and a Status that indicates its current state."@en ;
           rdfs:label "has Status"@en .


###  http://reference.data.gov.au/def/ont/agrif#hasVersionHistory
:hasVersionHistory rdf:type owl:ObjectProperty ;
                   rdfs:comment "A relation between a Record and its previous Version qualified through a Replace Event."@en ;
                   rdfs:label "has Version History"@en .


###  http://reference.data.gov.au/def/ont/agrif#isChangedBy
:isChangedBy rdf:type owl:ObjectProperty ;
             rdfs:subPropertyOf owl:topObjectProperty ;
             rdfs:comment "A relation between an Artefact or a Record and a Change Event."@en ;
             rdfs:label "is Changed By"@en .


###  http://reference.data.gov.au/def/ont/agrif#notifies
:notifies rdf:type owl:ObjectProperty ;
          rdfs:comment "A relation between a Trigger and an Agent that is to be notified."@en ;
          rdfs:label "notifies"@en .


###  http://reference.data.gov.au/def/ont/agrif#partOf
:partOf rdf:type owl:ObjectProperty ,
                 owl:TransitiveProperty ;
        rdfs:comment "A relation that defines part-whole relations amongst Organisational Units."@en ;
        rdfs:label "part Of"@en .


###  http://reference.data.gov.au/def/ont/agrif#positionIn
:positionIn rdf:type owl:ObjectProperty ;
            rdfs:comment "A relation that defines the position an Agent occupies in an Organisation or Organisational Unit."@en ;
            rdfs:label "position In"@en .


###  http://reference.data.gov.au/def/ont/agrif#qualifiedAssociation
:qualifiedAssociation rdf:type owl:ObjectProperty ;
                      rdfs:comment "A relation that associates an assignment of responsibility to an Agent for an Activity or Event, indicating that the Agent had a Role in the Activity or Event."@en ;
                      rdfs:label "qualified Association"@en .


###  http://reference.data.gov.au/def/ont/agrif#recordOf
:recordOf rdf:type owl:ObjectProperty ;
          rdfs:comment "A relation that defines what Artefact the Record is about."@en ;
          rdfs:label "record Of"@en .


###  http://reference.data.gov.au/def/ont/agrif#relatedTo
:relatedTo rdf:type owl:ObjectProperty ;
           rdfs:comment "A relation that indicates that there is some form of relation between a Record and another Record or between an Artefact and another Artefact."@en ;
           rdfs:label "related To"@en .


###  http://reference.data.gov.au/def/ont/agrif#replacedBy
:replacedBy rdf:type owl:ObjectProperty ;
            owl:inverseOf :replaces ;
            rdfs:comment "A relation that defines that a Record has been replaced by another Record, qualified through a Replace Event."@en ;
            rdfs:label "replaced By"@en .


###  http://reference.data.gov.au/def/ont/agrif#replaces
:replaces rdf:type owl:ObjectProperty ;
          rdfs:comment "A relation that defines that a Record replaces another Record, qualified through a Replace Event."@en ;
          rdfs:label "replaces"@en .


###  http://reference.data.gov.au/def/ont/agrif#requiresSecurityClassification
:requiresSecurityClassification rdf:type owl:ObjectProperty ;
                                rdfs:subPropertyOf :hasControl ;
                                rdfs:comment "A relation between a Record and a Security Classification that denotes the required level of Security Clearance an Agent needs to possess to access the Record."@en ;
                                rdfs:label "requires Security Classification"@en .


###  http://reference.data.gov.au/def/ont/agrif#sharedWith
:sharedWith rdf:type owl:ObjectProperty ;
            rdfs:subPropertyOf :wasAssociatedWith ;
            rdfs:comment "A relation that indicates that a Record was shared with an Agent as defined in a Share Activity."@en ;
            rdfs:label "shared With"@en .


###  http://reference.data.gov.au/def/ont/agrif#storedIn
:storedIn rdf:type owl:ObjectProperty ;
          rdfs:subPropertyOf owl:topObjectProperty ;
          rdfs:comment "A relation that indicates the Storage Location of an Artefact."@en ;
          rdfs:label "stored In"@en .


###  http://reference.data.gov.au/def/ont/agrif#transferredFrom
:transferredFrom rdf:type owl:ObjectProperty ;
                 rdfs:comment "A relation that defines that the Control of a Record has been transferred from that Role."@en ;
                 rdfs:label "transferred From"@en .


###  http://reference.data.gov.au/def/ont/agrif#transferredTo
:transferredTo rdf:type owl:ObjectProperty ;
               rdfs:comment "A relation that defines that the Control of a Record has been transferred to that new Role."@en ;
               rdfs:label "transferred To"@en .


###  http://reference.data.gov.au/def/ont/agrif#triggeredBy
:triggeredBy rdf:type owl:ObjectProperty ;
             rdfs:comment "A relation that indicates that a Change Event has been initiated by a Trigger."@en ;
             rdfs:label "triggered By"@en .


###  http://reference.data.gov.au/def/ont/agrif#triggers
:triggers rdf:type owl:ObjectProperty ;
          rdfs:comment "A relation that indicates that a Trigger has initiated a Change Event."@en ;
          rdfs:label "triggers"@en .


###  http://reference.data.gov.au/def/ont/agrif#usedRecord
:usedRecord rdf:type owl:ObjectProperty ;
            rdfs:comment "A relation between an Activity and a Record the Activity uses."@en ;
            rdfs:label "used Record"@en .


###  http://reference.data.gov.au/def/ont/agrif#wasAssociatedWith
:wasAssociatedWith rdf:type owl:ObjectProperty ;
                   dc:source "https://www.w3.org/TR/prov-o/#wasAssociatedWith" ;
                   rdfs:comment "A relation that assigns responsibility of an Agent for an Activity or Change Event."@en ;
                   rdfs:label "was Associated With"@en .


#################################################################
#    Data properties
#################################################################

###  http://purl.org/dc/terms/alternative
dcterms:alternative rdf:type owl:DatatypeProperty ;
                  rdfs:subPropertyOf dcterms:title .


###  http://purl.org/dc/terms/available
dcterms:available rdf:type owl:DatatypeProperty ;
                rdfs:subPropertyOf dcterms:date .


###  http://purl.org/dc/terms/bibliographicCitation
dcterms:bibliographicCitation rdf:type owl:DatatypeProperty ;
                            rdfs:subPropertyOf dcterms:identifier .


###  http://purl.org/dc/terms/created
dcterms:created rdf:type owl:DatatypeProperty ;
              rdfs:subPropertyOf dcterms:date .


###  http://purl.org/dc/terms/date
dcterms:date rdf:type owl:DatatypeProperty .


###  http://purl.org/dc/terms/dateAccepted
dcterms:dateAccepted rdf:type owl:DatatypeProperty ;
                   rdfs:subPropertyOf dcterms:date .


###  http://purl.org/dc/terms/dateCopyrighted
dcterms:dateCopyrighted rdf:type owl:DatatypeProperty ;
                      rdfs:subPropertyOf dcterms:date .


###  http://purl.org/dc/terms/dateSubmitted
dcterms:dateSubmitted rdf:type owl:DatatypeProperty ;
                    rdfs:subPropertyOf dcterms:date .


###  http://purl.org/dc/terms/identifier
dcterms:identifier rdf:type owl:DatatypeProperty .


###  http://purl.org/dc/terms/issued
dcterms:issued rdf:type owl:DatatypeProperty ;
             rdfs:subPropertyOf dcterms:date .


###  http://purl.org/dc/terms/modified
dcterms:modified rdf:type owl:DatatypeProperty ;
               rdfs:subPropertyOf dcterms:date .


###  http://purl.org/dc/terms/title
dcterms:title rdf:type owl:DatatypeProperty .


###  http://purl.org/dc/terms/valid
dcterms:valid rdf:type owl:DatatypeProperty ;
            rdfs:subPropertyOf dcterms:date .


###  http://reference.data.gov.au/def/ont/agrif#atTime
:atTime rdf:type owl:DatatypeProperty ;
        rdfs:range xsd:dateTime ;
        dc:source "https://www.w3.org/TR/prov-o/#atTime" ;
        rdfs:comment "The time at which an Event occurred, in the form of xsd:dateTime."@en .


###  http://reference.data.gov.au/def/ont/agrif#checksum
:checksum rdf:type owl:DatatypeProperty ;
          rdfs:range xsd:float ;
          dc:source "A checksum is a small-sized datum derived from a block of digital data representing a Record for the purpose of detecting errors during the transfer or storage of a Record."@en .


###  http://reference.data.gov.au/def/ont/agrif#disposalClassNumber
:disposalClassNumber rdf:type owl:DatatypeProperty ;
                     rdfs:range xsd:integer ;
                     rdfs:comment "The number defining the sentencing requirements of a Record."@en .


###  http://reference.data.gov.au/def/ont/agrif#endedAtTime
:endedAtTime rdf:type owl:DatatypeProperty ;
             rdfs:range xsd:dateTime ;
             dc:source "https://www.w3.org/TR/prov-o/#endedAtTime" ;
             rdfs:comment "The time at which an Activity ended."@en .


###  http://reference.data.gov.au/def/ont/agrif#filename
:filename rdf:type owl:DatatypeProperty ;
          rdfs:comment "A filename is a name used to uniquely identify a computer file stored in a file system." .


###  http://reference.data.gov.au/def/ont/agrif#filesize
:filesize rdf:type owl:DatatypeProperty ;
          rdfs:comment "File size is a measure of how much data a computer file contains or how much storage it consumes."@en .


###  http://reference.data.gov.au/def/ont/agrif#format
:format rdf:type owl:DatatypeProperty ;
        dc:source "http://purl.org/dc/elements/1.1/format" ;
        rdfs:comment "The file format, physical medium, or dimensions of the resource."@en .


###  http://reference.data.gov.au/def/ont/agrif#seriesNumber
:seriesNumber rdf:type owl:DatatypeProperty ;
              rdfs:range xsd:integer ;
              rdfs:comment "A seriesNumber is a numerical identifier for a Series."@en .


###  http://reference.data.gov.au/def/ont/agrif#startedAtTime
:startedAtTime rdf:type owl:DatatypeProperty ;
               rdfs:range xsd:dateTime ;
               dc:source "https://www.w3.org/TR/prov-o/#startedAtTime" ;
               rdfs:comment "The time at which an Activity started."@en .


#################################################################
#    Classes
#################################################################

###  http://purl.org/dc/dcam/VocabularyEncodingScheme
<http://purl.org/dc/dcam/VocabularyEncodingScheme> rdf:type owl:Class .


###  http://purl.org/dc/dcmitype/Collection
<http://purl.org/dc/dcmitype/Collection> rdf:type owl:Class .


###  http://purl.org/dc/terms/Agent
dcterms:Agent rdf:type owl:Class .


###  http://purl.org/dc/terms/AgentClass
dcterms:AgentClass rdf:type owl:Class ;
                 rdfs:subClassOf rdfs:Class .


###  http://purl.org/dc/terms/BibliographicResource
dcterms:BibliographicResource rdf:type owl:Class .


###  http://purl.org/dc/terms/FileFormat
dcterms:FileFormat rdf:type owl:Class ;
                 rdfs:subClassOf dcterms:MediaType .


###  http://purl.org/dc/terms/Frequency
dcterms:Frequency rdf:type owl:Class .


###  http://purl.org/dc/terms/Jurisdiction
dcterms:Jurisdiction rdf:type owl:Class ;
                   rdfs:subClassOf dcterms:LocationPeriodOrJurisdiction .


###  http://purl.org/dc/terms/LicenseDocument
dcterms:LicenseDocument rdf:type owl:Class ;
                      rdfs:subClassOf dcterms:RightsStatement .


###  http://purl.org/dc/terms/LinguisticSystem
dcterms:LinguisticSystem rdf:type owl:Class .


###  http://purl.org/dc/terms/Location
dcterms:Location rdf:type owl:Class ;
               rdfs:subClassOf dcterms:LocationPeriodOrJurisdiction .


###  http://purl.org/dc/terms/LocationPeriodOrJurisdiction
dcterms:LocationPeriodOrJurisdiction rdf:type owl:Class .


###  http://purl.org/dc/terms/MediaType
dcterms:MediaType rdf:type owl:Class ;
                rdfs:subClassOf dcterms:MediaTypeOrExtent .


###  http://purl.org/dc/terms/MediaTypeOrExtent
dcterms:MediaTypeOrExtent rdf:type owl:Class .


###  http://purl.org/dc/terms/MethodOfAccrual
dcterms:MethodOfAccrual rdf:type owl:Class .


###  http://purl.org/dc/terms/MethodOfInstruction
dcterms:MethodOfInstruction rdf:type owl:Class .


###  http://purl.org/dc/terms/PeriodOfTime
dcterms:PeriodOfTime rdf:type owl:Class ;
                   rdfs:subClassOf dcterms:LocationPeriodOrJurisdiction .


###  http://purl.org/dc/terms/PhysicalMedium
dcterms:PhysicalMedium rdf:type owl:Class ;
                     rdfs:subClassOf dcterms:MediaType .


###  http://purl.org/dc/terms/PhysicalResource
dcterms:PhysicalResource rdf:type owl:Class .


###  http://purl.org/dc/terms/Policy
dcterms:Policy rdf:type owl:Class .


###  http://purl.org/dc/terms/ProvenanceStatement
dcterms:ProvenanceStatement rdf:type owl:Class .


###  http://purl.org/dc/terms/RightsStatement
dcterms:RightsStatement rdf:type owl:Class .


###  http://purl.org/dc/terms/SizeOrDuration
dcterms:SizeOrDuration rdf:type owl:Class ;
                     rdfs:subClassOf dcterms:MediaTypeOrExtent .


###  http://purl.org/dc/terms/Standard
dcterms:Standard rdf:type owl:Class .


###  http://reference.data.gov.au/def/ont/agrif#AGIFTFunction
:AGIFTFunction rdf:type owl:Class ;
               rdfs:subClassOf :Function ;
               rdfs:comment "An AGIFT Function is a Function that classifies a Record according to the Australian Governments' Interactive Functions Thesaurus."@en ;
               rdfs:isDefinedBy "https://data.naa.gov.au/def/agift/"@en ;
               rdfs:label "AGIFT Function"@en .


###  http://reference.data.gov.au/def/ont/agrif#AccessActivity
:AccessActivity rdf:type owl:Class ;
                rdfs:subClassOf :Activity ,
                                [ rdf:type owl:Restriction ;
                                  owl:onProperty :accessedBy ;
                                  owl:someValuesFrom :Agent
                                ] ,
                                [ rdf:type owl:Restriction ;
                                  owl:onProperty :triggers ;
                                  owl:someValuesFrom :AccessTrigger
                                ] ;
                rdfs:comment "An Access Activity is an Activity where a Record is accessed by an Agent over a period of time."@en ;
                rdfs:label "Access Activity"@en .


###  http://reference.data.gov.au/def/ont/agrif#AccessControl
:AccessControl rdf:type owl:Class ;
               rdfs:subClassOf :Control ;
               rdfs:comment "Access Control is the selective restriction of access to a Record or Artefact."@en ;
               rdfs:label "Access Control"@en .


###  http://reference.data.gov.au/def/ont/agrif#AccessTrigger
:AccessTrigger rdf:type owl:Class ;
               rdfs:subClassOf :Trigger ;
               rdfs:comment "An Access Trigger is a Trigger that can be initiated when a Record is accessed."@en ;
               rdfs:label "Access Trigger"@en .


###  http://reference.data.gov.au/def/ont/agrif#Activity
:Activity rdf:type owl:Class ;
          rdfs:subClassOf [ rdf:type owl:Restriction ;
                            owl:onProperty :qualifiedAssociation ;
                            owl:someValuesFrom :Association
                          ] ,
                          [ rdf:type owl:Restriction ;
                            owl:onProperty :wasAssociatedWith ;
                            owl:someValuesFrom :Agent
                          ] ,
                          [ rdf:type owl:Restriction ;
                            owl:onProperty :associatedFunction ;
                            owl:allValuesFrom :Function
                          ] ,
                          [ rdf:type owl:Restriction ;
                            owl:onProperty :guidingPolicy ;
                            owl:allValuesFrom :Policy
                          ] ,
                          [ rdf:type owl:Restriction ;
                            owl:onProperty :hasLocation ;
                            owl:allValuesFrom :SpatialLocation
                          ] ,
                          [ rdf:type owl:Restriction ;
                            owl:onProperty :hasStatus ;
                            owl:allValuesFrom :Status
                          ] ,
                          [ rdf:type owl:Restriction ;
                            owl:onProperty :requiresSecurityClassification ;
                            owl:allValuesFrom :SecurityClassification
                          ] ,
                          [ rdf:type owl:Restriction ;
                            owl:onProperty :usedRecord ;
                            owl:allValuesFrom :Record
                          ] ,
                          [ rdf:type owl:Restriction ;
                            owl:onProperty :startedAtTime ;
                            owl:qualifiedCardinality "1"^^xsd:nonNegativeInteger ;
                            owl:onDataRange xsd:dateTime
                          ] ,
                          [ rdf:type owl:Restriction ;
                            owl:onProperty :endedAtTime ;
                            owl:maxQualifiedCardinality "1"^^xsd:nonNegativeInteger ;
                            owl:onDataRange xsd:dateTime
                          ] ;
          dc:source "https://www.w3.org/TR/prov-o/#Activity" ;
          rdfs:comment "An Activity is something that occurs over a period of time on a Record."@en ;
          rdfs:label "Activity"@en .


###  http://reference.data.gov.au/def/ont/agrif#Administrator
:Administrator rdf:type owl:Class ;
               rdfs:subClassOf :Role ;
               rdfs:comment "An Administrator is a Role that has overall responsibility for the administration and functions of an Information System, but not necessarily for the information stored within."@en ;
               rdfs:label "Administrator"@en .


###  http://reference.data.gov.au/def/ont/agrif#Agent
:Agent rdf:type owl:Class ;
       rdfs:subClassOf [ rdf:type owl:Restriction ;
                         owl:onProperty :actsAs ;
                         owl:someValuesFrom :Role
                       ] ,
                       [ rdf:type owl:Restriction ;
                         owl:onProperty :hasPermission ;
                         owl:someValuesFrom :Permission
                       ] ,
                       [ rdf:type owl:Restriction ;
                         owl:onProperty :positionIn ;
                         owl:someValuesFrom :Organisation
                       ] ;
       dc:source "https://www.w3.org/TR/prov-o/#Agent" ;
       rdfs:comment "An Agent is a corporate entity, organisational element or system, or individual responsible for the performance of some Activity or Event, including those on Records."@en ;
       rdfs:label "Agent"@en .


###  http://reference.data.gov.au/def/ont/agrif#Artefact
:Artefact rdf:type owl:Class ;
          rdfs:subClassOf [ rdf:type owl:Restriction ;
                            owl:onProperty :hasControl ;
                            owl:someValuesFrom :Control
                          ] ,
                          [ rdf:type owl:Restriction ;
                            owl:onProperty :hasQuality ;
                            owl:someValuesFrom :PreservationQuality
                          ] ,
                          [ rdf:type owl:Restriction ;
                            owl:onProperty :isChangedBy ;
                            owl:someValuesFrom :Event
                          ] ,
                          [ rdf:type owl:Restriction ;
                            owl:onProperty :relatedTo ;
                            owl:someValuesFrom :Artefact
                          ] ,
                          [ rdf:type owl:Restriction ;
                            owl:onProperty :storedIn ;
                            owl:someValuesFrom :ControlledVocabulary
                          ] ,
                          [ rdf:type owl:Restriction ;
                            owl:onProperty :hasLocation ;
                            owl:allValuesFrom :SpatialLocation
                          ] ;
          rdfs:comment "An Artefact is an object that is made by a Person and that is to be preserved."@en ;
          rdfs:label "Artefact"@en .


###  http://reference.data.gov.au/def/ont/agrif#Association
:Association rdf:type owl:Class ;
             rdfs:subClassOf [ rdf:type owl:Restriction ;
                               owl:onProperty :associatedRole ;
                               owl:allValuesFrom :Role
                             ] ,
                             [ rdf:type owl:Restriction ;
                               owl:onProperty :hasAgent ;
                               owl:allValuesFrom :Agent
                             ] ;
             dc:source "https://www.w3.org/TR/prov-o/#Association" ;
             rdfs:comment "An Association is a qualified assignment of responsibility to an Agent in an Activity or Event, indicating that the Agent had a Role in the Activity."@en ;
             rdfs:label "Association"@en .


###  http://reference.data.gov.au/def/ont/agrif#AuditEvent
:AuditEvent rdf:type owl:Class ;
            rdfs:subClassOf :ControlEvent ;
            rdfs:comment "An Audit Event is the systematic examination of a Record to ascertain how and where the Record is stored, who created it, or manages it, who uses it and how much longer the Record is required to be maintained."@en ;
            rdfs:label "Audit Event"@en .


###  http://reference.data.gov.au/def/ont/agrif#BusinessOwner
:BusinessOwner rdf:type owl:Class ;
               rdfs:subClassOf :Role ;
               rdfs:comment "A Business Owner is the Role that has the managerial control of a Function."@en ;
               rdfs:label "Business Owner"@en .


###  http://reference.data.gov.au/def/ont/agrif#Classifier
:Classifier rdf:type owl:Class ;
            rdfs:subClassOf [ rdf:type owl:Restriction ;
                              owl:onProperty :associatedFunction ;
                              owl:allValuesFrom :Function
                            ] ;
            rdfs:comment "A Classifier is a machine-generated and applied category that a set of Records belong to."@en ;
            rdfs:label "Classifier"@en .


###  http://reference.data.gov.au/def/ont/agrif#Control
:Control rdf:type owl:Class ;
         rdfs:comment "A Control is a security or access measure that safeguards or restricts access to an asset."@en ;
         rdfs:label "Control"@en .


###  http://reference.data.gov.au/def/ont/agrif#ControlEvent
:ControlEvent rdf:type owl:Class ;
              rdfs:subClassOf :Event ,
                              [ rdf:type owl:Restriction ;
                                owl:onProperty :hasControl ;
                                owl:someValuesFrom :Control
                              ] ;
              rdfs:comment "A Control Event is an Event that requires a particular level of access to the Record."@en ;
              rdfs:label "Control Event"@en .


###  http://reference.data.gov.au/def/ont/agrif#ControlledVocabulary
:ControlledVocabulary rdf:type owl:Class ;
                      rdfs:subClassOf :IntellectualControlSystem ,
                                      [ rdf:type owl:Restriction ;
                                        owl:onProperty :associatedFunction ;
                                        owl:minQualifiedCardinality "1"^^xsd:nonNegativeInteger ;
                                        owl:onClass :Function
                                      ] ;
                      rdfs:comment "A Controlled Vocabulary is an Intellectual Control System that provides a way to organize Records that facilitates a later discovery of a Record."@en ;
                      rdfs:label "Controlled Vocabulary"@en ;
                      rdfs:seeAlso "http://www.w3.org/2004/02/skos/core#ConceptScheme" .


###  http://reference.data.gov.au/def/ont/agrif#Coverage
:Coverage rdf:type owl:Class ;
          rdfs:comment "A Coverage denotes the jurisdictional applicability, or the temporal and/or spatial extent to which a Record is observed."@en ;
          rdfs:label "Coverage"@en .


###  http://reference.data.gov.au/def/ont/agrif#CreationEvent
:CreationEvent rdf:type owl:Class ;
               rdfs:subClassOf :Event ;
               rdfs:comment "A Creation Event is a Change Event that results in the creation of a Record."@en ;
               rdfs:label "Creation Event"@en .


###  http://reference.data.gov.au/def/ont/agrif#Creator
:Creator rdf:type owl:Class ;
         rdfs:subClassOf :Role ;
         rdfs:comment "A Creator is the Agent that has created a Record or Artefact."@en ;
         rdfs:label "Creator"@en .


###  http://reference.data.gov.au/def/ont/agrif#DecisionEvent
:DecisionEvent rdf:type owl:Class ;
               rdfs:subClassOf :ControlEvent ,
                               [ rdf:type owl:Restriction ;
                                 owl:onProperty :hasDecisionStatus ;
                                 owl:someValuesFrom :DecisionStatus
                               ] ,
                               [ rdf:type owl:Restriction ;
                                 owl:onProperty :hasPrerequisiteDecisionEvent ;
                                 owl:someValuesFrom :DecisionEvent
                               ] ;
               rdfs:comment "A Decision Event changes the Decision Status on the Control of a Record."@en ;
               rdfs:label "Decision Event"@en .


###  http://reference.data.gov.au/def/ont/agrif#DecisionStatus
:DecisionStatus rdf:type owl:Class ;
                rdfs:subClassOf :Status ;
                rdfs:comment "A Decision Status is a Status that indicates the approval or disapproval of a Decision Event."@en ;
                rdfs:label "Decision Status"@en .


###  http://reference.data.gov.au/def/ont/agrif#DestroyEvent
:DestroyEvent rdf:type owl:Class ;
              rdfs:subClassOf :DisposalEvent ;
              rdfs:comment "A Destroy Event is a Disposal Event that results in the regular authorised permanent desctruction of a Record that is no longer required for business purposes."@en ;
              rdfs:label "Destroy Event"@en .


###  http://reference.data.gov.au/def/ont/agrif#DigitalArtefact
:DigitalArtefact rdf:type owl:Class ;
                 rdfs:subClassOf :Artefact ,
                                 [ rdf:type owl:Restriction ;
                                   owl:onProperty :storedIn ;
                                   owl:someValuesFrom :InformationSystem
                                 ] ,
                                 [ rdf:type owl:Restriction ;
                                   owl:onProperty :filename ;
                                   owl:someValuesFrom rdfs:Literal
                                 ] ,
                                 [ rdf:type owl:Restriction ;
                                   owl:onProperty :filesize ;
                                   owl:someValuesFrom xsd:long
                                 ] ,
                                 [ rdf:type owl:Restriction ;
                                   owl:onProperty :format ;
                                   owl:someValuesFrom rdfs:Literal
                                 ] ;
                 rdfs:comment "A Digital Artefact is an Artefact that is of a digital nature and stored in an Information System."@en ;
                 rdfs:label "Digital Artefact"@en .


###  http://reference.data.gov.au/def/ont/agrif#DigitalHoldingSpace
:DigitalHoldingSpace rdf:type owl:Class ;
                     rdfs:subClassOf :HoldingSpace ;
                     rdfs:comment "A Digital Holding Space is a space that is used or reserved for the storage of a Digital Artefact on a storage medium or virtual storage space."@en ;
                     rdfs:label "Digital Holding Space"@en .


###  http://reference.data.gov.au/def/ont/agrif#DigitalPreservationPolicy
:DigitalPreservationPolicy rdf:type owl:Class ;
                           rdfs:subClassOf :Policy ;
                           rdfs:comment "The Digital Preservation Policy defines the process of active management by which the National Archives ensures that a digital object will be accessible in the future."@en ;
                           rdfs:label "Digital Preservation Policy"@en .


###  http://reference.data.gov.au/def/ont/agrif#DisposalClass
:DisposalClass rdf:type owl:Class ;
               rdfs:subClassOf :RecordsAuthorityPolicy ,
                               [ rdf:type owl:Restriction ;
                                 owl:onProperty :disposalClassNumber ;
                                 owl:qualifiedCardinality "1"^^xsd:nonNegativeInteger ;
                                 owl:onDataRange xsd:integer
                               ] ;
               rdfs:comment "A Disposal Class is a Policy that defines the sentencing requirements of an item."@en ;
               rdfs:label "Disposal Class"@en .


###  http://reference.data.gov.au/def/ont/agrif#DisposalEvent
:DisposalEvent rdf:type owl:Class ;
               rdfs:subClassOf :ControlEvent ;
               rdfs:comment "A Disposal Event is an Event that results in the regular authorised destruction or change of custody of a Record that is no longer required for business purposes."@en ;
               rdfs:label "Disposal Event"@en .


###  http://reference.data.gov.au/def/ont/agrif#Event
:Event rdf:type owl:Class ;
       rdfs:subClassOf [ rdf:type owl:Restriction ;
                         owl:onProperty :qualifiedAssociation ;
                         owl:someValuesFrom :Association
                       ] ,
                       [ rdf:type owl:Restriction ;
                         owl:onProperty :wasAssociatedWith ;
                         owl:someValuesFrom :Agent
                       ] ,
                       [ rdf:type owl:Restriction ;
                         owl:onProperty :associatedFunction ;
                         owl:allValuesFrom :Function
                       ] ,
                       [ rdf:type owl:Restriction ;
                         owl:onProperty :guidingPolicy ;
                         owl:allValuesFrom :Policy
                       ] ,
                       [ rdf:type owl:Restriction ;
                         owl:onProperty :hasStatus ;
                         owl:allValuesFrom :Status
                       ] ,
                       [ rdf:type owl:Restriction ;
                         owl:onProperty :triggeredBy ;
                         owl:allValuesFrom :Trigger
                       ] ,
                       [ rdf:type owl:Restriction ;
                         owl:onProperty :atTime ;
                         owl:qualifiedCardinality "1"^^xsd:nonNegativeInteger ;
                         owl:onDataRange xsd:dateTime
                       ] ;
       dc:source "https://www.w3.org/TR/prov-o/#InstantaneousEvent" ;
       rdfs:comment "An Event denotes an instantaneous transition in the world."@en ;
       rdfs:label "Event"@en .


###  http://reference.data.gov.au/def/ont/agrif#FormFactor
:FormFactor rdf:type owl:Class ;
            rdfs:comment "A Form Factor defines and prescribes the size, shape, and other physical specifications of a Physical Artefact that is stored."@en ;
            rdfs:label "Form Factor"@en .


###  http://reference.data.gov.au/def/ont/agrif#FreezeEvent
:FreezeEvent rdf:type owl:Class ;
             rdfs:subClassOf :DisposalEvent ;
             rdfs:comment "A Freeze Event is a Disposal Event that leads to a records disposal freeze or retention notice in support of compliance requirements or an identified need to suspend the Archives' records destruction permissions."@en ;
             rdfs:label "Freeze Event"@en .


###  http://reference.data.gov.au/def/ont/agrif#Function
:Function rdf:type owl:Class ;
          rdfs:subClassOf [ rdf:type owl:Restriction ;
                            owl:onProperty :guidingPolicy ;
                            owl:allValuesFrom :Policy
                          ] ;
          rdfs:comment "A Function is a process that is performed routinely to carry out a part of the mandate of an Australian Government Agency."@en ,
                       "A Function reflects the responsibilities of an Organisation that can be delegated through official channels. [Commonwealth Records Series Manual]"@en ;
          rdfs:label "Function"@en .


###  http://reference.data.gov.au/def/ont/agrif#HoldingSpace
:HoldingSpace rdf:type owl:Class ;
              rdfs:subClassOf :SpatialLocation ;
              rdfs:comment "A Holding Space is a space that is used or reserved for the storage of an Artefact."@en ;
              rdfs:label "Holding Space"@en .


###  http://reference.data.gov.au/def/ont/agrif#InformationManagementPolicy
:InformationManagementPolicy rdf:type owl:Class ;
                             rdfs:subClassOf :Policy ,
                                             [ rdf:type owl:Restriction ;
                                               owl:onProperty :hasDisposalClass ;
                                               owl:allValuesFrom :DisposalClass
                                             ] ;
                             rdfs:comment "An Information Management Policy is a Policy that helps to align information management practices to fulfill the requirements of an information governance framework. An Information Management Policy provides direction and guidance to staff for creating, capturing and managing information to satisfy business, legal and stakeholder requirements, and assigns responsibilities across the agency."@en ;
                             rdfs:label "Information Management Policy"@en .


###  http://reference.data.gov.au/def/ont/agrif#InformationSystem
:InformationSystem rdf:type owl:Class ;
                   rdfs:comment "An Information System is an organized system for the collection, organization, storage and communication of information, typically Digital Artefacts or Records."@en ;
                   rdfs:label "Information System"@en .


###  http://reference.data.gov.au/def/ont/agrif#IntellectualControlSystem
:IntellectualControlSystem rdf:type owl:Class ;
                           rdfs:subClassOf :InformationSystem ,
                                           [ rdf:type owl:Restriction ;
                                             owl:onProperty :guidingPolicy ;
                                             owl:allValuesFrom :Policy
                                           ] ;
                           rdfs:comment "An Intellectual Control System is a System that enables Agents to locate and manage information."@en ;
                           rdfs:label "Intellectual Control System"@en .


###  http://reference.data.gov.au/def/ont/agrif#JurisdictionalCoverage
:JurisdictionalCoverage rdf:type owl:Class ;
                        rdfs:subClassOf :Coverage ;
                        rdfs:comment "A Jurisdictional Coverage denotes the jurisdictional applicability of the Record."@en ;
                        rdfs:label "Jurisdictional Coverage"@en ;
                        rdfs:seeAlso "http://purl.org/dc/terms/Jurisdiction" .


###  http://reference.data.gov.au/def/ont/agrif#MaintainActivity
:MaintainActivity rdf:type owl:Class ;
                  rdfs:subClassOf :Activity ,
                                  [ rdf:type owl:Restriction ;
                                    owl:onProperty :hasQuality ;
                                    owl:someValuesFrom :PreservationQuality
                                  ] ;
                  rdfs:comment "A Maintain Activity is an Activity to maintain a Record over a period of time due to a BusinessFunction or Policy."@en ;
                  rdfs:label "Maintain Activity"@en .


###  http://reference.data.gov.au/def/ont/agrif#Manifest
:Manifest rdf:type owl:Class ;
          rdfs:subClassOf [ rdf:type owl:Restriction ;
                            owl:onProperty :checksum ;
                            owl:qualifiedCardinality "1"^^xsd:nonNegativeInteger ;
                            owl:onDataRange xsd:float
                          ] ;
          rdfs:comment "A Manifest describes the files involved in the transfer of a Record from an Agency to the National Archives, including details such as the filesize, the destination hierarchy and the file's metadata."@en ;
          rdfs:label "Manifest"@en .


###  http://reference.data.gov.au/def/ont/agrif#MinimumMetadataSetPolicy
:MinimumMetadataSetPolicy rdf:type owl:Class ;
                          rdfs:subClassOf :Policy ;
                          rdfs:comment "The Minimum Metadata Set Policy is a Policy that has been developed by the National Archives of Australia to identify metadata properties essential for agency management of information as well as those needed for records which will be transferred to the Archives. It supports the Digital Continuity 2020 principles of interoperable systems and processes and is a practical application of the Australian Government Recordkeeping Metadata Standard 2.2 (AGRkMS) to support metadata implementation and information use in agencies."@en ;
                          rdfs:label "Minimum Metadata Set Policy"@en .


###  http://reference.data.gov.au/def/ont/agrif#Organisation
:Organisation rdf:type owl:Class ;
              rdfs:subClassOf :Agent ,
                              [ rdf:type owl:Restriction ;
                                owl:onProperty :associatedFunction ;
                                owl:someValuesFrom :Function
                              ] ;
              dc:source "https://www.w3.org/TR/prov-o/#Organization" ;
              rdfs:comment "An Organisation is a type of Agent that denotes a social or legal institution such as a government agency, a corporation, society, etc."@en ;
              rdfs:label "Organisation"@en .


###  http://reference.data.gov.au/def/ont/agrif#OrganisationalUnit
:OrganisationalUnit rdf:type owl:Class ;
                    rdfs:subClassOf :Organisation ,
                                    [ rdf:type owl:Restriction ;
                                      owl:onProperty :partOf ;
                                      owl:someValuesFrom :Organisation
                                    ] ;
                    rdfs:comment "An Organisational Unit is a division of labour typically organised around a business function that form part of the Organisation."@en ;
                    rdfs:label "Organisational Unit"@en .


###  http://reference.data.gov.au/def/ont/agrif#Permission
:Permission rdf:type owl:Class ;
            dc:source "Australian Government Recordkeeping Metadata Standard"@en ;
            rdfs:comment "A Permission denotes the Security Clearance of an Agent that determines its access and use rights to Records."@en ;
            rdfs:label "Permission"@en .


###  http://reference.data.gov.au/def/ont/agrif#Person
:Person rdf:type owl:Class ;
        rdfs:subClassOf :Agent ;
        dc:source "https://www.w3.org/TR/prov-o/#Person" ;
        rdfs:comment "A Person is an Agent that denotes a human."@en ;
        rdfs:label "Person"@en .


###  http://reference.data.gov.au/def/ont/agrif#PhysicalArtefact
:PhysicalArtefact rdf:type owl:Class ;
                  rdfs:subClassOf :Artefact ,
                                  [ rdf:type owl:Restriction ;
                                    owl:onProperty :hasFormFactor ;
                                    owl:someValuesFrom :FormFactor
                                  ] ;
                  rdfs:comment "A Physical Artefact is an Artefact that is of physical nature."@en ;
                  rdfs:label "Physical Artefact"@en ;
                  skos:example "An example of a Phyiscal Artefact in the context of record keeping is information printed or written on paper."@en .


###  http://reference.data.gov.au/def/ont/agrif#PhysicalHoldingSpace
:PhysicalHoldingSpace rdf:type owl:Class ;
                      rdfs:subClassOf :HoldingSpace ;
                      rdfs:comment "A Physical Holding Space is a Spatial Location that is used or reserved for the storage of a Physical Artefact."@en ;
                      rdfs:label "Physical Holding Space"@en .


###  http://reference.data.gov.au/def/ont/agrif#Policy
:Policy rdf:type owl:Class ;
        dc:source "http://purl.org/dc/terms/Policy" ;
        rdfs:comment "A Policy is a deliberate system of principles to guide decisions and achieve rational outcomes."@en ;
        rdfs:label "Policy"@en .


###  http://reference.data.gov.au/def/ont/agrif#PreservationQuality
:PreservationQuality rdf:type owl:Class ;
                     rdfs:subClassOf :Quality ;
                     rdfs:comment "A Preservation Quality describes a Quality of an Artefact that supports or threatens the long term preservation of the information that is to be preserved."@en ;
                     rdfs:label "Preservation Quality"@en .


###  http://reference.data.gov.au/def/ont/agrif#Quality
:Quality rdf:type owl:Class ;
         rdfs:comment "A Quality is an attribute that is intrinsically associated with an entity."@en ;
         rdfs:label "Quality"@en .


###  http://reference.data.gov.au/def/ont/agrif#Record
:Record rdf:type owl:Class ;
        rdfs:subClassOf [ rdf:type owl:Restriction ;
                          owl:onProperty :hasClassifier ;
                          owl:someValuesFrom :Classifier
                        ] ,
                        [ rdf:type owl:Restriction ;
                          owl:onProperty :hasControl ;
                          owl:someValuesFrom :Control
                        ] ,
                        [ rdf:type owl:Restriction ;
                          owl:onProperty :qualifiedAssociation ;
                          owl:someValuesFrom :Association
                        ] ,
                        [ rdf:type owl:Restriction ;
                          owl:onProperty :relatedTo ;
                          owl:someValuesFrom :Record
                        ] ,
                        [ rdf:type owl:Restriction ;
                          owl:onProperty :hasActivity ;
                          owl:allValuesFrom :Activity
                        ] ,
                        [ rdf:type owl:Restriction ;
                          owl:onProperty :hasCoverage ;
                          owl:allValuesFrom :Coverage
                        ] ,
                        [ rdf:type owl:Restriction ;
                          owl:onProperty :hasSeries ;
                          owl:allValuesFrom :Series
                        ] ,
                        [ rdf:type owl:Restriction ;
                          owl:onProperty :hasStatus ;
                          owl:allValuesFrom :Status
                        ] ,
                        [ rdf:type owl:Restriction ;
                          owl:onProperty :isChangedBy ;
                          owl:allValuesFrom :Event
                        ] ,
                        [ rdf:type owl:Restriction ;
                          owl:onProperty :replaces ;
                          owl:allValuesFrom :Record
                        ] ,
                        [ rdf:type owl:Restriction ;
                          owl:onProperty :requiresSecurityClassification ;
                          owl:allValuesFrom :SecurityClassification
                        ] ,
                        [ rdf:type owl:Restriction ;
                          owl:onProperty :associatedFunction ;
                          owl:minQualifiedCardinality "1"^^xsd:nonNegativeInteger ;
                          owl:onClass :Function
                        ] ,
                        [ rdf:type owl:Restriction ;
                          owl:onProperty :recordOf ;
                          owl:minQualifiedCardinality "1"^^xsd:nonNegativeInteger ;
                          owl:onClass :Artefact
                        ] ,
                        [ rdf:type owl:Restriction ;
                          owl:onProperty :hasDisposalClass ;
                          owl:qualifiedCardinality "1"^^xsd:nonNegativeInteger ;
                          owl:onClass :DisposalClass
                        ] ,
                        [ rdf:type owl:Restriction ;
                          owl:onProperty :isChangedBy ;
                          owl:qualifiedCardinality "1"^^xsd:nonNegativeInteger ;
                          owl:onClass :CreationEvent
                        ] ,
                        [ rdf:type owl:Restriction ;
                          owl:onProperty :checksum ;
                          owl:maxQualifiedCardinality "1"^^xsd:nonNegativeInteger ;
                          owl:onDataRange xsd:float
                        ] ;
        rdfs:comment "A Record is information in any format created, received and maintained as evidence by an Organisation or Person, in pursuance of legal obligations or in the transaction of business. A Record may comprise a Digital or Physical Artefact."@en ;
        rdfs:label "Record"@en .


###  http://reference.data.gov.au/def/ont/agrif#RecordStorageStandard
:RecordStorageStandard rdf:type owl:Class ;
                       rdfs:subClassOf :Policy ;
                       rdfs:comment "The Standard for the storage of non-digital archival Records is designed to set out the requirements for the safe storage and preservation of non-digital records in the Archives’ custody; to ensure all non-digital records are protected, secure and accessible for as long as they are required to meet business and accountability needs and community expectations; and to ensure all non-digital records are stored in the most cost-effective manner possible."@en ;
                       rdfs:label "Record Storage Standard"@en .


###  http://reference.data.gov.au/def/ont/agrif#RecordsAuthorityFunction
:RecordsAuthorityFunction rdf:type owl:Class ;
                          rdfs:subClassOf :Function ;
                          rdfs:comment "A Records Authority Function is a Function that is assigned by the National Archives to classify Agency business."@en ;
                          rdfs:label "Records Authority Function"@en .


###  http://reference.data.gov.au/def/ont/agrif#RecordsAuthorityPolicy
:RecordsAuthorityPolicy rdf:type owl:Class ;
                        rdfs:subClassOf :Policy ,
                                        [ rdf:type owl:Restriction ;
                                          owl:onProperty :hasDisposalClass ;
                                          owl:allValuesFrom :DisposalClass
                                        ] ;
                        dc:source "Australian Government Recordkeeping Metadata Standard"@en ;
                        rdfs:comment "A Records Authority Disposal Class Policy is a Policy that identifies the specific disposal class that authorises the retention or destruction of a Record."@en ;
                        rdfs:label "Records Authority Disposal Class Policy"@en .


###  http://reference.data.gov.au/def/ont/agrif#ReplaceEvent
:ReplaceEvent rdf:type owl:Class ;
              rdfs:subClassOf :ControlEvent ,
                              [ rdf:type owl:Restriction ;
                                owl:onProperty :hasVersionHistory ;
                                owl:someValuesFrom :VersionHistory
                              ] ,
                              [ rdf:type owl:Restriction ;
                                owl:onProperty :replacedBy ;
                                owl:qualifiedCardinality "1"^^xsd:nonNegativeInteger ;
                                owl:onClass :Record
                              ] ;
              rdfs:comment "A Replace Event is an Event that results in the replacement of a Record with a new version. Edits to a Record constitute a Replace Event."@en ;
              rdfs:label "Replace Event"@en .


###  http://reference.data.gov.au/def/ont/agrif#Role
:Role rdf:type owl:Class ;
      rdfs:subClassOf [ rdf:type owl:Restriction ;
                        owl:onProperty :hasPermission ;
                        owl:someValuesFrom :Permission
                      ] ;
      dc:source "https://www.w3.org/TR/prov-o/#Role" ;
      rdfs:comment "A Role is the function of an entity or agent with respect to an Activity or Event, in the context of a usage, generation, invalidation, association, start, and end."@en ;
      rdfs:label "Role"@en .


###  http://reference.data.gov.au/def/ont/agrif#SecurityClassification
:SecurityClassification rdf:type owl:Class ;
                        rdfs:subClassOf :AccessControl ;
                        dc:source "Australian Government Recordkeeping Metadata Standard"@en ;
                        rdfs:comment "A Security Classification denotes the security status of a Record that an Agent needs to possess to access the Record."@en ;
                        rdfs:label "Security Classification"@en .


###  http://reference.data.gov.au/def/ont/agrif#SecurityControl
:SecurityControl rdf:type owl:Class ;
                 rdfs:subClassOf :Control ;
                 rdfs:comment "A Security Control is a safeguard or countermeasures to avoid, detect, counteract, or minimize security risks to a Record or Artefact."@en ;
                 rdfs:label "Security Control"@en .


###  http://reference.data.gov.au/def/ont/agrif#SentencingEvent
:SentencingEvent rdf:type owl:Class ;
                 rdfs:subClassOf :ControlEvent ;
                 rdfs:comment "A Sentencing Event is an Event that classifies an Agencies Record to a specific class of a Records Authority Policy. This helps determine the Records value and how it should be managed throughout its lifecycle."@en ;
                 rdfs:label "Sentencing Event"@en .


###  http://reference.data.gov.au/def/ont/agrif#Series
:Series rdf:type owl:Class ;
        rdfs:subClassOf :IntellectualControlSystem ,
                        [ rdf:type owl:Restriction ;
                          owl:onProperty :associatedFunction ;
                          owl:allValuesFrom :Function
                        ] ;
        rdfs:comment "A Series is an identifier for an item, and when combined with a control symbol gives an item its intellectual context."@en ;
        rdfs:label "Series"@en .


###  http://reference.data.gov.au/def/ont/agrif#ShareActivity
:ShareActivity rdf:type owl:Class ;
               rdfs:subClassOf :Activity ,
                               [ rdf:type owl:Restriction ;
                                 owl:onProperty :sharedWith ;
                                 owl:someValuesFrom :Agent
                               ] ;
               rdfs:comment "A Share Activity is an Activity where the custodianship of a Record is transferred to or shared with Agents over a period of time."@en ;
               rdfs:label "Share Activity"@en .


###  http://reference.data.gov.au/def/ont/agrif#SpatialCoverage
:SpatialCoverage rdf:type owl:Class ;
                 rdfs:subClassOf :Coverage ;
                 rdfs:comment "A Spatial Coverage denotes the spatial extent to which a Record is observed."@en ;
                 rdfs:label "Spatial Coverage"@en ;
                 rdfs:seeAlso "http://purl.org/dc/terms/spatial" .


###  http://reference.data.gov.au/def/ont/agrif#SpatialLocation
:SpatialLocation rdf:type owl:Class ;
                 rdfs:comment "A Spatial Location describes where a something (e.g. a Record, Collection or Artefact) is physically located, using geospatial coordinates such as latitude and longitude."@en ;
                 rdfs:label "Spatial Location"@en .


###  http://reference.data.gov.au/def/ont/agrif#Status
:Status rdf:type owl:Class ;
        rdfs:comment "A Status indicates an Activities current state."@en ;
        rdfs:label "Status"@en .


###  http://reference.data.gov.au/def/ont/agrif#TemporalCoverage
:TemporalCoverage rdf:type owl:Class ;
                  rdfs:subClassOf :Coverage ;
                  rdfs:comment "A Temporal Coverage denotes the temporal extent to which a Record is observed."@en ;
                  rdfs:label "Temporal Coverage"@en ;
                  rdfs:seeAlso "http://purl.org/dc/terms/temporal" .


###  http://reference.data.gov.au/def/ont/agrif#TransferEvent
:TransferEvent rdf:type owl:Class ;
               rdfs:subClassOf :DisposalEvent ,
                               [ rdf:type owl:Restriction ;
                                 owl:onProperty :hasManifest ;
                                 owl:someValuesFrom :Manifest
                               ] ,
                               [ rdf:type owl:Restriction ;
                                 owl:onProperty :transferredFrom ;
                                 owl:someValuesFrom :BusinessOwner
                               ] ,
                               [ rdf:type owl:Restriction ;
                                 owl:onProperty :transferredFrom ;
                                 owl:someValuesFrom :Role
                               ] ,
                               [ rdf:type owl:Restriction ;
                                 owl:onProperty :transferredTo ;
                                 owl:someValuesFrom :BusinessOwner
                               ] ,
                               [ rdf:type owl:Restriction ;
                                 owl:onProperty :transferredTo ;
                                 owl:someValuesFrom :Role
                               ] ;
               rdfs:comment "A Transfer Event is a Disposal Event that results in a change of custody."@en ;
               rdfs:label "Transfer Event"@en ;
               skos:example "An example of a Transfer Event is the transfer of a Record from an Agency to the National Archives. Section 27 of the Archives Act 1983 requires Australian government agencies to transfer Records to the Archives within 15 years of their creation."@en .


###  http://reference.data.gov.au/def/ont/agrif#Trigger
:Trigger rdf:type owl:Class ;
         rdfs:subClassOf [ rdf:type owl:Restriction ;
                           owl:onProperty :notifies ;
                           owl:someValuesFrom :Agent
                         ] ;
         rdfs:comment "A Trigger is an entity that initiated an Activity or Event."@en ;
         rdfs:label "Trigger"@en .


###  http://reference.data.gov.au/def/ont/agrif#User
:User rdf:type owl:Class ;
      rdfs:subClassOf :Role ;
      rdfs:comment "A User is an Agent that uses a Record."@en ;
      rdfs:label "User"@en .


###  http://reference.data.gov.au/def/ont/agrif#VersionHistory
:VersionHistory rdf:type owl:Class ;
                rdfs:comment "A Version History is the cumulative change to a previous version of a file."@en ;
                rdfs:label "Version History"@en .


###  http://www.w3.org/2000/01/rdf-schema#Class
rdfs:Class rdf:type owl:Class .


#################################################################
#    Individuals
#################################################################

###  http://purl.org/dc/aboutdcmi#DCMI
<http://purl.org/dc/aboutdcmi#DCMI> rdf:type owl:NamedIndividual .


###  http://purl.org/dc/terms/
dcterms: rdf:type owl:NamedIndividual ;
       dcterms:modified "2012-06-14"^^xsd:date ;
       dcterms:publisher <http://purl.org/dc/aboutdcmi#DCMI> ;
       dcterms:title "DCMI Metadata Terms - other"@en .


###  http://purl.org/dc/terms/Agent
dcterms:Agent rdf:type owl:NamedIndividual ,
                     dcterms:AgentClass .


###  http://purl.org/dc/terms/AgentClass
dcterms:AgentClass rdf:type owl:NamedIndividual .


###  http://purl.org/dc/terms/BibliographicResource
dcterms:BibliographicResource rdf:type owl:NamedIndividual .


###  http://purl.org/dc/terms/Box
dcterms:Box rdf:type owl:NamedIndividual .


###  http://purl.org/dc/terms/DCMIType
dcterms:DCMIType rdf:type owl:NamedIndividual ,
                        <http://purl.org/dc/dcam/VocabularyEncodingScheme> ;
               dcterms:hasVersion <http://dublincore.org/usage/terms/history/#DCMIType-005> ;
               dcterms:issued "2000-07-11"^^xsd:date ;
               dcterms:modified "2012-06-14"^^xsd:date ;
               rdfs:comment "The set of classes specified by the DCMI Type Vocabulary, used to categorize the nature or genre of the resource."@en ;
               rdfs:isDefinedBy dcterms: ;
               rdfs:label "DCMI Type Vocabulary"@en ;
               rdfs:seeAlso <http://purl.org/dc/dcmitype/> .


###  http://purl.org/dc/terms/DDC
dcterms:DDC rdf:type owl:NamedIndividual ,
                   <http://purl.org/dc/dcam/VocabularyEncodingScheme> ;
          dcterms:hasVersion <http://dublincore.org/usage/terms/history/#DDC-003> ;
          dcterms:issued "2000-07-11"^^xsd:date ;
          dcterms:modified "2008-01-14"^^xsd:date ;
          rdfs:comment "The set of conceptual resources specified by the Dewey Decimal Classification."@en ;
          rdfs:isDefinedBy dcterms: ;
          rdfs:label "DDC"@en ;
          rdfs:seeAlso <http://www.oclc.org/dewey/> .


###  http://purl.org/dc/terms/FileFormat
dcterms:FileFormat rdf:type owl:NamedIndividual .


###  http://purl.org/dc/terms/Frequency
dcterms:Frequency rdf:type owl:NamedIndividual .


###  http://purl.org/dc/terms/IMT
dcterms:IMT rdf:type owl:NamedIndividual ,
                   <http://purl.org/dc/dcam/VocabularyEncodingScheme> ;
          dcterms:hasVersion <http://dublincore.org/usage/terms/history/#IMT-004> ;
          dcterms:issued "2000-07-11"^^xsd:date ;
          dcterms:modified "2008-01-14"^^xsd:date ;
          rdfs:comment "The set of media types specified by the Internet Assigned Numbers Authority."@en ;
          rdfs:isDefinedBy dcterms: ;
          rdfs:label "IMT"@en ;
          rdfs:seeAlso <http://www.iana.org/assignments/media-types/> .


###  http://purl.org/dc/terms/ISO3166
dcterms:ISO3166 rdf:type owl:NamedIndividual .


###  http://purl.org/dc/terms/ISO639-2
dcterms:ISO639-2 rdf:type owl:NamedIndividual .


###  http://purl.org/dc/terms/ISO639-3
dcterms:ISO639-3 rdf:type owl:NamedIndividual .


###  http://purl.org/dc/terms/Jurisdiction
dcterms:Jurisdiction rdf:type owl:NamedIndividual .


###  http://purl.org/dc/terms/LCC
dcterms:LCC rdf:type owl:NamedIndividual ,
                   <http://purl.org/dc/dcam/VocabularyEncodingScheme> ;
          dcterms:hasVersion <http://dublincore.org/usage/terms/history/#LCC-003> ;
          dcterms:issued "2000-07-11"^^xsd:date ;
          dcterms:modified "2008-01-14"^^xsd:date ;
          rdfs:comment "The set of conceptual resources specified by the Library of Congress Classification."@en ;
          rdfs:isDefinedBy dcterms: ;
          rdfs:label "LCC"@en ;
          rdfs:seeAlso <http://lcweb.loc.gov/catdir/cpso/lcco/lcco.html> .


###  http://purl.org/dc/terms/LCSH
dcterms:LCSH rdf:type owl:NamedIndividual ,
                    <http://purl.org/dc/dcam/VocabularyEncodingScheme> ;
           dcterms:hasVersion <http://dublincore.org/usage/terms/history/#LCSH-003> ;
           dcterms:issued "2000-07-11"^^xsd:date ;
           dcterms:modified "2008-01-14"^^xsd:date ;
           rdfs:comment "The set of labeled concepts specified by the Library of Congress Subject Headings."@en ;
           rdfs:isDefinedBy dcterms: ;
           rdfs:label "LCSH"@en .


###  http://purl.org/dc/terms/LicenseDocument
dcterms:LicenseDocument rdf:type owl:NamedIndividual .


###  http://purl.org/dc/terms/LinguisticSystem
dcterms:LinguisticSystem rdf:type owl:NamedIndividual .


###  http://purl.org/dc/terms/Location
dcterms:Location rdf:type owl:NamedIndividual .


###  http://purl.org/dc/terms/LocationPeriodOrJurisdiction
dcterms:LocationPeriodOrJurisdiction rdf:type owl:NamedIndividual .


###  http://purl.org/dc/terms/MESH
dcterms:MESH rdf:type owl:NamedIndividual ,
                    <http://purl.org/dc/dcam/VocabularyEncodingScheme> ;
           dcterms:hasVersion <http://dublincore.org/usage/terms/history/#MESH-003> ;
           dcterms:issued "2000-07-11"^^xsd:date ;
           dcterms:modified "2008-01-14"^^xsd:date ;
           rdfs:comment "The set of labeled concepts specified by the Medical Subject Headings."@en ;
           rdfs:isDefinedBy dcterms: ;
           rdfs:label "MeSH"@en ;
           rdfs:seeAlso <http://www.nlm.nih.gov/mesh/meshhome.html> .


###  http://purl.org/dc/terms/MediaType
dcterms:MediaType rdf:type owl:NamedIndividual .


###  http://purl.org/dc/terms/MediaTypeOrExtent
dcterms:MediaTypeOrExtent rdf:type owl:NamedIndividual .


###  http://purl.org/dc/terms/MethodOfAccrual
dcterms:MethodOfAccrual rdf:type owl:NamedIndividual .


###  http://purl.org/dc/terms/MethodOfInstruction
dcterms:MethodOfInstruction rdf:type owl:NamedIndividual .


###  http://purl.org/dc/terms/NLM
dcterms:NLM rdf:type owl:NamedIndividual ,
                   <http://purl.org/dc/dcam/VocabularyEncodingScheme> ;
          dcterms:hasVersion <http://dublincore.org/usage/terms/history/#NLM-002> ;
          dcterms:issued "2005-06-13"^^xsd:date ;
          dcterms:modified "2008-01-14"^^xsd:date ;
          rdfs:comment "The set of conceptual resources specified by the National Library of Medicine Classification."@en ;
          rdfs:isDefinedBy dcterms: ;
          rdfs:label "NLM"@en ;
          rdfs:seeAlso <http://wwwcf.nlm.nih.gov/class/> .


###  http://purl.org/dc/terms/Period
dcterms:Period rdf:type owl:NamedIndividual .


###  http://purl.org/dc/terms/PeriodOfTime
dcterms:PeriodOfTime rdf:type owl:NamedIndividual .


###  http://purl.org/dc/terms/PhysicalMedium
dcterms:PhysicalMedium rdf:type owl:NamedIndividual .


###  http://purl.org/dc/terms/PhysicalResource
dcterms:PhysicalResource rdf:type owl:NamedIndividual .


###  http://purl.org/dc/terms/Point
dcterms:Point rdf:type owl:NamedIndividual .


###  http://purl.org/dc/terms/Policy
dcterms:Policy rdf:type owl:NamedIndividual .


###  http://purl.org/dc/terms/ProvenanceStatement
dcterms:ProvenanceStatement rdf:type owl:NamedIndividual .


###  http://purl.org/dc/terms/RFC1766
dcterms:RFC1766 rdf:type owl:NamedIndividual .


###  http://purl.org/dc/terms/RFC3066
dcterms:RFC3066 rdf:type owl:NamedIndividual .


###  http://purl.org/dc/terms/RFC4646
dcterms:RFC4646 rdf:type owl:NamedIndividual .


###  http://purl.org/dc/terms/RFC5646
dcterms:RFC5646 rdf:type owl:NamedIndividual .


###  http://purl.org/dc/terms/RightsStatement
dcterms:RightsStatement rdf:type owl:NamedIndividual .


###  http://purl.org/dc/terms/SizeOrDuration
dcterms:SizeOrDuration rdf:type owl:NamedIndividual .


###  http://purl.org/dc/terms/Standard
dcterms:Standard rdf:type owl:NamedIndividual .


###  http://purl.org/dc/terms/TGN
dcterms:TGN rdf:type owl:NamedIndividual ,
                   <http://purl.org/dc/dcam/VocabularyEncodingScheme> ;
          dcterms:hasVersion <http://dublincore.org/usage/terms/history/#TGN-003> ;
          dcterms:issued "2000-07-11"^^xsd:date ;
          dcterms:modified "2008-01-14"^^xsd:date ;
          rdfs:comment "The set of places specified by the Getty Thesaurus of Geographic Names."@en ;
          rdfs:isDefinedBy dcterms: ;
          rdfs:label "TGN"@en ;
          rdfs:seeAlso <http://www.getty.edu/research/tools/vocabulary/tgn/index.html> .


###  http://purl.org/dc/terms/UDC
dcterms:UDC rdf:type owl:NamedIndividual ,
                   <http://purl.org/dc/dcam/VocabularyEncodingScheme> ;
          dcterms:hasVersion <http://dublincore.org/usage/terms/history/#UDC-003> ;
          dcterms:issued "2000-07-11"^^xsd:date ;
          dcterms:modified "2008-01-14"^^xsd:date ;
          rdfs:comment "The set of conceptual resources specified by the Universal Decimal Classification."@en ;
          rdfs:isDefinedBy dcterms: ;
          rdfs:label "UDC"@en ;
          rdfs:seeAlso <http://www.udcc.org/> .


###  http://purl.org/dc/terms/URI
dcterms:URI rdf:type owl:NamedIndividual .


###  http://purl.org/dc/terms/W3CDTF
dcterms:W3CDTF rdf:type owl:NamedIndividual .


###  http://purl.org/dc/terms/abstract
dcterms:abstract rdf:type owl:NamedIndividual .


###  http://purl.org/dc/terms/accessRights
dcterms:accessRights rdf:type owl:NamedIndividual .


###  http://purl.org/dc/terms/accrualMethod
dcterms:accrualMethod rdf:type owl:NamedIndividual .


###  http://purl.org/dc/terms/accrualPeriodicity
dcterms:accrualPeriodicity rdf:type owl:NamedIndividual .


###  http://purl.org/dc/terms/accrualPolicy
dcterms:accrualPolicy rdf:type owl:NamedIndividual .


###  http://purl.org/dc/terms/alternative
dcterms:alternative rdf:type owl:NamedIndividual .


###  http://purl.org/dc/terms/audience
dcterms:audience rdf:type owl:NamedIndividual .


###  http://purl.org/dc/terms/available
dcterms:available rdf:type owl:NamedIndividual .


###  http://purl.org/dc/terms/bibliographicCitation
dcterms:bibliographicCitation rdf:type owl:NamedIndividual .


###  http://purl.org/dc/terms/conformsTo
dcterms:conformsTo rdf:type owl:NamedIndividual .


###  http://purl.org/dc/terms/contributor
dcterms:contributor rdf:type owl:NamedIndividual .


###  http://purl.org/dc/terms/coverage
dcterms:coverage rdf:type owl:NamedIndividual .


###  http://purl.org/dc/terms/created
dcterms:created rdf:type owl:NamedIndividual .


###  http://purl.org/dc/terms/creator
dcterms:creator rdf:type owl:NamedIndividual .


###  http://purl.org/dc/terms/date
dcterms:date rdf:type owl:NamedIndividual .


###  http://purl.org/dc/terms/dateAccepted
dcterms:dateAccepted rdf:type owl:NamedIndividual .


###  http://purl.org/dc/terms/dateCopyrighted
dcterms:dateCopyrighted rdf:type owl:NamedIndividual .


###  http://purl.org/dc/terms/dateSubmitted
dcterms:dateSubmitted rdf:type owl:NamedIndividual .


###  http://purl.org/dc/terms/description
dcterms:description rdf:type owl:NamedIndividual .


###  http://purl.org/dc/terms/educationLevel
dcterms:educationLevel rdf:type owl:NamedIndividual .


###  http://purl.org/dc/terms/extent
dcterms:extent rdf:type owl:NamedIndividual .


###  http://purl.org/dc/terms/format
dcterms:format rdf:type owl:NamedIndividual .


###  http://purl.org/dc/terms/hasFormat
dcterms:hasFormat rdf:type owl:NamedIndividual .


###  http://purl.org/dc/terms/hasPart
dcterms:hasPart rdf:type owl:NamedIndividual .


###  http://purl.org/dc/terms/hasVersion
dcterms:hasVersion rdf:type owl:NamedIndividual .


###  http://purl.org/dc/terms/identifier
dcterms:identifier rdf:type owl:NamedIndividual .


###  http://purl.org/dc/terms/instructionalMethod
dcterms:instructionalMethod rdf:type owl:NamedIndividual .


###  http://purl.org/dc/terms/isFormatOf
dcterms:isFormatOf rdf:type owl:NamedIndividual .


###  http://purl.org/dc/terms/isPartOf
dcterms:isPartOf rdf:type owl:NamedIndividual .


###  http://purl.org/dc/terms/isReferencedBy
dcterms:isReferencedBy rdf:type owl:NamedIndividual .


###  http://purl.org/dc/terms/isReplacedBy
dcterms:isReplacedBy rdf:type owl:NamedIndividual .


###  http://purl.org/dc/terms/isRequiredBy
dcterms:isRequiredBy rdf:type owl:NamedIndividual .


###  http://purl.org/dc/terms/isVersionOf
dcterms:isVersionOf rdf:type owl:NamedIndividual .


###  http://purl.org/dc/terms/issued
dcterms:issued rdf:type owl:NamedIndividual .


###  http://purl.org/dc/terms/language
dcterms:language rdf:type owl:NamedIndividual .


###  http://purl.org/dc/terms/license
dcterms:license rdf:type owl:NamedIndividual .


###  http://purl.org/dc/terms/mediator
dcterms:mediator rdf:type owl:NamedIndividual .


###  http://purl.org/dc/terms/medium
dcterms:medium rdf:type owl:NamedIndividual .


###  http://purl.org/dc/terms/modified
dcterms:modified rdf:type owl:NamedIndividual .


###  http://purl.org/dc/terms/provenance
dcterms:provenance rdf:type owl:NamedIndividual .


###  http://purl.org/dc/terms/publisher
dcterms:publisher rdf:type owl:NamedIndividual .


###  http://purl.org/dc/terms/references
dcterms:references rdf:type owl:NamedIndividual .


###  http://purl.org/dc/terms/relation
dcterms:relation rdf:type owl:NamedIndividual .


###  http://purl.org/dc/terms/replaces
dcterms:replaces rdf:type owl:NamedIndividual .


###  http://purl.org/dc/terms/requires
dcterms:requires rdf:type owl:NamedIndividual .


###  http://purl.org/dc/terms/rights
dcterms:rights rdf:type owl:NamedIndividual .


###  http://purl.org/dc/terms/rightsHolder
dcterms:rightsHolder rdf:type owl:NamedIndividual .


###  http://purl.org/dc/terms/source
dcterms:source rdf:type owl:NamedIndividual .


###  http://purl.org/dc/terms/spatial
dcterms:spatial rdf:type owl:NamedIndividual .


###  http://purl.org/dc/terms/subject
dcterms:subject rdf:type owl:NamedIndividual .


###  http://purl.org/dc/terms/tableOfContents
dcterms:tableOfContents rdf:type owl:NamedIndividual .


###  http://purl.org/dc/terms/temporal
dcterms:temporal rdf:type owl:NamedIndividual .


###  http://purl.org/dc/terms/title
dcterms:title rdf:type owl:NamedIndividual .


###  http://purl.org/dc/terms/type
dcterms:type rdf:type owl:NamedIndividual .


###  http://purl.org/dc/terms/valid
dcterms:valid rdf:type owl:NamedIndividual .


###  http://reference.data.gov.au/def/ont/agrif#Active
:Active rdf:type owl:NamedIndividual ,
                 :Status .


###  http://reference.data.gov.au/def/ont/agrif#Approved
:Approved rdf:type owl:NamedIndividual ,
                   :DecisionStatus .


###  http://reference.data.gov.au/def/ont/agrif#AwaitingDisposal
:AwaitingDisposal rdf:type owl:NamedIndividual ,
                           :Status .


###  http://reference.data.gov.au/def/ont/agrif#Completed
:Completed rdf:type owl:NamedIndividual ,
                    :Status .


###  http://reference.data.gov.au/def/ont/agrif#Confidential
:Confidential rdf:type owl:NamedIndividual ,
                       :SecurityClassification ;
              rdfs:label "Confidential"@en .


###  http://reference.data.gov.au/def/ont/agrif#Disapproved
:Disapproved rdf:type owl:NamedIndividual ,
                      :DecisionStatus .


###  http://reference.data.gov.au/def/ont/agrif#Disposed
:Disposed rdf:type owl:NamedIndividual ,
                   :Status .


###  http://reference.data.gov.au/def/ont/agrif#HighlyProtected
:HighlyProtected rdf:type owl:NamedIndividual ,
                          :SecurityClassification ;
                 rdfs:label "Highly Protected"@en .


###  http://reference.data.gov.au/def/ont/agrif#Protected
:Protected rdf:type owl:NamedIndividual ,
                    :SecurityClassification ;
           rdfs:label "Protected"@en .


###  http://reference.data.gov.au/def/ont/agrif#Redundant
:Redundant rdf:type owl:NamedIndividual ,
                    :Status .


###  http://reference.data.gov.au/def/ont/agrif#RetainAsNationalArchives
:RetainAsNationalArchives rdf:type owl:NamedIndividual ,
                                   :DisposalClass .


###  http://reference.data.gov.au/def/ont/agrif#Secret
:Secret rdf:type owl:NamedIndividual ,
                 :SecurityClassification ;
        rdfs:label "Secret"@en .


###  http://reference.data.gov.au/def/ont/agrif#TopSecretNV
:TopSecretNV rdf:type owl:NamedIndividual ,
                      :SecurityClassification ;
             rdfs:label "Top Secret (NV)"@en .


###  http://reference.data.gov.au/def/ont/agrif#TopSecretPV
:TopSecretPV rdf:type owl:NamedIndividual ,
                      :SecurityClassification ;
             rdfs:label "Top Secret (PV)"@en .


###  http://reference.data.gov.au/def/ont/agrif#Unclassified
:Unclassified rdf:type owl:NamedIndividual ,
                       :SecurityClassification ;
              rdfs:label "Unclassified"@en .


#################################################################
#    Annotations
#################################################################

dcterms:Agent rdfs:label "Agent"@en ;
            rdfs:isDefinedBy dcterms: ;
            rdfs:comment "A resource that acts or has the power to act."@en ;
            dcterms:issued "2008-01-14"^^xsd:date ;
            dcterms:description "Examples of Agent include person, organization, and software agent."@en ;
            dcterms:hasVersion <http://dublincore.org/usage/terms/history/#Agent-001> .


dcterms:AgentClass dcterms:issued "2008-01-14"^^xsd:date ;
                 rdfs:isDefinedBy dcterms: ;
                 rdfs:label "Agent Class"@en ;
                 rdfs:comment "A group of agents."@en ;
                 dcterms:modified "2012-06-14"^^xsd:date ;
                 dcterms:description "Examples of Agent Class include groups seen as classes, such as students, women, charities, lecturers."@en ;
                 dcterms:hasVersion <http://dublincore.org/usage/terms/history/#AgentClass-003> .


dcterms:BibliographicResource rdfs:isDefinedBy dcterms: ;
                            dcterms:hasVersion <http://dublincore.org/usage/terms/history/#BibliographicResource-001> ;
                            rdfs:comment "A book, article, or other documentary resource."@en ;
                            rdfs:label "Bibliographic Resource"@en ;
                            dcterms:issued "2008-01-14"^^xsd:date .


dcterms:Box dcterms:issued "2000-07-11"^^xsd:date ;
          rdfs:comment "The set of regions in space defined by their geographic coordinates according to the DCMI Box Encoding Scheme."@en ;
          rdfs:isDefinedBy dcterms: ;
          rdfs:seeAlso <http://dublincore.org/documents/dcmi-box/> ;
          rdfs:label "DCMI Box"@en ;
          dcterms:modified "2008-01-14"^^xsd:date ;
          dcterms:hasVersion <http://dublincore.org/usage/terms/history/#Box-003> .


dcterms:FileFormat dcterms:description "Examples include the formats defined by the list of Internet Media Types."@en ;
                 dcterms:hasVersion <http://dublincore.org/usage/terms/history/#FileFormat-001> ;
                 rdfs:comment "A digital resource format."@en ;
                 rdfs:label "File Format"@en ;
                 dcterms:issued "2008-01-14"^^xsd:date ;
                 rdfs:isDefinedBy dcterms: .


dcterms:Frequency rdfs:label "Frequency"@en ;
                dcterms:hasVersion <http://dublincore.org/usage/terms/history/#Frequency-001> ;
                rdfs:isDefinedBy dcterms: ;
                rdfs:comment "A rate at which something recurs."@en ;
                dcterms:issued "2008-01-14"^^xsd:date .


dcterms:ISO3166 dcterms:issued "2000-07-11"^^xsd:date ;
              rdfs:comment "The set of codes listed in ISO 3166-1 for the representation of names of countries."@en ;
              rdfs:isDefinedBy dcterms: ;
              dcterms:hasVersion <http://dublincore.org/usage/terms/history/#ISO3166-004> ;
              dcterms:modified "2008-01-14"^^xsd:date ;
              rdfs:label "ISO 3166"@en ;
              rdfs:seeAlso <http://www.iso.org/iso/en/prods-services/iso3166ma/02iso-3166-code-lists/list-en1.html> .


dcterms:ISO639-2 rdfs:seeAlso <http://lcweb.loc.gov/standards/iso639-2/langhome.html> ;
               dcterms:modified "2008-01-14"^^xsd:date ;
               dcterms:issued "2000-07-11"^^xsd:date ;
               rdfs:comment "The three-letter alphabetic codes listed in ISO639-2 for the representation of names of languages."@en ;
               rdfs:isDefinedBy dcterms: ;
               rdfs:label "ISO 639-2"@en ;
               dcterms:hasVersion <http://dublincore.org/usage/terms/history/#ISO639-2-003> .


dcterms:ISO639-3 rdfs:label "ISO 639-3"@en ;
               rdfs:comment "The set of three-letter codes listed in ISO 639-3 for the representation of names of languages."@en ;
               dcterms:hasVersion <http://dublincore.org/usage/terms/history/#ISO639-3-001> ;
               dcterms:issued "2008-01-14"^^xsd:date ;
               rdfs:isDefinedBy dcterms: ;
               rdfs:seeAlso <http://www.sil.org/iso639-3/> .


dcterms:Jurisdiction dcterms:hasVersion <http://dublincore.org/usage/terms/history/#Jurisdiction-001> ;
                   rdfs:label "Jurisdiction"@en ;
                   dcterms:issued "2008-01-14"^^xsd:date ;
                   rdfs:isDefinedBy dcterms: ;
                   rdfs:comment "The extent or range of judicial, law enforcement, or other authority."@en .


dcterms:LicenseDocument rdfs:isDefinedBy dcterms: ;
                      rdfs:label "License Document"@en ;
                      dcterms:issued "2008-01-14"^^xsd:date ;
                      rdfs:comment "A legal document giving official permission to do something with a Resource."@en ;
                      dcterms:hasVersion <http://dublincore.org/usage/terms/history/#LicenseDocument-001> .


dcterms:LinguisticSystem dcterms:issued "2008-01-14"^^xsd:date ;
                       dcterms:hasVersion <http://dublincore.org/usage/terms/history/#LinguisticSystem-001> ;
                       dcterms:description "Examples include written, spoken, sign, and computer languages."@en ;
                       rdfs:isDefinedBy dcterms: ;
                       rdfs:comment "A system of signs, symbols, sounds, gestures, or rules used in communication."@en ;
                       rdfs:label "Linguistic System"@en .


dcterms:Location dcterms:hasVersion <http://dublincore.org/usage/terms/history/#Location-001> ;
               dcterms:issued "2008-01-14"^^xsd:date ;
               rdfs:label "Location"@en ;
               rdfs:isDefinedBy dcterms: ;
               rdfs:comment "A spatial region or named place."@en .


dcterms:LocationPeriodOrJurisdiction rdfs:label "Location, Period, or Jurisdiction"@en ;
                                   dcterms:issued "2008-01-14"^^xsd:date ;
                                   rdfs:comment "A location, period of time, or jurisdiction."@en ;
                                   rdfs:isDefinedBy dcterms: ;
                                   dcterms:hasVersion <http://dublincore.org/usage/terms/history/#LocationPeriodOrJurisdiction-001> .


dcterms:MediaType rdfs:comment "A file format or physical medium."@en ;
                rdfs:label "Media Type"@en ;
                rdfs:isDefinedBy dcterms: ;
                dcterms:hasVersion <http://dublincore.org/usage/terms/history/#MediaType-001> ;
                dcterms:issued "2008-01-14"^^xsd:date .


dcterms:MediaTypeOrExtent rdfs:isDefinedBy dcterms: ;
                        rdfs:comment "A media type or extent."@en ;
                        rdfs:label "Media Type or Extent"@en ;
                        dcterms:issued "2008-01-14"^^xsd:date ;
                        dcterms:hasVersion <http://dublincore.org/usage/terms/history/#MediaTypeOrExtent-001> .


dcterms:MethodOfAccrual rdfs:isDefinedBy dcterms: ;
                      rdfs:comment "A method by which resources are added to a collection."@en ;
                      dcterms:hasVersion <http://dublincore.org/usage/terms/history/#MethodOfAccrual-001> ;
                      rdfs:label "Method of Accrual"@en ;
                      dcterms:issued "2008-01-14"^^xsd:date .


dcterms:MethodOfInstruction rdfs:label "Method of Instruction"@en ;
                          rdfs:comment "A process that is used to engender knowledge, attitudes, and skills."@en ;
                          rdfs:isDefinedBy dcterms: ;
                          dcterms:hasVersion <http://dublincore.org/usage/terms/history/#MethodOfInstruction-001> ;
                          dcterms:issued "2008-01-14"^^xsd:date .


dcterms:Period rdfs:seeAlso <http://dublincore.org/documents/dcmi-period/> ;
             rdfs:comment "The set of time intervals defined by their limits according to the DCMI Period Encoding Scheme."@en ;
             dcterms:modified "2008-01-14"^^xsd:date ;
             dcterms:issued "2000-07-11"^^xsd:date ;
             rdfs:label "DCMI Period"@en ;
             rdfs:isDefinedBy dcterms: ;
             dcterms:hasVersion <http://dublincore.org/usage/terms/history/#Period-003> .


dcterms:PeriodOfTime rdfs:comment "An interval of time that is named or defined by its start and end dates."@en ;
                   dcterms:hasVersion <http://dublincore.org/usage/terms/history/#PeriodOfTime-001> ;
                   rdfs:isDefinedBy dcterms: ;
                   rdfs:label "Period of Time"@en ;
                   dcterms:issued "2008-01-14"^^xsd:date .


dcterms:PhysicalMedium dcterms:hasVersion <http://dublincore.org/usage/terms/history/#PhysicalMedium-001> ;
                     dcterms:issued "2008-01-14"^^xsd:date ;
                     dcterms:description "Examples include paper, canvas, or DVD."@en ;
                     rdfs:isDefinedBy dcterms: ;
                     rdfs:label "Physical Medium"@en ;
                     rdfs:comment "A physical material or carrier."@en .


dcterms:PhysicalResource rdfs:isDefinedBy dcterms: ;
                       dcterms:issued "2008-01-14"^^xsd:date ;
                       rdfs:comment "A material thing."@en ;
                       dcterms:hasVersion <http://dublincore.org/usage/terms/history/#PhysicalResource-001> ;
                       rdfs:label "Physical Resource"@en .


dcterms:Point rdfs:comment "The set of points in space defined by their geographic coordinates according to the DCMI Point Encoding Scheme."@en ;
            rdfs:label "DCMI Point"@en ;
            dcterms:modified "2008-01-14"^^xsd:date ;
            dcterms:issued "2000-07-11"^^xsd:date ;
            dcterms:hasVersion <http://dublincore.org/usage/terms/history/#Point-003> ;
            rdfs:seeAlso <http://dublincore.org/documents/dcmi-point/> ;
            rdfs:isDefinedBy dcterms: .


dcterms:Policy rdfs:isDefinedBy dcterms: ;
             rdfs:label "Policy"@en ;
             rdfs:comment "A plan or course of action by an authority, intended to influence and determine decisions, actions, and other matters."@en ;
             dcterms:hasVersion <http://dublincore.org/usage/terms/history/#Policy-001> ;
             dcterms:issued "2008-01-14"^^xsd:date .


dcterms:ProvenanceStatement rdfs:label "Provenance Statement"@en ;
                          rdfs:isDefinedBy dcterms: ;
                          dcterms:issued "2008-01-14"^^xsd:date ;
                          dcterms:hasVersion <http://dublincore.org/usage/terms/history/#ProvenanceStatement-001> ;
                          rdfs:comment "A statement of any changes in ownership and custody of a resource since its creation that are significant for its authenticity, integrity, and interpretation."@en .


dcterms:RFC1766 rdfs:isDefinedBy dcterms: ;
              dcterms:issued "2000-07-11"^^xsd:date ;
              dcterms:modified "2008-01-14"^^xsd:date ;
              dcterms:hasVersion <http://dublincore.org/usage/terms/history/#RFC1766-003> ;
              rdfs:comment "The set of tags, constructed according to RFC 1766, for the identification of languages."@en ;
              rdfs:seeAlso <http://www.ietf.org/rfc/rfc1766.txt> ;
              rdfs:label "RFC 1766"@en .


dcterms:RFC3066 dcterms:issued "2002-07-13"^^xsd:date ;
              rdfs:label "RFC 3066"@en ;
              rdfs:isDefinedBy dcterms: ;
              dcterms:description "RFC 3066 has been obsoleted by RFC 4646."@en ;
              rdfs:comment "The set of tags constructed according to RFC 3066 for the identification of languages."@en ;
              dcterms:modified "2008-01-14"^^xsd:date ;
              rdfs:seeAlso <http://www.ietf.org/rfc/rfc3066.txt> ;
              dcterms:hasVersion <http://dublincore.org/usage/terms/history/#RFC3066-002> .


dcterms:RFC4646 dcterms:description "RFC 4646 obsoletes RFC 3066."@en ;
              dcterms:issued "2008-01-14"^^xsd:date ;
              dcterms:hasVersion <http://dublincore.org/usage/terms/history/#RFC4646-001> ;
              rdfs:seeAlso <http://www.ietf.org/rfc/rfc4646.txt> ;
              rdfs:isDefinedBy dcterms: ;
              rdfs:label "RFC 4646"@en ;
              rdfs:comment "The set of tags constructed according to RFC 4646 for the identification of languages."@en .


dcterms:RFC5646 dcterms:issued "2010-10-11"^^xsd:date ;
              rdfs:seeAlso <http://www.ietf.org/rfc/rfc5646.txt> ;
              dcterms:hasVersion <http://dublincore.org/usage/terms/history/#RFC5646-001> ;
              rdfs:comment "The set of tags constructed according to RFC 5646 for the identification of languages."@en ;
              rdfs:label "RFC 5646"@en ;
              dcterms:description "RFC 5646 obsoletes RFC 4646."@en ;
              rdfs:isDefinedBy dcterms: .


dcterms:RightsStatement rdfs:label "Rights Statement"@en ;
                      rdfs:isDefinedBy dcterms: ;
                      rdfs:comment "A statement about the intellectual property rights (IPR) held in or over a Resource, a legal document giving official permission to do something with a resource, or a statement about access rights."@en ;
                      dcterms:issued "2008-01-14"^^xsd:date ;
                      dcterms:hasVersion <http://dublincore.org/usage/terms/history/#RightsStatement-001> .


dcterms:SizeOrDuration rdfs:label "Size or Duration"@en ;
                     dcterms:hasVersion <http://dublincore.org/usage/terms/history/#SizeOrDuration-001> ;
                     dcterms:description "Examples include a number of pages, a specification of length, width, and breadth, or a period in hours, minutes, and seconds."@en ;
                     rdfs:comment "A dimension or extent, or a time taken to play or execute."@en ;
                     dcterms:issued "2008-01-14"^^xsd:date ;
                     rdfs:isDefinedBy dcterms: .


dcterms:Standard rdfs:comment "A basis for comparison; a reference point against which other things can be evaluated."@en ;
               rdfs:label "Standard"@en ;
               rdfs:isDefinedBy dcterms: ;
               dcterms:issued "2008-01-14"^^xsd:date ;
               dcterms:hasVersion <http://dublincore.org/usage/terms/history/#Standard-001> .


dcterms:URI rdfs:comment "The set of identifiers constructed according to the generic syntax for Uniform Resource Identifiers as specified by the Internet Engineering Task Force."@en ;
          rdfs:isDefinedBy dcterms: ;
          dcterms:issued "2000-07-11"^^xsd:date ;
          rdfs:seeAlso <http://www.ietf.org/rfc/rfc3986.txt> ;
          dcterms:hasVersion <http://dublincore.org/usage/terms/history/#URI-003> ;
          rdfs:label "URI"@en ;
          dcterms:modified "2008-01-14"^^xsd:date .


dcterms:W3CDTF rdfs:label "W3C-DTF"@en ;
             rdfs:comment "The set of dates and times constructed according to the W3C Date and Time Formats Specification."@en ;
             rdfs:isDefinedBy dcterms: ;
             dcterms:hasVersion <http://dublincore.org/usage/terms/history/#W3CDTF-003> ;
             dcterms:issued "2000-07-11"^^xsd:date ;
             rdfs:seeAlso <http://www.w3.org/TR/NOTE-datetime> ;
             dcterms:modified "2008-01-14"^^xsd:date .


dcterms:abstract rdfs:label "Abstract"@en ;
               dcterms:modified "2008-01-14"^^xsd:date ;
               dcterms:hasVersion <http://dublincore.org/usage/terms/history/#abstract-003> ;
               dcterms:issued "2000-07-11"^^xsd:date ;
               rdfs:comment "A summary of the resource."@en ;
               rdfs:isDefinedBy dcterms: .


dcterms:accessRights dcterms:description "Access Rights may include information regarding access or restrictions based on privacy, security, or other policies."@en ;
                   dcterms:issued "2003-02-15"^^xsd:date ;
                   rdfs:comment "Information about who can access the resource or an indication of its security status."@en ;
                   rdfs:label "Access Rights"@en ;
                   dcterms:modified "2008-01-14"^^xsd:date ;
                   dcterms:hasVersion <http://dublincore.org/usage/terms/history/#accessRights-002> ;
                   rdfs:isDefinedBy dcterms: .


dcterms:accrualMethod rdfs:label "Accrual Method"@en ;
                    dcterms:hasVersion <http://dublincore.org/usage/terms/history/#accrualMethod-003> ;
                    dcterms:modified "2010-10-11"^^xsd:date ;
                    rdfs:comment "The method by which items are added to a collection."@en ;
                    rdfs:isDefinedBy dcterms: ;
                    dcterms:issued "2005-06-13"^^xsd:date .


dcterms:accrualPeriodicity dcterms:modified "2010-10-11"^^xsd:date ;
                         dcterms:hasVersion <http://dublincore.org/usage/terms/history/#accrualPeriodicity-003> ;
                         rdfs:label "Accrual Periodicity"@en ;
                         rdfs:comment "The frequency with which items are added to a collection."@en ;
                         rdfs:isDefinedBy dcterms: ;
                         dcterms:issued "2005-06-13"^^xsd:date .


dcterms:accrualPolicy rdfs:isDefinedBy dcterms: ;
                    dcterms:issued "2005-06-13"^^xsd:date ;
                    dcterms:modified "2010-10-11"^^xsd:date ;
                    dcterms:hasVersion <http://dublincore.org/usage/terms/history/#accrualPolicy-003> ;
                    rdfs:comment "The policy governing the addition of items to a collection."@en ;
                    rdfs:label "Accrual Policy"@en .


dcterms:alternative rdfs:comment "An alternative name for the resource."@en ;
                  rdfs:isDefinedBy dcterms: ;
                  dcterms:hasVersion <http://dublincore.org/usage/terms/history/#alternative-003> ;
                  dcterms:modified "2010-10-11"^^xsd:date ;
                  dcterms:description "The distinction between titles and alternative titles is application-specific."@en ;
                  dcterms:issued "2000-07-11"^^xsd:date ;
                  rdfs:label "Alternative Title"@en .


dcterms:audience dcterms:issued "2001-05-21"^^xsd:date ;
               rdfs:comment "A class of entity for whom the resource is intended or useful."@en ;
               dcterms:hasVersion <http://dublincore.org/usage/terms/history/#audience-003> ;
               rdfs:label "Audience"@en ;
               rdfs:isDefinedBy dcterms: ;
               dcterms:modified "2008-01-14"^^xsd:date .


dcterms:available rdfs:isDefinedBy dcterms: ;
                rdfs:comment "Date (often a range) that the resource became or will become available."@en ;
                rdfs:label "Date Available"@en ;
                dcterms:hasVersion <http://dublincore.org/usage/terms/history/#available-003> ;
                dcterms:modified "2008-01-14"^^xsd:date ;
                dcterms:issued "2000-07-11"^^xsd:date .


dcterms:bibliographicCitation dcterms:modified "2008-01-14"^^xsd:date ;
                            dcterms:description "Recommended practice is to include sufficient bibliographic detail to identify the resource as unambiguously as possible."@en ;
                            rdfs:label "Bibliographic Citation"@en ;
                            dcterms:hasVersion <http://dublincore.org/usage/terms/history/#bibliographicCitation-002> ;
                            rdfs:comment "A bibliographic reference for the resource."@en ;
                            rdfs:isDefinedBy dcterms: ;
                            dcterms:issued "2003-02-15"^^xsd:date .


dcterms:conformsTo rdfs:isDefinedBy dcterms: ;
                 rdfs:label "Conforms To"@en ;
                 rdfs:comment "An established standard to which the described resource conforms."@en ;
                 dcterms:modified "2008-01-14"^^xsd:date ;
                 dcterms:hasVersion <http://dublincore.org/usage/terms/history/#conformsTo-003> ;
                 dcterms:issued "2001-05-21"^^xsd:date .


dcterms:contributor rdfs:comment "An entity responsible for making contributions to the resource."@en ;
                  dcterms:modified "2010-10-11"^^xsd:date ;
                  rdfs:isDefinedBy dcterms: ;
                  dcterms:description "Examples of a Contributor include a person, an organization, or a service."@en ;
                  dcterms:issued "2008-01-14"^^xsd:date ;
                  dcterms:hasVersion <http://dublincore.org/usage/terms/history/#contributorT-001> ;
                  rdfs:label "Contributor"@en .


dcterms:coverage rdfs:isDefinedBy dcterms: ;
               dcterms:hasVersion <http://dublincore.org/usage/terms/history/#coverageT-001> ;
               dcterms:description "Spatial topic and spatial applicability may be a named place or a location specified by its geographic coordinates. Temporal topic may be a named period, date, or date range. A jurisdiction may be a named administrative entity or a geographic place to which the resource applies. Recommended best practice is to use a controlled vocabulary such as the Thesaurus of Geographic Names [TGN]. Where appropriate, named places or time periods can be used in preference to numeric identifiers such as sets of coordinates or date ranges."@en ;
               rdfs:label "Coverage"@en ;
               dcterms:issued "2008-01-14"^^xsd:date ;
               rdfs:comment "The spatial or temporal topic of the resource, the spatial applicability of the resource, or the jurisdiction under which the resource is relevant."@en ;
               dcterms:modified "2008-01-14"^^xsd:date .


dcterms:created rdfs:isDefinedBy dcterms: ;
              rdfs:comment "Date of creation of the resource."@en ;
              dcterms:hasVersion <http://dublincore.org/usage/terms/history/#created-003> ;
              dcterms:modified "2008-01-14"^^xsd:date ;
              rdfs:label "Date Created"@en ;
              dcterms:issued "2000-07-11"^^xsd:date .


dcterms:creator rdfs:comment "An entity primarily responsible for making the resource."@en ;
              dcterms:hasVersion <http://dublincore.org/usage/terms/history/#creatorT-002> ;
              rdfs:isDefinedBy dcterms: ;
              dcterms:modified "2010-10-11"^^xsd:date ;
              dcterms:issued "2008-01-14"^^xsd:date ;
              rdfs:label "Creator"@en ;
              dcterms:description "Examples of a Creator include a person, an organization, or a service."@en .


dcterms:date rdfs:isDefinedBy dcterms: ;
           dcterms:hasVersion <http://dublincore.org/usage/terms/history/#dateT-001> ;
           rdfs:comment "A point or period of time associated with an event in the lifecycle of the resource."@en ;
           dcterms:description "Date may be used to express temporal information at any level of granularity.  Recommended best practice is to use an encoding scheme, such as the W3CDTF profile of ISO 8601 [W3CDTF]."@en ;
           rdfs:label "Date"@en ;
           dcterms:issued "2008-01-14"^^xsd:date ;
           dcterms:modified "2008-01-14"^^xsd:date .


dcterms:dateAccepted dcterms:modified "2008-01-14"^^xsd:date ;
                   dcterms:hasVersion <http://dublincore.org/usage/terms/history/#dateAccepted-002> ;
                   dcterms:issued "2002-07-13"^^xsd:date ;
                   dcterms:description "Examples of resources to which a Date Accepted may be relevant are a thesis (accepted by a university department) or an article (accepted by a journal)."@en ;
                   rdfs:label "Date Accepted"@en ;
                   rdfs:comment "Date of acceptance of the resource."@en ;
                   rdfs:isDefinedBy dcterms: .


dcterms:dateCopyrighted rdfs:isDefinedBy dcterms: ;
                      rdfs:label "Date Copyrighted"@en ;
                      rdfs:comment "Date of copyright."@en ;
                      dcterms:modified "2008-01-14"^^xsd:date ;
                      dcterms:hasVersion <http://dublincore.org/usage/terms/history/#dateCopyrighted-002> ;
                      dcterms:issued "2002-07-13"^^xsd:date .


dcterms:dateSubmitted dcterms:modified "2008-01-14"^^xsd:date ;
                    rdfs:comment "Date of submission of the resource."@en ;
                    dcterms:description "Examples of resources to which a Date Submitted may be relevant are a thesis (submitted to a university department) or an article (submitted to a journal)."@en ;
                    dcterms:issued "2002-07-13"^^xsd:date ;
                    rdfs:label "Date Submitted"@en ;
                    dcterms:hasVersion <http://dublincore.org/usage/terms/history/#dateSubmitted-002> ;
                    rdfs:isDefinedBy dcterms: .


dcterms:description dcterms:modified "2008-01-14"^^xsd:date ;
                  rdfs:label "Description"@en ;
                  rdfs:isDefinedBy dcterms: ;
                  dcterms:issued "2008-01-14"^^xsd:date ;
                  dcterms:hasVersion <http://dublincore.org/usage/terms/history/#descriptionT-001> ;
                  rdfs:comment "An account of the resource."@en ;
                  dcterms:description "Description may include but is not limited to: an abstract, a table of contents, a graphical representation, or a free-text account of the resource."@en .


dcterms:educationLevel dcterms:modified "2008-01-14"^^xsd:date ;
                     rdfs:isDefinedBy dcterms: ;
                     dcterms:issued "2002-07-13"^^xsd:date ;
                     rdfs:label "Audience Education Level"@en ;
                     rdfs:comment "A class of entity, defined in terms of progression through an educational or training context, for which the described resource is intended."@en ;
                     dcterms:hasVersion <http://dublincore.org/usage/terms/history/#educationLevel-002> .


dcterms:extent dcterms:modified "2008-01-14"^^xsd:date ;
             dcterms:issued "2000-07-11"^^xsd:date ;
             rdfs:isDefinedBy dcterms: ;
             rdfs:comment "The size or duration of the resource."@en ;
             rdfs:label "Extent"@en ;
             dcterms:hasVersion <http://dublincore.org/usage/terms/history/#extent-003> .


dcterms:format dcterms:issued "2008-01-14"^^xsd:date ;
             dcterms:hasVersion <http://dublincore.org/usage/terms/history/#formatT-001> ;
             dcterms:modified "2008-01-14"^^xsd:date ;
             rdfs:comment "The file format, physical medium, or dimensions of the resource."@en ;
             dcterms:description "Examples of dimensions include size and duration. Recommended best practice is to use a controlled vocabulary such as the list of Internet Media Types [MIME]."@en ;
             rdfs:isDefinedBy dcterms: ;
             rdfs:label "Format"@en .


dcterms:hasFormat rdfs:isDefinedBy dcterms: ;
                skos:note "This term is intended to be used with non-literal values as defined in the DCMI Abstract Model (http://dublincore.org/documents/abstract-model/).  As of December 2007, the DCMI Usage Board is seeking a way to express this intention with a formal range declaration."@en ;
                dcterms:hasVersion <http://dublincore.org/usage/terms/history/#hasFormat-003> ;
                dcterms:modified "2008-01-14"^^xsd:date ;
                rdfs:label "Has Format"@en ;
                rdfs:comment "A related resource that is substantially the same as the pre-existing described resource, but in another format."@en ;
                dcterms:issued "2000-07-11"^^xsd:date .


dcterms:hasPart rdfs:isDefinedBy dcterms: ;
              skos:note "This term is intended to be used with non-literal values as defined in the DCMI Abstract Model (http://dublincore.org/documents/abstract-model/).  As of December 2007, the DCMI Usage Board is seeking a way to express this intention with a formal range declaration."@en ;
              dcterms:issued "2000-07-11"^^xsd:date ;
              rdfs:label "Has Part"@en ;
              dcterms:modified "2008-01-14"^^xsd:date ;
              rdfs:comment "A related resource that is included either physically or logically in the described resource."@en ;
              dcterms:hasVersion <http://dublincore.org/usage/terms/history/#hasPart-003> .


dcterms:hasVersion dcterms:hasVersion <http://dublincore.org/usage/terms/history/#hasVersion-003> ;
                 rdfs:isDefinedBy dcterms: ;
                 rdfs:comment "A related resource that is a version, edition, or adaptation of the described resource."@en ;
                 skos:note "This term is intended to be used with non-literal values as defined in the DCMI Abstract Model (http://dublincore.org/documents/abstract-model/).  As of December 2007, the DCMI Usage Board is seeking a way to express this intention with a formal range declaration."@en ;
                 rdfs:label "Has Version"@en ;
                 dcterms:issued "2000-07-11"^^xsd:date ;
                 dcterms:modified "2008-01-14"^^xsd:date .


dcterms:identifier dcterms:hasVersion <http://dublincore.org/usage/terms/history/#identifierT-001> ;
                 rdfs:isDefinedBy dcterms: ;
                 dcterms:description "Recommended best practice is to identify the resource by means of a string conforming to a formal identification system. "@en ;
                 dcterms:modified "2008-01-14"^^xsd:date ;
                 rdfs:comment "An unambiguous reference to the resource within a given context."@en ;
                 rdfs:label "Identifier"@en ;
                 dcterms:issued "2008-01-14"^^xsd:date .


dcterms:instructionalMethod dcterms:issued "2005-06-13"^^xsd:date ;
                          dcterms:description "Instructional Method will typically include ways of presenting instructional materials or conducting instructional activities, patterns of learner-to-learner and learner-to-instructor interactions, and mechanisms by which group and individual levels of learning are measured.  Instructional methods include all aspects of the instruction and learning processes from planning and implementation through evaluation and feedback."@en ;
                          rdfs:label "Instructional Method"@en ;
                          dcterms:modified "2008-01-14"^^xsd:date ;
                          rdfs:comment "A process, used to engender knowledge, attitudes and skills, that the described resource is designed to support."@en ;
                          dcterms:hasVersion <http://dublincore.org/usage/terms/history/#instructionalMethod-002> ;
                          rdfs:isDefinedBy dcterms: .


dcterms:isFormatOf dcterms:hasVersion <http://dublincore.org/usage/terms/history/#isFormatOf-003> ;
                 dcterms:modified "2008-01-14"^^xsd:date ;
                 rdfs:comment "A related resource that is substantially the same as the described resource, but in another format."@en ;
                 dcterms:issued "2000-07-11"^^xsd:date ;
                 skos:note "This term is intended to be used with non-literal values as defined in the DCMI Abstract Model (http://dublincore.org/documents/abstract-model/).  As of December 2007, the DCMI Usage Board is seeking a way to express this intention with a formal range declaration."@en ;
                 rdfs:label "Is Format Of"@en ;
                 rdfs:isDefinedBy dcterms: .


dcterms:isPartOf dcterms:modified "2008-01-14"^^xsd:date ;
               rdfs:label "Is Part Of"@en ;
               dcterms:hasVersion <http://dublincore.org/usage/terms/history/#isPartOf-003> ;
               dcterms:issued "2000-07-11"^^xsd:date ;
               skos:note "This term is intended to be used with non-literal values as defined in the DCMI Abstract Model (http://dublincore.org/documents/abstract-model/).  As of December 2007, the DCMI Usage Board is seeking a way to express this intention with a formal range declaration."@en ;
               rdfs:isDefinedBy dcterms: ;
               rdfs:comment "A related resource in which the described resource is physically or logically included."@en .


dcterms:isReferencedBy rdfs:label "Is Referenced By"@en ;
                     rdfs:comment "A related resource that references, cites, or otherwise points to the described resource."@en ;
                     dcterms:modified "2008-01-14"^^xsd:date ;
                     skos:note "This term is intended to be used with non-literal values as defined in the DCMI Abstract Model (http://dublincore.org/documents/abstract-model/).  As of December 2007, the DCMI Usage Board is seeking a way to express this intention with a formal range declaration."@en ;
                     rdfs:isDefinedBy dcterms: ;
                     dcterms:issued "2000-07-11"^^xsd:date ;
                     dcterms:hasVersion <http://dublincore.org/usage/terms/history/#isReferencedBy-003> .


dcterms:isReplacedBy rdfs:isDefinedBy dcterms: ;
                   rdfs:label "Is Replaced By"@en ;
                   dcterms:modified "2008-01-14"^^xsd:date ;
                   rdfs:comment "A related resource that supplants, displaces, or supersedes the described resource."@en ;
                   dcterms:issued "2000-07-11"^^xsd:date ;
                   skos:note "This term is intended to be used with non-literal values as defined in the DCMI Abstract Model (http://dublincore.org/documents/abstract-model/).  As of December 2007, the DCMI Usage Board is seeking a way to express this intention with a formal range declaration."@en ;
                   dcterms:hasVersion <http://dublincore.org/usage/terms/history/#isReplacedBy-003> .


dcterms:isRequiredBy rdfs:isDefinedBy dcterms: ;
                   skos:note "This term is intended to be used with non-literal values as defined in the DCMI Abstract Model (http://dublincore.org/documents/abstract-model/).  As of December 2007, the DCMI Usage Board is seeking a way to express this intention with a formal range declaration."@en ;
                   dcterms:issued "2000-07-11"^^xsd:date ;
                   rdfs:label "Is Required By"@en ;
                   dcterms:hasVersion <http://dublincore.org/usage/terms/history/#isRequiredBy-003> ;
                   dcterms:modified "2008-01-14"^^xsd:date ;
                   rdfs:comment "A related resource that requires the described resource to support its function, delivery, or coherence."@en .


dcterms:isVersionOf rdfs:label "Is Version Of"@en ;
                  rdfs:comment "A related resource of which the described resource is a version, edition, or adaptation."@en ;
                  rdfs:isDefinedBy dcterms: ;
                  dcterms:issued "2000-07-11"^^xsd:date ;
                  skos:note "This term is intended to be used with non-literal values as defined in the DCMI Abstract Model (http://dublincore.org/documents/abstract-model/).  As of December 2007, the DCMI Usage Board is seeking a way to express this intention with a formal range declaration."@en ;
                  dcterms:hasVersion <http://dublincore.org/usage/terms/history/#isVersionOf-003> ;
                  dcterms:modified "2008-01-14"^^xsd:date ;
                  dcterms:description "Changes in version imply substantive changes in content rather than differences in format."@en .


dcterms:issued dcterms:modified "2008-01-14"^^xsd:date ;
             rdfs:comment "Date of formal issuance (e.g., publication) of the resource."@en ;
             rdfs:isDefinedBy dcterms: ;
             dcterms:hasVersion <http://dublincore.org/usage/terms/history/#issued-003> ;
             dcterms:issued "2000-07-11"^^xsd:date ;
             rdfs:label "Date Issued"@en .


dcterms:language rdfs:label "Language"@en ;
               dcterms:issued "2008-01-14"^^xsd:date ;
               dcterms:hasVersion <http://dublincore.org/usage/terms/history/#languageT-001> ;
               dcterms:modified "2008-01-14"^^xsd:date ;
               dcterms:description "Recommended best practice is to use a controlled vocabulary such as RFC 4646 [RFC4646]."@en ;
               rdfs:isDefinedBy dcterms: ;
               rdfs:comment "A language of the resource."@en .


dcterms:license dcterms:issued "2004-06-14"^^xsd:date ;
              rdfs:label "License"@en ;
              rdfs:comment "A legal document giving official permission to do something with the resource."@en ;
              dcterms:modified "2008-01-14"^^xsd:date ;
              dcterms:hasVersion <http://dublincore.org/usage/terms/history/#license-002> ;
              rdfs:isDefinedBy dcterms: .


dcterms:mediator dcterms:description "In an educational context, a mediator might be a parent, teacher, teaching assistant, or care-giver."@en ;
               dcterms:modified "2008-01-14"^^xsd:date ;
               rdfs:comment "An entity that mediates access to the resource and for whom the resource is intended or useful."@en ;
               dcterms:hasVersion <http://dublincore.org/usage/terms/history/#mediator-003> ;
               rdfs:isDefinedBy dcterms: ;
               rdfs:label "Mediator"@en ;
               dcterms:issued "2001-05-21"^^xsd:date .


dcterms:medium rdfs:isDefinedBy dcterms: ;
             rdfs:label "Medium"@en ;
             rdfs:comment "The material or physical carrier of the resource."@en ;
             dcterms:issued "2000-07-11"^^xsd:date ;
             dcterms:modified "2008-01-14"^^xsd:date ;
             dcterms:hasVersion <http://dublincore.org/usage/terms/history/#medium-003> .


dcterms:modified rdfs:isDefinedBy dcterms: ;
               rdfs:label "Date Modified"@en ;
               dcterms:hasVersion <http://dublincore.org/usage/terms/history/#modified-003> ;
               dcterms:modified "2008-01-14"^^xsd:date ;
               rdfs:comment "Date on which the resource was changed."@en ;
               dcterms:issued "2000-07-11"^^xsd:date .


dcterms:provenance rdfs:comment "A statement of any changes in ownership and custody of the resource since its creation that are significant for its authenticity, integrity, and interpretation."@en ;
                 dcterms:modified "2008-01-14"^^xsd:date ;
                 dcterms:issued "2004-09-20"^^xsd:date ;
                 rdfs:isDefinedBy dcterms: ;
                 dcterms:description "The statement may include a description of any changes successive custodians made to the resource."@en ;
                 dcterms:hasVersion <http://dublincore.org/usage/terms/history/#provenance-002> ;
                 rdfs:label "Provenance"@en .


dcterms:publisher dcterms:modified "2010-10-11"^^xsd:date ;
                dcterms:issued "2008-01-14"^^xsd:date ;
                rdfs:label "Publisher"@en ;
                dcterms:hasVersion <http://dublincore.org/usage/terms/history/#publisherT-001> ;
                dcterms:description "Examples of a Publisher include a person, an organization, or a service."@en ;
                rdfs:isDefinedBy dcterms: ;
                rdfs:comment "An entity responsible for making the resource available."@en .


dcterms:references rdfs:comment "A related resource that is referenced, cited, or otherwise pointed to by the described resource."@en ;
                 rdfs:label "References"@en ;
                 dcterms:modified "2008-01-14"^^xsd:date ;
                 dcterms:issued "2000-07-11"^^xsd:date ;
                 dcterms:hasVersion <http://dublincore.org/usage/terms/history/#references-003> ;
                 rdfs:isDefinedBy dcterms: ;
                 skos:note "This term is intended to be used with non-literal values as defined in the DCMI Abstract Model (http://dublincore.org/documents/abstract-model/).  As of December 2007, the DCMI Usage Board is seeking a way to express this intention with a formal range declaration."@en .


dcterms:relation dcterms:issued "2008-01-14"^^xsd:date ;
               skos:note "This term is intended to be used with non-literal values as defined in the DCMI Abstract Model (http://dublincore.org/documents/abstract-model/).  As of December 2007, the DCMI Usage Board is seeking a way to express this intention with a formal range declaration."@en ;
               rdfs:isDefinedBy dcterms: ;
               dcterms:hasVersion <http://dublincore.org/usage/terms/history/#relationT-001> ;
               rdfs:label "Relation"@en ;
               dcterms:description "Recommended best practice is to identify the related resource by means of a string conforming to a formal identification system. "@en ;
               rdfs:comment "A related resource."@en ;
               dcterms:modified "2008-01-14"^^xsd:date .


dcterms:replaces skos:note "This term is intended to be used with non-literal values as defined in the DCMI Abstract Model (http://dublincore.org/documents/abstract-model/).  As of December 2007, the DCMI Usage Board is seeking a way to express this intention with a formal range declaration."@en ;
               dcterms:issued "2000-07-11"^^xsd:date ;
               dcterms:modified "2008-01-14"^^xsd:date ;
               rdfs:label "Replaces"@en ;
               dcterms:hasVersion <http://dublincore.org/usage/terms/history/#replaces-003> ;
               rdfs:comment "A related resource that is supplanted, displaced, or superseded by the described resource."@en ;
               rdfs:isDefinedBy dcterms: .


dcterms:requires dcterms:hasVersion <http://dublincore.org/usage/terms/history/#requires-003> ;
               dcterms:modified "2008-01-14"^^xsd:date ;
               rdfs:label "Requires"@en ;
               rdfs:comment "A related resource that is required by the described resource to support its function, delivery, or coherence."@en ;
               rdfs:isDefinedBy dcterms: ;
               dcterms:issued "2000-07-11"^^xsd:date ;
               skos:note "This term is intended to be used with non-literal values as defined in the DCMI Abstract Model (http://dublincore.org/documents/abstract-model/).  As of December 2007, the DCMI Usage Board is seeking a way to express this intention with a formal range declaration."@en .


dcterms:rights dcterms:issued "2008-01-14"^^xsd:date ;
             rdfs:isDefinedBy dcterms: ;
             rdfs:label "Rights"@en ;
             rdfs:comment "Information about rights held in and over the resource."@en ;
             dcterms:modified "2008-01-14"^^xsd:date ;
             dcterms:hasVersion <http://dublincore.org/usage/terms/history/#rightsT-001> ;
             dcterms:description "Typically, rights information includes a statement about various property rights associated with the resource, including intellectual property rights."@en .


dcterms:rightsHolder dcterms:hasVersion <http://dublincore.org/usage/terms/history/#rightsHolder-002> ;
                   rdfs:isDefinedBy dcterms: ;
                   dcterms:modified "2008-01-14"^^xsd:date ;
                   rdfs:comment "A person or organization owning or managing rights over the resource."@en ;
                   dcterms:issued "2004-06-14"^^xsd:date ;
                   rdfs:label "Rights Holder"@en .


dcterms:source rdfs:label "Source"@en ;
             skos:note "This term is intended to be used with non-literal values as defined in the DCMI Abstract Model (http://dublincore.org/documents/abstract-model/).  As of December 2007, the DCMI Usage Board is seeking a way to express this intention with a formal range declaration."@en ;
             dcterms:issued "2008-01-14"^^xsd:date ;
             rdfs:isDefinedBy dcterms: ;
             dcterms:modified "2008-01-14"^^xsd:date ;
             dcterms:hasVersion <http://dublincore.org/usage/terms/history/#sourceT-001> ;
             rdfs:comment "A related resource from which the described resource is derived."@en ;
             dcterms:description "The described resource may be derived from the related resource in whole or in part. Recommended best practice is to identify the related resource by means of a string conforming to a formal identification system."@en .


dcterms:spatial rdfs:label "Spatial Coverage"@en ;
              dcterms:issued "2000-07-11"^^xsd:date ;
              rdfs:isDefinedBy dcterms: ;
              rdfs:comment "Spatial characteristics of the resource."@en ;
              dcterms:modified "2008-01-14"^^xsd:date ;
              dcterms:hasVersion <http://dublincore.org/usage/terms/history/#spatial-003> .


dcterms:subject dcterms:modified "2012-06-14"^^xsd:date ;
              dcterms:hasVersion <http://dublincore.org/usage/terms/history/#subjectT-002> ;
              skos:note "This term is intended to be used with non-literal values as defined in the DCMI Abstract Model (http://dublincore.org/documents/abstract-model/).  As of December 2007, the DCMI Usage Board is seeking a way to express this intention with a formal range declaration."@en ;
              dcterms:issued "2008-01-14"^^xsd:date ;
              rdfs:label "Subject"@en ;
              rdfs:comment "The topic of the resource."@en ;
              dcterms:description "Typically, the subject will be represented using keywords, key phrases, or classification codes. Recommended best practice is to use a controlled vocabulary."@en ;
              rdfs:isDefinedBy dcterms: .


dcterms:tableOfContents rdfs:comment "A list of subunits of the resource."@en ;
                      dcterms:issued "2000-07-11"^^xsd:date ;
                      rdfs:isDefinedBy dcterms: ;
                      rdfs:label "Table Of Contents"@en ;
                      dcterms:modified "2008-01-14"^^xsd:date ;
                      dcterms:hasVersion <http://dublincore.org/usage/terms/history/#tableOfContents-003> .


dcterms:temporal dcterms:modified "2008-01-14"^^xsd:date ;
               dcterms:issued "2000-07-11"^^xsd:date ;
               rdfs:label "Temporal Coverage"@en ;
               rdfs:comment "Temporal characteristics of the resource."@en ;
               dcterms:hasVersion <http://dublincore.org/usage/terms/history/#temporal-003> ;
               rdfs:isDefinedBy dcterms: .


dcterms:title rdfs:label "Title"@en ;
            rdfs:comment "A name given to the resource."@en ;
            dcterms:issued "2008-01-14"^^xsd:date ;
            dcterms:hasVersion <http://dublincore.org/usage/terms/history/#titleT-002> ;
            rdfs:isDefinedBy dcterms: ;
            dcterms:modified "2010-10-11"^^xsd:date .


dcterms:type rdfs:isDefinedBy dcterms: ;
           dcterms:description "Recommended best practice is to use a controlled vocabulary such as the DCMI Type Vocabulary [DCMITYPE]. To describe the file format, physical medium, or dimensions of the resource, use the Format element."@en ;
           rdfs:comment "The nature or genre of the resource."@en ;
           rdfs:label "Type"@en ;
           dcterms:modified "2008-01-14"^^xsd:date ;
           dcterms:hasVersion <http://dublincore.org/usage/terms/history/#typeT-001> ;
           dcterms:issued "2008-01-14"^^xsd:date .


dcterms:valid rdfs:comment "Date (often a range) of validity of a resource."@en ;
            dcterms:modified "2008-01-14"^^xsd:date ;
            dcterms:issued "2000-07-11"^^xsd:date ;
            rdfs:label "Date Valid"@en ;
            dcterms:hasVersion <http://dublincore.org/usage/terms/history/#valid-003> ;
            rdfs:isDefinedBy dcterms: .


###  Generated by the OWL API (version 4.2.8.20170104-2310) https://github.com/owlcs/owlapi
